@prefix foaf: <http://xmlns.com/foaf/0.1/> .
@prefix cc: <http://creativecommons.org/ns#> .
@prefix xsd: <http://www.w3.org/2001/XMLSchema#> .
@prefix dc: <http://purl.org/dc/terms/> .
@prefix owl: <http://www.w3.org/2002/07/owl#> .
@prefix ns0: <http://purl.org/vocab/vann/> .
@prefix rdfs: <http://www.w3.org/2000/01/rdf-schema#> .
@prefix schema: <http://schema.org/> .

<http://datex2.eu/vocab/3/LocationReferencing>
  a foaf:Document ;
  cc:license "http://creativecommons.org/licenses/by/3.0/"^^xsd:string ;
  dc:hasFormat "http://datex2.eu/vocab/3/LocationReferencing/vocabulary.jsonld"^^xsd:string ;
  dc:issued "2023-11-10"^^xsd:date ;
  dc:modified "2023-11-10"^^xsd:date ;
  dc:rights "Copyright 2023 - DATEX TMG"^^xsd:string ;
  foaf:primaryTopic <http://datex2.eu/vocab/3/LocationReferencing/Ontology> .

<http://datex2.eu/vocab/3/LocationReferencing/Ontology>
  a owl:Ontology ;
  dc:creator "DATEX TMG "^^xsd:string ;
  dc:description "This document gives URIs to all terms used within Datex II"@en ;
  dc:title "DATEX II"@en ;
  ns0:preferredNamespacePrefix "datex_LocationReferencing"^^xsd:string ;
  ns0:preferredNamespaceUri "http://datex2.eu/vocab/3/LocationReferencing"^^xsd:string ;
  rdfs:comment "A mapping of DATEX II to a Linked Data vocabulary"@en ;
  rdfs:label "Linked DATEX II"@en ;
  rdfs:seeAlso <http://datex2.eu/schema/3/LocationReferencing> .

<http://datex2.eu/vocab/3/LocationReferencing/PositionConfidenceCodedErrorEnum>
  a owl:Class ;
  rdfs:comment "Position confidence coded error enum"@en ;
  rdfs:label "Position confidence coded error enum"@en ;
  rdfs:subClassOf schema:Enumeration .

<http://datex2.eu/vocab/3/LocationReferencing/PositionConfidenceCodedErrorEnum#outOfRange>
  a <http://datex2.eu/vocab/3/LocationReferencing/PositionConfidenceCodedErrorEnum> ;
  rdfs:comment "Indicates the accuracy is out of range, i.e. greater than 4 093 cm for horizontal position."@en ;
  rdfs:label "Position confidence coded error enum out of range"@en .

<http://datex2.eu/vocab/3/LocationReferencing/PositionConfidenceCodedErrorEnum#unavailable>
  a <http://datex2.eu/vocab/3/LocationReferencing/PositionConfidenceCodedErrorEnum> ;
  rdfs:comment "Indicates the accuracy information is unavailable."@en ;
  rdfs:label "Position confidence coded error enum unavailable"@en .

<http://datex2.eu/vocab/3/LocationReferencing/LinearElementNatureEnum>
  a owl:Class ;
  rdfs:comment "Linear element nature enum"@en ;
  rdfs:label "Linear element nature enum"@en ;
  rdfs:subClassOf schema:Enumeration .

<http://datex2.eu/vocab/3/LocationReferencing/LinearElementNatureEnum#road>
  a <http://datex2.eu/vocab/3/LocationReferencing/LinearElementNatureEnum> ;
  rdfs:comment "The nature of the linear element is a road."@en ;
  rdfs:label "Linear element nature enum road"@en .

<http://datex2.eu/vocab/3/LocationReferencing/LinearElementNatureEnum#roadSection>
  a <http://datex2.eu/vocab/3/LocationReferencing/LinearElementNatureEnum> ;
  rdfs:comment "The nature of the linear element is a section of a road."@en ;
  rdfs:label "Linear element nature enum road section"@en .

<http://datex2.eu/vocab/3/LocationReferencing/LinearElementNatureEnum#slipRoad>
  a <http://datex2.eu/vocab/3/LocationReferencing/LinearElementNatureEnum> ;
  rdfs:comment "The nature of the linear element is a slip road."@en ;
  rdfs:label "Linear element nature enum slip road"@en .

<http://datex2.eu/vocab/3/LocationReferencing/LinearElementNatureEnum#other>
  a <http://datex2.eu/vocab/3/LocationReferencing/LinearElementNatureEnum> ;
  rdfs:comment "Other than as defined in this enumeration."@en ;
  rdfs:label "Linear element nature enum other"@en .

<http://datex2.eu/vocab/3/LocationReferencing/TpegLoc03IlcPointDescriptorSubtypeEnum>
  a owl:Class ;
  rdfs:comment "TPEG loc03 ILC point descriptor subtype enum"@en ;
  rdfs:label "TPEG loc03 ILC point descriptor subtype enum"@en ;
  rdfs:subClassOf schema:Enumeration .

<http://datex2.eu/vocab/3/LocationReferencing/TpegLoc03IlcPointDescriptorSubtypeEnum#tpegIlcName1>
  a <http://datex2.eu/vocab/3/LocationReferencing/TpegLoc03IlcPointDescriptorSubtypeEnum> ;
  rdfs:comment "The name of the road on which the junction point is located."@en ;
  rdfs:label "TPEG loc03 ILC point descriptor subtype enum tpeg ILC name1"@en .

<http://datex2.eu/vocab/3/LocationReferencing/TpegLoc03IlcPointDescriptorSubtypeEnum#tpegIlcName2>
  a <http://datex2.eu/vocab/3/LocationReferencing/TpegLoc03IlcPointDescriptorSubtypeEnum> ;
  rdfs:comment "The name of the first intersecting road at the junction."@en ;
  rdfs:label "TPEG loc03 ILC point descriptor subtype enum tpeg ILC name2"@en .

<http://datex2.eu/vocab/3/LocationReferencing/TpegLoc03IlcPointDescriptorSubtypeEnum#tpegIlcName3>
  a <http://datex2.eu/vocab/3/LocationReferencing/TpegLoc03IlcPointDescriptorSubtypeEnum> ;
  rdfs:comment "The name of the second intersecting road (if one exists) at the junction."@en ;
  rdfs:label "TPEG loc03 ILC point descriptor subtype enum tpeg ILC name3"@en .

<http://datex2.eu/vocab/3/LocationReferencing/DirectionEnum>
  a owl:Class ;
  rdfs:comment "Direction enum"@en ;
  rdfs:label "Direction enum"@en ;
  rdfs:subClassOf schema:Enumeration .

<http://datex2.eu/vocab/3/LocationReferencing/DirectionEnum#aligned>
  a <http://datex2.eu/vocab/3/LocationReferencing/DirectionEnum> ;
  rdfs:comment "Same direction as the normal direction of flow at this point on the road network."@en ;
  rdfs:label "Direction enum aligned"@en .

<http://datex2.eu/vocab/3/LocationReferencing/DirectionEnum#allDirections>
  a <http://datex2.eu/vocab/3/LocationReferencing/DirectionEnum> ;
  rdfs:comment "All directions (where more than two are applicable) at this point on the road network."@en ;
  rdfs:label "Direction enum all directions"@en .

<http://datex2.eu/vocab/3/LocationReferencing/DirectionEnum#anticlockwise>
  a <http://datex2.eu/vocab/3/LocationReferencing/DirectionEnum> ;
  rdfs:comment "Anti-clockwise."@en ;
  rdfs:label "Direction enum anticlockwise"@en .

<http://datex2.eu/vocab/3/LocationReferencing/DirectionEnum#bothWays>
  a <http://datex2.eu/vocab/3/LocationReferencing/DirectionEnum> ;
  rdfs:comment "Both directions that are applicable at this point on the road network."@en ;
  rdfs:label "Direction enum both ways"@en .

<http://datex2.eu/vocab/3/LocationReferencing/DirectionEnum#clockwise>
  a <http://datex2.eu/vocab/3/LocationReferencing/DirectionEnum> ;
  rdfs:comment "Clockwise."@en ;
  rdfs:label "Direction enum clockwise"@en .

<http://datex2.eu/vocab/3/LocationReferencing/DirectionEnum#innerRing>
  a <http://datex2.eu/vocab/3/LocationReferencing/DirectionEnum> ;
  rdfs:comment "Inner ring direction."@en ;
  rdfs:label "Direction enum inner ring"@en .

<http://datex2.eu/vocab/3/LocationReferencing/DirectionEnum#outerRing>
  a <http://datex2.eu/vocab/3/LocationReferencing/DirectionEnum> ;
  rdfs:comment "Outer ring direction."@en ;
  rdfs:label "Direction enum outer ring"@en .

<http://datex2.eu/vocab/3/LocationReferencing/DirectionEnum#eastBound>
  a <http://datex2.eu/vocab/3/LocationReferencing/DirectionEnum> ;
  rdfs:comment "East bound general direction."@en ;
  rdfs:label "Direction enum east bound"@en .

<http://datex2.eu/vocab/3/LocationReferencing/DirectionEnum#northBound>
  a <http://datex2.eu/vocab/3/LocationReferencing/DirectionEnum> ;
  rdfs:comment "North bound general direction."@en ;
  rdfs:label "Direction enum north bound"@en .

<http://datex2.eu/vocab/3/LocationReferencing/DirectionEnum#northEastBound>
  a <http://datex2.eu/vocab/3/LocationReferencing/DirectionEnum> ;
  rdfs:comment "North east bound general direction."@en ;
  rdfs:label "Direction enum north east bound"@en .

<http://datex2.eu/vocab/3/LocationReferencing/DirectionEnum#northWestBound>
  a <http://datex2.eu/vocab/3/LocationReferencing/DirectionEnum> ;
  rdfs:comment "North west bound general direction."@en ;
  rdfs:label "Direction enum north west bound"@en .

<http://datex2.eu/vocab/3/LocationReferencing/DirectionEnum#southBound>
  a <http://datex2.eu/vocab/3/LocationReferencing/DirectionEnum> ;
  rdfs:comment "South bound general direction."@en ;
  rdfs:label "Direction enum south bound"@en .

<http://datex2.eu/vocab/3/LocationReferencing/DirectionEnum#southEastBound>
  a <http://datex2.eu/vocab/3/LocationReferencing/DirectionEnum> ;
  rdfs:comment "South east bound general direction."@en ;
  rdfs:label "Direction enum south east bound"@en .

<http://datex2.eu/vocab/3/LocationReferencing/DirectionEnum#southWestBound>
  a <http://datex2.eu/vocab/3/LocationReferencing/DirectionEnum> ;
  rdfs:comment "South west bound general direction."@en ;
  rdfs:label "Direction enum south west bound"@en .

<http://datex2.eu/vocab/3/LocationReferencing/DirectionEnum#westBound>
  a <http://datex2.eu/vocab/3/LocationReferencing/DirectionEnum> ;
  rdfs:comment "West bound general direction."@en ;
  rdfs:label "Direction enum west bound"@en .

<http://datex2.eu/vocab/3/LocationReferencing/DirectionEnum#inboundTowardsTown>
  a <http://datex2.eu/vocab/3/LocationReferencing/DirectionEnum> ;
  rdfs:comment "Heading towards town centre direction of travel."@en ;
  rdfs:label "Direction enum inbound towards town"@en .

<http://datex2.eu/vocab/3/LocationReferencing/DirectionEnum#outboundFromTown>
  a <http://datex2.eu/vocab/3/LocationReferencing/DirectionEnum> ;
  rdfs:comment "Heading out of or away from the town centre direction of travel."@en ;
  rdfs:label "Direction enum outbound from town"@en .

<http://datex2.eu/vocab/3/LocationReferencing/DirectionEnum#opposite>
  a <http://datex2.eu/vocab/3/LocationReferencing/DirectionEnum> ;
  rdfs:comment "Opposite direction to the normal direction of flow at this point on the road network."@en ;
  rdfs:label "Direction enum opposite"@en .

<http://datex2.eu/vocab/3/LocationReferencing/DirectionEnum#unknown>
  a <http://datex2.eu/vocab/3/LocationReferencing/DirectionEnum> ;
  rdfs:comment "Direction is unknown."@en ;
  rdfs:label "Direction enum unknown"@en .

<http://datex2.eu/vocab/3/LocationReferencing/DirectionEnum#other>
  a <http://datex2.eu/vocab/3/LocationReferencing/DirectionEnum> ;
  rdfs:comment "Other than as defined in this enumeration."@en ;
  rdfs:label "Direction enum other"@en .

<http://datex2.eu/vocab/3/LocationReferencing/AlertCLocationCode>
  a owl:Class ;
  rdfs:comment "A positive integer number (between 1 and 63 487) which uniquely identifies a pre-defined Alert C location defined within an Alert-C table."@en ;
  rdfs:label "ALERT-C location code"@en ;
  rdfs:subClassOf <http://datex2.eu/vocab/3/Common/NonNegativeInteger> .

<http://datex2.eu/vocab/3/LocationReferencing/GeographicCharacteristicEnum>
  a owl:Class ;
  rdfs:comment "Geographic characteristic enum"@en ;
  rdfs:label "Geographic characteristic enum"@en ;
  rdfs:subClassOf schema:Enumeration .

<http://datex2.eu/vocab/3/LocationReferencing/GeographicCharacteristicEnum#aroundABendInRoad>
  a <http://datex2.eu/vocab/3/LocationReferencing/GeographicCharacteristicEnum> ;
  rdfs:comment "Around a bend in the road."@en ;
  rdfs:label "Geographic characteristic enum around a bend in road"@en .

<http://datex2.eu/vocab/3/LocationReferencing/GeographicCharacteristicEnum#onBorder>
  a <http://datex2.eu/vocab/3/LocationReferencing/GeographicCharacteristicEnum> ;
  rdfs:comment "On border crossing."@en ;
  rdfs:label "Geographic characteristic enum on border"@en .

<http://datex2.eu/vocab/3/LocationReferencing/GeographicCharacteristicEnum#onPass>
  a <http://datex2.eu/vocab/3/LocationReferencing/GeographicCharacteristicEnum> ;
  rdfs:comment "On mountain pass."@en ;
  rdfs:label "Geographic characteristic enum on pass"@en .

<http://datex2.eu/vocab/3/LocationReferencing/GeographicCharacteristicEnum#overCrestOfHill>
  a <http://datex2.eu/vocab/3/LocationReferencing/GeographicCharacteristicEnum> ;
  rdfs:comment "Over the crest of a hill."@en ;
  rdfs:label "Geographic characteristic enum over crest of hill"@en .

<http://datex2.eu/vocab/3/LocationReferencing/CarriagewayEnum>
  a owl:Class ;
  rdfs:comment "Carriageway enum"@en ;
  rdfs:label "Carriageway enum"@en ;
  rdfs:subClassOf schema:Enumeration .

<http://datex2.eu/vocab/3/LocationReferencing/CarriagewayEnum#connectingCarriageway>
  a <http://datex2.eu/vocab/3/LocationReferencing/CarriagewayEnum> ;
  rdfs:comment "On the connecting carriageway."@en ;
  rdfs:label "Carriageway enum connecting carriageway"@en .

<http://datex2.eu/vocab/3/LocationReferencing/CarriagewayEnum#cycleTrack>
  a <http://datex2.eu/vocab/3/LocationReferencing/CarriagewayEnum> ;
  rdfs:comment "Independent road or part of a road designated for cycles, signposted as such. A cycle track is separated from other roads or other parts of the same road by structural means."@en ;
  rdfs:label "Carriageway enum cycle track"@en .

<http://datex2.eu/vocab/3/LocationReferencing/CarriagewayEnum#entrySlipRoad>
  a <http://datex2.eu/vocab/3/LocationReferencing/CarriagewayEnum> ;
  rdfs:comment "On the entry slip road."@en ;
  rdfs:label "Carriageway enum entry slip road"@en .

<http://datex2.eu/vocab/3/LocationReferencing/CarriagewayEnum#exitSlipRoad>
  a <http://datex2.eu/vocab/3/LocationReferencing/CarriagewayEnum> ;
  rdfs:comment "On the exit slip road."@en ;
  rdfs:label "Carriageway enum exit slip road"@en .

<http://datex2.eu/vocab/3/LocationReferencing/CarriagewayEnum#flyover>
  a <http://datex2.eu/vocab/3/LocationReferencing/CarriagewayEnum> ;
  rdfs:comment "On the flyover, i.e. the section of road passing over another."@en ;
  rdfs:label "Carriageway enum flyover"@en .

<http://datex2.eu/vocab/3/LocationReferencing/CarriagewayEnum#footpath>
  a <http://datex2.eu/vocab/3/LocationReferencing/CarriagewayEnum> ;
  rdfs:comment "On the footpath"@en ;
  rdfs:label "Carriageway enum footpath"@en .

<http://datex2.eu/vocab/3/LocationReferencing/CarriagewayEnum#leftHandFeederRoad>
  a <http://datex2.eu/vocab/3/LocationReferencing/CarriagewayEnum> ;
  rdfs:comment "On the left hand feeder road."@en ;
  rdfs:label "Carriageway enum left hand feeder road"@en .

<http://datex2.eu/vocab/3/LocationReferencing/CarriagewayEnum#leftHandParallelCarriageway>
  a <http://datex2.eu/vocab/3/LocationReferencing/CarriagewayEnum> ;
  rdfs:comment "On the left hand parallel carriageway."@en ;
  rdfs:label "Carriageway enum left hand parallel carriageway"@en .

<http://datex2.eu/vocab/3/LocationReferencing/CarriagewayEnum#mainCarriageway>
  a <http://datex2.eu/vocab/3/LocationReferencing/CarriagewayEnum> ;
  rdfs:comment "On the main carriageway."@en ;
  rdfs:label "Carriageway enum main carriageway"@en .

<http://datex2.eu/vocab/3/LocationReferencing/CarriagewayEnum#oppositeCarriageway>
  a <http://datex2.eu/vocab/3/LocationReferencing/CarriagewayEnum> ;
  rdfs:comment "On the opposite carriageway."@en ;
  rdfs:label "Carriageway enum opposite carriageway"@en .

<http://datex2.eu/vocab/3/LocationReferencing/CarriagewayEnum#parallelCarriageway>
  a <http://datex2.eu/vocab/3/LocationReferencing/CarriagewayEnum> ;
  rdfs:comment "On the adjacent external parallel carriageway."@en ;
  rdfs:label "Carriageway enum parallel carriageway"@en .

<http://datex2.eu/vocab/3/LocationReferencing/CarriagewayEnum#rightHandFeederRoad>
  a <http://datex2.eu/vocab/3/LocationReferencing/CarriagewayEnum> ;
  rdfs:comment "On the right hand feeder road."@en ;
  rdfs:label "Carriageway enum right hand feeder road"@en .

<http://datex2.eu/vocab/3/LocationReferencing/CarriagewayEnum#rightHandParallelCarriageway>
  a <http://datex2.eu/vocab/3/LocationReferencing/CarriagewayEnum> ;
  rdfs:comment "On the right hand parallel carriageway."@en ;
  rdfs:label "Carriageway enum right hand parallel carriageway"@en .

<http://datex2.eu/vocab/3/LocationReferencing/CarriagewayEnum#roundabout>
  a <http://datex2.eu/vocab/3/LocationReferencing/CarriagewayEnum> ;
  rdfs:comment "On the roundabout."@en ;
  rdfs:label "Carriageway enum roundabout"@en .

<http://datex2.eu/vocab/3/LocationReferencing/CarriagewayEnum#serviceRoad>
  a <http://datex2.eu/vocab/3/LocationReferencing/CarriagewayEnum> ;
  rdfs:comment "On the adjacent service road."@en ;
  rdfs:label "Carriageway enum service road"@en .

<http://datex2.eu/vocab/3/LocationReferencing/CarriagewayEnum#slipRoads>
  a <http://datex2.eu/vocab/3/LocationReferencing/CarriagewayEnum> ;
  rdfs:comment "On the slip roads."@en ;
  rdfs:label "Carriageway enum slip roads"@en .

<http://datex2.eu/vocab/3/LocationReferencing/CarriagewayEnum#underpass>
  a <http://datex2.eu/vocab/3/LocationReferencing/CarriagewayEnum> ;
  rdfs:comment "On the underpass, i.e. the section of road passing under another."@en ;
  rdfs:label "Carriageway enum underpass"@en .

<http://datex2.eu/vocab/3/LocationReferencing/CarriagewayEnum#unspecifiedCarriageway>
  a <http://datex2.eu/vocab/3/LocationReferencing/CarriagewayEnum> ;
  rdfs:comment "On an unspecified carriageway"@en ;
  rdfs:label "Carriageway enum unspecified carriageway"@en .

<http://datex2.eu/vocab/3/LocationReferencing/OpenlrOrientationEnum>
  a owl:Class ;
  rdfs:comment "Openlr orientation enum"@en ;
  rdfs:label "Openlr orientation enum"@en ;
  rdfs:subClassOf schema:Enumeration .

<http://datex2.eu/vocab/3/LocationReferencing/OpenlrOrientationEnum#noOrientationOrUnknown>
  a <http://datex2.eu/vocab/3/LocationReferencing/OpenlrOrientationEnum> ;
  rdfs:comment "No orientation or unknown"@en ;
  rdfs:label "Openlr orientation enum no orientation or unknown"@en .

<http://datex2.eu/vocab/3/LocationReferencing/OpenlrOrientationEnum#withLineDirection>
  a <http://datex2.eu/vocab/3/LocationReferencing/OpenlrOrientationEnum> ;
  rdfs:comment "With line direction"@en ;
  rdfs:label "Openlr orientation enum with line direction"@en .

<http://datex2.eu/vocab/3/LocationReferencing/OpenlrOrientationEnum#againstLineDirection>
  a <http://datex2.eu/vocab/3/LocationReferencing/OpenlrOrientationEnum> ;
  rdfs:comment "Against line direction"@en ;
  rdfs:label "Openlr orientation enum against line direction"@en .

<http://datex2.eu/vocab/3/LocationReferencing/OpenlrOrientationEnum#both>
  a <http://datex2.eu/vocab/3/LocationReferencing/OpenlrOrientationEnum> ;
  rdfs:comment "Both directions"@en ;
  rdfs:label "Openlr orientation enum both"@en .

<http://datex2.eu/vocab/3/LocationReferencing/LinearDirectionEnum>
  a owl:Class ;
  rdfs:comment "Linear direction enum"@en ;
  rdfs:label "Linear direction enum"@en ;
  rdfs:subClassOf schema:Enumeration .

<http://datex2.eu/vocab/3/LocationReferencing/LinearDirectionEnum#both>
  a <http://datex2.eu/vocab/3/LocationReferencing/LinearDirectionEnum> ;
  rdfs:comment "Indicates that both directions of traffic flow are affected by the situation or relate to the traffic data."@en ;
  rdfs:label "Linear direction enum both"@en .

<http://datex2.eu/vocab/3/LocationReferencing/LinearDirectionEnum#opposite>
  a <http://datex2.eu/vocab/3/LocationReferencing/LinearDirectionEnum> ;
  rdfs:comment "Indicates that the direction of traffic flow affected by the situation or related to the traffic data is in the opposite sense to the direction in which the linear element is defined."@en ;
  rdfs:label "Linear direction enum opposite"@en .

<http://datex2.eu/vocab/3/LocationReferencing/LinearDirectionEnum#aligned>
  a <http://datex2.eu/vocab/3/LocationReferencing/LinearDirectionEnum> ;
  rdfs:comment "Indicates that the direction of traffic flow affected by the situation or related to the traffic data is in the same sense as the direction in which the linear element is defined."@en ;
  rdfs:label "Linear direction enum aligned"@en .

<http://datex2.eu/vocab/3/LocationReferencing/LinearDirectionEnum#unknown>
  a <http://datex2.eu/vocab/3/LocationReferencing/LinearDirectionEnum> ;
  rdfs:comment "Indicates that the direction of traffic flow affected by the situation or related to the traffic data is unknown."@en ;
  rdfs:label "Linear direction enum unknown"@en .

<http://datex2.eu/vocab/3/LocationReferencing/TpegLoc01LinearLocationSubtypeEnum>
  a owl:Class ;
  rdfs:comment "TPEG loc01 linear location subtype enum"@en ;
  rdfs:label "TPEG loc01 linear location subtype enum"@en ;
  rdfs:subClassOf schema:Enumeration .

<http://datex2.eu/vocab/3/LocationReferencing/TpegLoc01LinearLocationSubtypeEnum#segment>
  a <http://datex2.eu/vocab/3/LocationReferencing/TpegLoc01LinearLocationSubtypeEnum> ;
  rdfs:comment "A segment (or link) of the road network corresponding to the way in which the road operator has segmented the network."@en ;
  rdfs:label "TPEG loc01 linear location subtype enum segment"@en .

<http://datex2.eu/vocab/3/LocationReferencing/GmlPosList>
  a owl:Class ;
  rdfs:comment "List of coordinates, space-separated, within the same coordinate reference system, defining a geometric entity. Modelled on DirectPositionListType in GML (EN ISO 19136), but constrained to represent a 2D or 3D polyline."@en ;
  rdfs:label "Gml pos list"@en ;
  rdfs:subClassOf <http://datex2.eu/vocab/3/Common/LongString> .

<http://datex2.eu/vocab/3/LocationReferencing/LaneEnum>
  a owl:Class ;
  rdfs:comment "Lane enum"@en ;
  rdfs:label "Lane enum"@en ;
  rdfs:subClassOf schema:Enumeration .

<http://datex2.eu/vocab/3/LocationReferencing/LaneEnum#allLanesCompleteCarriageway>
  a <http://datex2.eu/vocab/3/LocationReferencing/LaneEnum> ;
  rdfs:comment "In all lanes of the carriageway."@en ;
  rdfs:label "Lane enum all lanes complete carriageway"@en .

<http://datex2.eu/vocab/3/LocationReferencing/LaneEnum#busLane>
  a <http://datex2.eu/vocab/3/LocationReferencing/LaneEnum> ;
  rdfs:comment "In the bus lane."@en ;
  rdfs:label "Lane enum bus lane"@en .

<http://datex2.eu/vocab/3/LocationReferencing/LaneEnum#busStop>
  a <http://datex2.eu/vocab/3/LocationReferencing/LaneEnum> ;
  rdfs:comment "In the bus stop lane."@en ;
  rdfs:label "Lane enum bus stop"@en .

<http://datex2.eu/vocab/3/LocationReferencing/LaneEnum#carPoolLane>
  a <http://datex2.eu/vocab/3/LocationReferencing/LaneEnum> ;
  rdfs:comment "In the carpool lane."@en ;
  rdfs:label "Lane enum car pool lane"@en .

<http://datex2.eu/vocab/3/LocationReferencing/LaneEnum#centralReservation>
  a <http://datex2.eu/vocab/3/LocationReferencing/LaneEnum> ;
  rdfs:comment "On the central reservation separating the two directional carriageways of the highway."@en ;
  rdfs:label "Lane enum central reservation"@en .

<http://datex2.eu/vocab/3/LocationReferencing/LaneEnum#crawlerLane>
  a <http://datex2.eu/vocab/3/LocationReferencing/LaneEnum> ;
  rdfs:comment "In the crawler lane - a lane that should be used by slower vehicles."@en ;
  rdfs:label "Lane enum crawler lane"@en .

<http://datex2.eu/vocab/3/LocationReferencing/LaneEnum#cycleLane>
  a <http://datex2.eu/vocab/3/LocationReferencing/LaneEnum> ;
  rdfs:comment "Part of a carriageway designated for cycles. A cycle lane is distinguished from the rest of the carriageway by longitudinal road markings."@en ;
  rdfs:label "Lane enum cycle lane"@en .

<http://datex2.eu/vocab/3/LocationReferencing/LaneEnum#emergencyLane>
  a <http://datex2.eu/vocab/3/LocationReferencing/LaneEnum> ;
  rdfs:comment "In the emergency lane."@en ;
  rdfs:label "Lane enum emergency lane"@en .

<http://datex2.eu/vocab/3/LocationReferencing/LaneEnum#escapeLane>
  a <http://datex2.eu/vocab/3/LocationReferencing/LaneEnum> ;
  rdfs:comment "In the escape lane."@en ;
  rdfs:label "Lane enum escape lane"@en .

<http://datex2.eu/vocab/3/LocationReferencing/LaneEnum#expressLane>
  a <http://datex2.eu/vocab/3/LocationReferencing/LaneEnum> ;
  rdfs:comment "In the express lane."@en ;
  rdfs:label "Lane enum express lane"@en .

<http://datex2.eu/vocab/3/LocationReferencing/LaneEnum#hardShoulder>
  a <http://datex2.eu/vocab/3/LocationReferencing/LaneEnum> ;
  rdfs:comment "On the hard shoulder."@en ;
  rdfs:label "Lane enum hard shoulder"@en .

<http://datex2.eu/vocab/3/LocationReferencing/LaneEnum#heavyVehicleLane>
  a <http://datex2.eu/vocab/3/LocationReferencing/LaneEnum> ;
  rdfs:comment "In the heavy vehicle lane."@en ;
  rdfs:label "Lane enum heavy vehicle lane"@en .

<http://datex2.eu/vocab/3/LocationReferencing/LaneEnum#layBy>
  a <http://datex2.eu/vocab/3/LocationReferencing/LaneEnum> ;
  rdfs:comment "In a lay-by."@en ;
  rdfs:label "Lane enum lay by"@en .

<http://datex2.eu/vocab/3/LocationReferencing/LaneEnum#leftHandTurningLane>
  a <http://datex2.eu/vocab/3/LocationReferencing/LaneEnum> ;
  rdfs:comment "In the left hand turning lane."@en ;
  rdfs:label "Lane enum left hand turning lane"@en .

<http://datex2.eu/vocab/3/LocationReferencing/LaneEnum#leftLane>
  a <http://datex2.eu/vocab/3/LocationReferencing/LaneEnum> ;
  rdfs:comment "In the left lane."@en ;
  rdfs:label "Lane enum left lane"@en .

<http://datex2.eu/vocab/3/LocationReferencing/LaneEnum#localTrafficLane>
  a <http://datex2.eu/vocab/3/LocationReferencing/LaneEnum> ;
  rdfs:comment "In the local traffic lane."@en ;
  rdfs:label "Lane enum local traffic lane"@en .

<http://datex2.eu/vocab/3/LocationReferencing/LaneEnum#middleLane>
  a <http://datex2.eu/vocab/3/LocationReferencing/LaneEnum> ;
  rdfs:comment "In the middle lane."@en ;
  rdfs:label "Lane enum middle lane"@en .

<http://datex2.eu/vocab/3/LocationReferencing/LaneEnum#overtakingLane>
  a <http://datex2.eu/vocab/3/LocationReferencing/LaneEnum> ;
  rdfs:comment "In the overtaking lane."@en ;
  rdfs:label "Lane enum overtaking lane"@en .

<http://datex2.eu/vocab/3/LocationReferencing/LaneEnum#rightHandTurningLane>
  a <http://datex2.eu/vocab/3/LocationReferencing/LaneEnum> ;
  rdfs:comment "In the right hand turning lane."@en ;
  rdfs:label "Lane enum right hand turning lane"@en .

<http://datex2.eu/vocab/3/LocationReferencing/LaneEnum#rightLane>
  a <http://datex2.eu/vocab/3/LocationReferencing/LaneEnum> ;
  rdfs:comment "In the right lane."@en ;
  rdfs:label "Lane enum right lane"@en .

<http://datex2.eu/vocab/3/LocationReferencing/LaneEnum#rushHourLane>
  a <http://datex2.eu/vocab/3/LocationReferencing/LaneEnum> ;
  rdfs:comment "In the lane dedicated for use during the rush (peak) hour."@en ;
  rdfs:label "Lane enum rush hour lane"@en .

<http://datex2.eu/vocab/3/LocationReferencing/LaneEnum#setDownArea>
  a <http://datex2.eu/vocab/3/LocationReferencing/LaneEnum> ;
  rdfs:comment "In the area/lane reserved for passenger pick-up or set-down."@en ;
  rdfs:label "Lane enum set down area"@en .

<http://datex2.eu/vocab/3/LocationReferencing/LaneEnum#slowVehicleLane>
  a <http://datex2.eu/vocab/3/LocationReferencing/LaneEnum> ;
  rdfs:comment "In a lane dedicated to vehicles that are not permitted to exceed a fixed slow speed."@en ;
  rdfs:label "Lane enum slow vehicle lane"@en .

<http://datex2.eu/vocab/3/LocationReferencing/LaneEnum#throughTrafficLane>
  a <http://datex2.eu/vocab/3/LocationReferencing/LaneEnum> ;
  rdfs:comment "In the through traffic lane."@en ;
  rdfs:label "Lane enum through traffic lane"@en .

<http://datex2.eu/vocab/3/LocationReferencing/LaneEnum#tidalFlowLane>
  a <http://datex2.eu/vocab/3/LocationReferencing/LaneEnum> ;
  rdfs:comment "In the lane dedicated for use as a tidal flow lane."@en ;
  rdfs:label "Lane enum tidal flow lane"@en .

<http://datex2.eu/vocab/3/LocationReferencing/LaneEnum#turningLane>
  a <http://datex2.eu/vocab/3/LocationReferencing/LaneEnum> ;
  rdfs:comment "In the turning lane."@en ;
  rdfs:label "Lane enum turning lane"@en .

<http://datex2.eu/vocab/3/LocationReferencing/LaneEnum#verge>
  a <http://datex2.eu/vocab/3/LocationReferencing/LaneEnum> ;
  rdfs:comment "On the verge."@en ;
  rdfs:label "Lane enum verge"@en .

<http://datex2.eu/vocab/3/LocationReferencing/HeightGradeEnum>
  a owl:Class ;
  rdfs:comment "Height grade enum"@en ;
  rdfs:label "Height grade enum"@en ;
  rdfs:subClassOf schema:Enumeration .

<http://datex2.eu/vocab/3/LocationReferencing/HeightGradeEnum#aboveGrade>
  a <http://datex2.eu/vocab/3/LocationReferencing/HeightGradeEnum> ;
  rdfs:comment "Above or over the normal road grade elevation."@en ;
  rdfs:label "Height grade enum above grade"@en .

<http://datex2.eu/vocab/3/LocationReferencing/HeightGradeEnum#atGrade>
  a <http://datex2.eu/vocab/3/LocationReferencing/HeightGradeEnum> ;
  rdfs:comment "At the normal road grade elevation."@en ;
  rdfs:label "Height grade enum at grade"@en .

<http://datex2.eu/vocab/3/LocationReferencing/HeightGradeEnum#belowGrade>
  a <http://datex2.eu/vocab/3/LocationReferencing/HeightGradeEnum> ;
  rdfs:comment "Below or under the normal road grade elevation."@en ;
  rdfs:label "Height grade enum below grade"@en .

<http://datex2.eu/vocab/3/LocationReferencing/AlertCDirectionEnum>
  a owl:Class ;
  rdfs:comment "ALERT-C direction enum"@en ;
  rdfs:label "ALERT-C direction enum"@en ;
  rdfs:subClassOf schema:Enumeration .

<http://datex2.eu/vocab/3/LocationReferencing/AlertCDirectionEnum#negative>
  a <http://datex2.eu/vocab/3/LocationReferencing/AlertCDirectionEnum> ;
  rdfs:comment "The direction of navigation in an ALERT-C table that corresponds to the negative offset usage to go from the secondary location to the primary location within the ALERT-C location table."@en ;
  rdfs:label "ALERT-C direction enum negative"@en .

<http://datex2.eu/vocab/3/LocationReferencing/AlertCDirectionEnum#positive>
  a <http://datex2.eu/vocab/3/LocationReferencing/AlertCDirectionEnum> ;
  rdfs:comment "The direction of navigation in an ALERT-C table that corresponds to the positive offset usage to go from the secondary location to the primary location within the ALERT-C location table."@en ;
  rdfs:label "ALERT-C direction enum positive"@en .

<http://datex2.eu/vocab/3/LocationReferencing/OpenlrFunctionalRoadClassEnum>
  a owl:Class ;
  rdfs:comment "Openlr functional road class enum"@en ;
  rdfs:label "Openlr functional road class enum"@en ;
  rdfs:subClassOf schema:Enumeration .

<http://datex2.eu/vocab/3/LocationReferencing/OpenlrFunctionalRoadClassEnum#frc0>
  a <http://datex2.eu/vocab/3/LocationReferencing/OpenlrFunctionalRoadClassEnum> ;
  rdfs:comment "Main road, highest importance"@en ;
  rdfs:label "Openlr functional road class enum frc0"@en .

<http://datex2.eu/vocab/3/LocationReferencing/OpenlrFunctionalRoadClassEnum#frc1>
  a <http://datex2.eu/vocab/3/LocationReferencing/OpenlrFunctionalRoadClassEnum> ;
  rdfs:comment "First class road"@en ;
  rdfs:label "Openlr functional road class enum frc1"@en .

<http://datex2.eu/vocab/3/LocationReferencing/OpenlrFunctionalRoadClassEnum#frc2>
  a <http://datex2.eu/vocab/3/LocationReferencing/OpenlrFunctionalRoadClassEnum> ;
  rdfs:comment "Second class road"@en ;
  rdfs:label "Openlr functional road class enum frc2"@en .

<http://datex2.eu/vocab/3/LocationReferencing/OpenlrFunctionalRoadClassEnum#frc3>
  a <http://datex2.eu/vocab/3/LocationReferencing/OpenlrFunctionalRoadClassEnum> ;
  rdfs:comment "Third class road"@en ;
  rdfs:label "Openlr functional road class enum frc3"@en .

<http://datex2.eu/vocab/3/LocationReferencing/OpenlrFunctionalRoadClassEnum#frc4>
  a <http://datex2.eu/vocab/3/LocationReferencing/OpenlrFunctionalRoadClassEnum> ;
  rdfs:comment "Fourth class road"@en ;
  rdfs:label "Openlr functional road class enum frc4"@en .

<http://datex2.eu/vocab/3/LocationReferencing/OpenlrFunctionalRoadClassEnum#frc5>
  a <http://datex2.eu/vocab/3/LocationReferencing/OpenlrFunctionalRoadClassEnum> ;
  rdfs:comment "Fifth class road"@en ;
  rdfs:label "Openlr functional road class enum frc5"@en .

<http://datex2.eu/vocab/3/LocationReferencing/OpenlrFunctionalRoadClassEnum#frc6>
  a <http://datex2.eu/vocab/3/LocationReferencing/OpenlrFunctionalRoadClassEnum> ;
  rdfs:comment "Sixth class road"@en ;
  rdfs:label "Openlr functional road class enum frc6"@en .

<http://datex2.eu/vocab/3/LocationReferencing/OpenlrFunctionalRoadClassEnum#frc7>
  a <http://datex2.eu/vocab/3/LocationReferencing/OpenlrFunctionalRoadClassEnum> ;
  rdfs:comment "Other class road, lowest importance"@en ;
  rdfs:label "Openlr functional road class enum frc7"@en .

<http://datex2.eu/vocab/3/LocationReferencing/TpegLoc01AreaLocationSubtypeEnum>
  a owl:Class ;
  rdfs:comment "TPEG loc01 area location subtype enum"@en ;
  rdfs:label "TPEG loc01 area location subtype enum"@en ;
  rdfs:subClassOf schema:Enumeration .

<http://datex2.eu/vocab/3/LocationReferencing/TpegLoc01AreaLocationSubtypeEnum#largeArea>
  a <http://datex2.eu/vocab/3/LocationReferencing/TpegLoc01AreaLocationSubtypeEnum> ;
  rdfs:comment "A geographic or geometric large area."@en ;
  rdfs:label "TPEG loc01 area location subtype enum large area"@en .

<http://datex2.eu/vocab/3/LocationReferencing/TpegLoc01AreaLocationSubtypeEnum#other>
  a <http://datex2.eu/vocab/3/LocationReferencing/TpegLoc01AreaLocationSubtypeEnum> ;
  rdfs:comment "Other than as defined in this enumeration."@en ;
  rdfs:label "TPEG loc01 area location subtype enum other"@en .

<http://datex2.eu/vocab/3/LocationReferencing/TpegLoc01FramedPointLocationSubtypeEnum>
  a owl:Class ;
  rdfs:comment "TPEG loc01 framed point location subtype enum"@en ;
  rdfs:label "TPEG loc01 framed point location subtype enum"@en ;
  rdfs:subClassOf schema:Enumeration .

<http://datex2.eu/vocab/3/LocationReferencing/TpegLoc01FramedPointLocationSubtypeEnum#framedPoint>
  a <http://datex2.eu/vocab/3/LocationReferencing/TpegLoc01FramedPointLocationSubtypeEnum> ;
  rdfs:comment "A point on the road network framed by two other points on the same road."@en ;
  rdfs:label "TPEG loc01 framed point location subtype enum framed point"@en .

<http://datex2.eu/vocab/3/LocationReferencing/ReferentTypeEnum>
  a owl:Class ;
  rdfs:comment "Referent type enum"@en ;
  rdfs:label "Referent type enum"@en ;
  rdfs:subClassOf schema:Enumeration .

<http://datex2.eu/vocab/3/LocationReferencing/ReferentTypeEnum#boundary>
  a <http://datex2.eu/vocab/3/LocationReferencing/ReferentTypeEnum> ;
  rdfs:comment "A boundary between two jurisdictional or administrative areas. These may be legal boundaries such as between counties or countries, maintenance responsibility boundaries or control boundaries. "@en ;
  rdfs:label "Referent type enum boundary"@en .

<http://datex2.eu/vocab/3/LocationReferencing/ReferentTypeEnum#intersection>
  a <http://datex2.eu/vocab/3/LocationReferencing/ReferentTypeEnum> ;
  rdfs:comment "A crossing of two or more roads where the precise point of intersection is defined according to specific business rules."@en ;
  rdfs:label "Referent type enum intersection"@en .

<http://datex2.eu/vocab/3/LocationReferencing/ReferentTypeEnum#referenceMarker>
  a <http://datex2.eu/vocab/3/LocationReferencing/ReferentTypeEnum> ;
  rdfs:comment "A marker which is usually but not necessarily physical that is one of a sequence which are spaced out along the linear object (road) to provide a location reference. The spacing of markers is not necessarily even."@en ;
  rdfs:label "Referent type enum reference marker"@en .

<http://datex2.eu/vocab/3/LocationReferencing/ReferentTypeEnum#landmark>
  a <http://datex2.eu/vocab/3/LocationReferencing/ReferentTypeEnum> ;
  rdfs:comment "A visible identifiable physical landmark either alongside or close to the linear object."@en ;
  rdfs:label "Referent type enum landmark"@en .

<http://datex2.eu/vocab/3/LocationReferencing/ReferentTypeEnum#roadNode>
  a <http://datex2.eu/vocab/3/LocationReferencing/ReferentTypeEnum> ;
  rdfs:comment "A topological node defined on a road network. Such nodes may delineate the segmentation of the road network according to defined business rules or may constitute a purely topological representation of a road network."@en ;
  rdfs:label "Referent type enum road node"@en .

<http://datex2.eu/vocab/3/LocationReferencing/AltitudeAccuracyEnum>
  a owl:Class ;
  rdfs:comment "Altitude accuracy enum"@en ;
  rdfs:label "Altitude accuracy enum"@en ;
  rdfs:subClassOf schema:Enumeration .

<http://datex2.eu/vocab/3/LocationReferencing/AltitudeAccuracyEnum#equalToOrLessThan1Centimetre>
  a <http://datex2.eu/vocab/3/LocationReferencing/AltitudeAccuracyEnum> ;
  rdfs:comment "Indicates if the altitude accuracy is equal to or less than 1 centimetre"@en ;
  rdfs:label "Altitude accuracy enum equal to or less than1 centimetre"@en .

<http://datex2.eu/vocab/3/LocationReferencing/AltitudeAccuracyEnum#equalToOrLessThan2Centimetres>
  a <http://datex2.eu/vocab/3/LocationReferencing/AltitudeAccuracyEnum> ;
  rdfs:comment "Indicates if the altitude accuracy is equal to or less than 2 centimetres"@en ;
  rdfs:label "Altitude accuracy enum equal to or less than2 centimetres"@en .

<http://datex2.eu/vocab/3/LocationReferencing/AltitudeAccuracyEnum#equalToOrLessThan5Centimetres>
  a <http://datex2.eu/vocab/3/LocationReferencing/AltitudeAccuracyEnum> ;
  rdfs:comment "Indicates if the altitude accuracy is equal to or less than 5 centimetres"@en ;
  rdfs:label "Altitude accuracy enum equal to or less than5 centimetres"@en .

<http://datex2.eu/vocab/3/LocationReferencing/AltitudeAccuracyEnum#equalToOrLessThan10Centimetres>
  a <http://datex2.eu/vocab/3/LocationReferencing/AltitudeAccuracyEnum> ;
  rdfs:comment "Indicates if the altitude accuracy is equal to or less than 10 centimetres"@en ;
  rdfs:label "Altitude accuracy enum equal to or less than10 centimetres"@en .

<http://datex2.eu/vocab/3/LocationReferencing/AltitudeAccuracyEnum#equalToOrLessThan20Centimetres>
  a <http://datex2.eu/vocab/3/LocationReferencing/AltitudeAccuracyEnum> ;
  rdfs:comment "Indicates if the altitude accuracy is equal to or less than 20 centimetres"@en ;
  rdfs:label "Altitude accuracy enum equal to or less than20 centimetres"@en .

<http://datex2.eu/vocab/3/LocationReferencing/AltitudeAccuracyEnum#equalToOrLessThan50Centimetres>
  a <http://datex2.eu/vocab/3/LocationReferencing/AltitudeAccuracyEnum> ;
  rdfs:comment "Indicates if the altitude accuracy is equal to or less than 50 centimetres"@en ;
  rdfs:label "Altitude accuracy enum equal to or less than50 centimetres"@en .

<http://datex2.eu/vocab/3/LocationReferencing/AltitudeAccuracyEnum#equalToOrLessThan1Metre>
  a <http://datex2.eu/vocab/3/LocationReferencing/AltitudeAccuracyEnum> ;
  rdfs:comment "Indicates if the altitude accuracy is equal to or less than 1 metre"@en ;
  rdfs:label "Altitude accuracy enum equal to or less than1 metre"@en .

<http://datex2.eu/vocab/3/LocationReferencing/AltitudeAccuracyEnum#equalToOrLessThan2Metres>
  a <http://datex2.eu/vocab/3/LocationReferencing/AltitudeAccuracyEnum> ;
  rdfs:comment "Indicates if the altitude accuracy is equal to or less than 2 metres"@en ;
  rdfs:label "Altitude accuracy enum equal to or less than2 metres"@en .

<http://datex2.eu/vocab/3/LocationReferencing/AltitudeAccuracyEnum#equalToOrLessThan5Metres>
  a <http://datex2.eu/vocab/3/LocationReferencing/AltitudeAccuracyEnum> ;
  rdfs:comment "Indicates if the altitude accuracy is equal to or less than 5 metres"@en ;
  rdfs:label "Altitude accuracy enum equal to or less than5 metres"@en .

<http://datex2.eu/vocab/3/LocationReferencing/AltitudeAccuracyEnum#equalToOrLessThan10Metres>
  a <http://datex2.eu/vocab/3/LocationReferencing/AltitudeAccuracyEnum> ;
  rdfs:comment "Indicates if the altitude accuracy is equal to or less than 10 metres"@en ;
  rdfs:label "Altitude accuracy enum equal to or less than10 metres"@en .

<http://datex2.eu/vocab/3/LocationReferencing/AltitudeAccuracyEnum#equalToOrLessThan20Metres>
  a <http://datex2.eu/vocab/3/LocationReferencing/AltitudeAccuracyEnum> ;
  rdfs:comment "Indicates if the altitude accuracy is equal to or less than 20 metres"@en ;
  rdfs:label "Altitude accuracy enum equal to or less than20 metres"@en .

<http://datex2.eu/vocab/3/LocationReferencing/AltitudeAccuracyEnum#equalToOrLessThan50Metres>
  a <http://datex2.eu/vocab/3/LocationReferencing/AltitudeAccuracyEnum> ;
  rdfs:comment "Indicates if the altitude accuracy is equal to or less than 50 metres"@en ;
  rdfs:label "Altitude accuracy enum equal to or less than50 metres"@en .

<http://datex2.eu/vocab/3/LocationReferencing/AltitudeAccuracyEnum#equalToOrLessThan100Metres>
  a <http://datex2.eu/vocab/3/LocationReferencing/AltitudeAccuracyEnum> ;
  rdfs:comment "Indicates if the altitude accuracy is equal to or less than 100 metres"@en ;
  rdfs:label "Altitude accuracy enum equal to or less than100 metres"@en .

<http://datex2.eu/vocab/3/LocationReferencing/AltitudeAccuracyEnum#equalToOrLessThan200Metres>
  a <http://datex2.eu/vocab/3/LocationReferencing/AltitudeAccuracyEnum> ;
  rdfs:comment "Indicates if the altitude accuracy is equal to or less than 200 metres"@en ;
  rdfs:label "Altitude accuracy enum equal to or less than200 metres"@en .

<http://datex2.eu/vocab/3/LocationReferencing/DirectionPurposeEnum>
  a owl:Class ;
  rdfs:comment "Direction purpose enum"@en ;
  rdfs:label "Direction purpose enum"@en ;
  rdfs:subClassOf schema:Enumeration .

<http://datex2.eu/vocab/3/LocationReferencing/DirectionPurposeEnum#inbound>
  a <http://datex2.eu/vocab/3/LocationReferencing/DirectionPurposeEnum> ;
  rdfs:comment "On the carriageway or lane which is inbound towards the centre of the town or city."@en ;
  rdfs:label "Direction purpose enum inbound"@en .

<http://datex2.eu/vocab/3/LocationReferencing/DirectionPurposeEnum#outbound>
  a <http://datex2.eu/vocab/3/LocationReferencing/DirectionPurposeEnum> ;
  rdfs:comment "On the carriageway or lane which is outbound from the centre of the town or city."@en ;
  rdfs:label "Direction purpose enum outbound"@en .

<http://datex2.eu/vocab/3/LocationReferencing/TpegLoc03OtherPointDescriptorSubtypeEnum>
  a owl:Class ;
  rdfs:comment "TPEG loc03 other point descriptor subtype enum"@en ;
  rdfs:label "TPEG loc03 other point descriptor subtype enum"@en ;
  rdfs:subClassOf schema:Enumeration .

<http://datex2.eu/vocab/3/LocationReferencing/TpegLoc03OtherPointDescriptorSubtypeEnum#administrativeAreaName>
  a <http://datex2.eu/vocab/3/LocationReferencing/TpegLoc03OtherPointDescriptorSubtypeEnum> ;
  rdfs:comment "Name of an administrative area."@en ;
  rdfs:label "TPEG loc03 other point descriptor subtype enum administrative area name"@en .

<http://datex2.eu/vocab/3/LocationReferencing/TpegLoc03OtherPointDescriptorSubtypeEnum#administrativeReferenceName>
  a <http://datex2.eu/vocab/3/LocationReferencing/TpegLoc03OtherPointDescriptorSubtypeEnum> ;
  rdfs:comment "Reference name by which an administrative area is known."@en ;
  rdfs:label "TPEG loc03 other point descriptor subtype enum administrative reference name"@en .

<http://datex2.eu/vocab/3/LocationReferencing/TpegLoc03OtherPointDescriptorSubtypeEnum#airportName>
  a <http://datex2.eu/vocab/3/LocationReferencing/TpegLoc03OtherPointDescriptorSubtypeEnum> ;
  rdfs:comment "Name of an airport."@en ;
  rdfs:label "TPEG loc03 other point descriptor subtype enum airport name"@en .

<http://datex2.eu/vocab/3/LocationReferencing/TpegLoc03OtherPointDescriptorSubtypeEnum#areaName>
  a <http://datex2.eu/vocab/3/LocationReferencing/TpegLoc03OtherPointDescriptorSubtypeEnum> ;
  rdfs:comment "Name of an area."@en ;
  rdfs:label "TPEG loc03 other point descriptor subtype enum area name"@en .

<http://datex2.eu/vocab/3/LocationReferencing/TpegLoc03OtherPointDescriptorSubtypeEnum#buildingName>
  a <http://datex2.eu/vocab/3/LocationReferencing/TpegLoc03OtherPointDescriptorSubtypeEnum> ;
  rdfs:comment "Name of a building."@en ;
  rdfs:label "TPEG loc03 other point descriptor subtype enum building name"@en .

<http://datex2.eu/vocab/3/LocationReferencing/TpegLoc03OtherPointDescriptorSubtypeEnum#busStopIdentifier>
  a <http://datex2.eu/vocab/3/LocationReferencing/TpegLoc03OtherPointDescriptorSubtypeEnum> ;
  rdfs:comment "Identifier of a bus stop on the road network."@en ;
  rdfs:label "TPEG loc03 other point descriptor subtype enum bus stop identifier"@en .

<http://datex2.eu/vocab/3/LocationReferencing/TpegLoc03OtherPointDescriptorSubtypeEnum#busStopName>
  a <http://datex2.eu/vocab/3/LocationReferencing/TpegLoc03OtherPointDescriptorSubtypeEnum> ;
  rdfs:comment "Name of a bus stop on the road network."@en ;
  rdfs:label "TPEG loc03 other point descriptor subtype enum bus stop name"@en .

<http://datex2.eu/vocab/3/LocationReferencing/TpegLoc03OtherPointDescriptorSubtypeEnum#canalName>
  a <http://datex2.eu/vocab/3/LocationReferencing/TpegLoc03OtherPointDescriptorSubtypeEnum> ;
  rdfs:comment "Name of a canal."@en ;
  rdfs:label "TPEG loc03 other point descriptor subtype enum canal name"@en .

<http://datex2.eu/vocab/3/LocationReferencing/TpegLoc03OtherPointDescriptorSubtypeEnum#countyName>
  a <http://datex2.eu/vocab/3/LocationReferencing/TpegLoc03OtherPointDescriptorSubtypeEnum> ;
  rdfs:comment "Name of a county (administrative sub-division)."@en ;
  rdfs:label "TPEG loc03 other point descriptor subtype enum county name"@en .

<http://datex2.eu/vocab/3/LocationReferencing/TpegLoc03OtherPointDescriptorSubtypeEnum#ferryPortName>
  a <http://datex2.eu/vocab/3/LocationReferencing/TpegLoc03OtherPointDescriptorSubtypeEnum> ;
  rdfs:comment "Name of a ferry port."@en ;
  rdfs:label "TPEG loc03 other point descriptor subtype enum ferry port name"@en .

<http://datex2.eu/vocab/3/LocationReferencing/TpegLoc03OtherPointDescriptorSubtypeEnum#intersectionName>
  a <http://datex2.eu/vocab/3/LocationReferencing/TpegLoc03OtherPointDescriptorSubtypeEnum> ;
  rdfs:comment "Name of a road network intersection."@en ;
  rdfs:label "TPEG loc03 other point descriptor subtype enum intersection name"@en .

<http://datex2.eu/vocab/3/LocationReferencing/TpegLoc03OtherPointDescriptorSubtypeEnum#lakeName>
  a <http://datex2.eu/vocab/3/LocationReferencing/TpegLoc03OtherPointDescriptorSubtypeEnum> ;
  rdfs:comment "Name of a lake."@en ;
  rdfs:label "TPEG loc03 other point descriptor subtype enum lake name"@en .

<http://datex2.eu/vocab/3/LocationReferencing/TpegLoc03OtherPointDescriptorSubtypeEnum#linkName>
  a <http://datex2.eu/vocab/3/LocationReferencing/TpegLoc03OtherPointDescriptorSubtypeEnum> ;
  rdfs:comment "Name of a road link."@en ;
  rdfs:label "TPEG loc03 other point descriptor subtype enum link name"@en .

<http://datex2.eu/vocab/3/LocationReferencing/TpegLoc03OtherPointDescriptorSubtypeEnum#localLinkName>
  a <http://datex2.eu/vocab/3/LocationReferencing/TpegLoc03OtherPointDescriptorSubtypeEnum> ;
  rdfs:comment "Local name of a road link."@en ;
  rdfs:label "TPEG loc03 other point descriptor subtype enum local link name"@en .

<http://datex2.eu/vocab/3/LocationReferencing/TpegLoc03OtherPointDescriptorSubtypeEnum#metroStationName>
  a <http://datex2.eu/vocab/3/LocationReferencing/TpegLoc03OtherPointDescriptorSubtypeEnum> ;
  rdfs:comment "Name of a metro/underground station."@en ;
  rdfs:label "TPEG loc03 other point descriptor subtype enum metro station name"@en .

<http://datex2.eu/vocab/3/LocationReferencing/TpegLoc03OtherPointDescriptorSubtypeEnum#nationName>
  a <http://datex2.eu/vocab/3/LocationReferencing/TpegLoc03OtherPointDescriptorSubtypeEnum> ;
  rdfs:comment "Name of a nation (e.g. Wales) which is a sub-division of a ISO recognised country."@en ;
  rdfs:label "TPEG loc03 other point descriptor subtype enum nation name"@en .

<http://datex2.eu/vocab/3/LocationReferencing/TpegLoc03OtherPointDescriptorSubtypeEnum#nonLinkedPointName>
  a <http://datex2.eu/vocab/3/LocationReferencing/TpegLoc03OtherPointDescriptorSubtypeEnum> ;
  rdfs:comment "Name of a point on the road network which is not at a junction or intersection. "@en ;
  rdfs:label "TPEG loc03 other point descriptor subtype enum non linked point name"@en .

<http://datex2.eu/vocab/3/LocationReferencing/TpegLoc03OtherPointDescriptorSubtypeEnum#parkingFacilityName>
  a <http://datex2.eu/vocab/3/LocationReferencing/TpegLoc03OtherPointDescriptorSubtypeEnum> ;
  rdfs:comment "Name of a parking facility."@en ;
  rdfs:label "TPEG loc03 other point descriptor subtype enum parking facility name"@en .

<http://datex2.eu/vocab/3/LocationReferencing/TpegLoc03OtherPointDescriptorSubtypeEnum#pointName>
  a <http://datex2.eu/vocab/3/LocationReferencing/TpegLoc03OtherPointDescriptorSubtypeEnum> ;
  rdfs:comment "Name of a specific point."@en ;
  rdfs:label "TPEG loc03 other point descriptor subtype enum point name"@en .

<http://datex2.eu/vocab/3/LocationReferencing/TpegLoc03OtherPointDescriptorSubtypeEnum#pointOfInterestName>
  a <http://datex2.eu/vocab/3/LocationReferencing/TpegLoc03OtherPointDescriptorSubtypeEnum> ;
  rdfs:comment "Name of a general point of interest."@en ;
  rdfs:label "TPEG loc03 other point descriptor subtype enum point of interest name"@en .

<http://datex2.eu/vocab/3/LocationReferencing/TpegLoc03OtherPointDescriptorSubtypeEnum#railwayStation>
  a <http://datex2.eu/vocab/3/LocationReferencing/TpegLoc03OtherPointDescriptorSubtypeEnum> ;
  rdfs:comment "Name of a railway station."@en ;
  rdfs:label "TPEG loc03 other point descriptor subtype enum railway station"@en .

<http://datex2.eu/vocab/3/LocationReferencing/TpegLoc03OtherPointDescriptorSubtypeEnum#regionName>
  a <http://datex2.eu/vocab/3/LocationReferencing/TpegLoc03OtherPointDescriptorSubtypeEnum> ;
  rdfs:comment "Name of a geographic region."@en ;
  rdfs:label "TPEG loc03 other point descriptor subtype enum region name"@en .

<http://datex2.eu/vocab/3/LocationReferencing/TpegLoc03OtherPointDescriptorSubtypeEnum#riverName>
  a <http://datex2.eu/vocab/3/LocationReferencing/TpegLoc03OtherPointDescriptorSubtypeEnum> ;
  rdfs:comment "Name of a river."@en ;
  rdfs:label "TPEG loc03 other point descriptor subtype enum river name"@en .

<http://datex2.eu/vocab/3/LocationReferencing/TpegLoc03OtherPointDescriptorSubtypeEnum#seaName>
  a <http://datex2.eu/vocab/3/LocationReferencing/TpegLoc03OtherPointDescriptorSubtypeEnum> ;
  rdfs:comment "Name of a sea."@en ;
  rdfs:label "TPEG loc03 other point descriptor subtype enum sea name"@en .

<http://datex2.eu/vocab/3/LocationReferencing/TpegLoc03OtherPointDescriptorSubtypeEnum#serviceAreaName>
  a <http://datex2.eu/vocab/3/LocationReferencing/TpegLoc03OtherPointDescriptorSubtypeEnum> ;
  rdfs:comment "Name of a service area on a road network."@en ;
  rdfs:label "TPEG loc03 other point descriptor subtype enum service area name"@en .

<http://datex2.eu/vocab/3/LocationReferencing/TpegLoc03OtherPointDescriptorSubtypeEnum#tidalRiverName>
  a <http://datex2.eu/vocab/3/LocationReferencing/TpegLoc03OtherPointDescriptorSubtypeEnum> ;
  rdfs:comment "Name of a river which is of a tidal nature."@en ;
  rdfs:label "TPEG loc03 other point descriptor subtype enum tidal river name"@en .

<http://datex2.eu/vocab/3/LocationReferencing/TpegLoc03OtherPointDescriptorSubtypeEnum#townName>
  a <http://datex2.eu/vocab/3/LocationReferencing/TpegLoc03OtherPointDescriptorSubtypeEnum> ;
  rdfs:comment "Name of a town."@en ;
  rdfs:label "TPEG loc03 other point descriptor subtype enum town name"@en .

<http://datex2.eu/vocab/3/LocationReferencing/TpegLoc03OtherPointDescriptorSubtypeEnum#other>
  a <http://datex2.eu/vocab/3/LocationReferencing/TpegLoc03OtherPointDescriptorSubtypeEnum> ;
  rdfs:comment "Other than as defined in this enumeration."@en ;
  rdfs:label "TPEG loc03 other point descriptor subtype enum other"@en .

<http://datex2.eu/vocab/3/LocationReferencing/TpegLoc01SimplePointLocationSubtypeEnum>
  a owl:Class ;
  rdfs:comment "TPEG loc01 simple point location subtype enum"@en ;
  rdfs:label "TPEG loc01 simple point location subtype enum"@en ;
  rdfs:subClassOf schema:Enumeration .

<http://datex2.eu/vocab/3/LocationReferencing/TpegLoc01SimplePointLocationSubtypeEnum#intersection>
  a <http://datex2.eu/vocab/3/LocationReferencing/TpegLoc01SimplePointLocationSubtypeEnum> ;
  rdfs:comment "An point on the road network at which one or more roads intersect."@en ;
  rdfs:label "TPEG loc01 simple point location subtype enum intersection"@en .

<http://datex2.eu/vocab/3/LocationReferencing/TpegLoc01SimplePointLocationSubtypeEnum#nonLinkedPoint>
  a <http://datex2.eu/vocab/3/LocationReferencing/TpegLoc01SimplePointLocationSubtypeEnum> ;
  rdfs:comment "A point on the road network which is not at a junction or intersection."@en ;
  rdfs:label "TPEG loc01 simple point location subtype enum non linked point"@en .

<http://datex2.eu/vocab/3/LocationReferencing/TpegLoc04HeightTypeEnum>
  a owl:Class ;
  rdfs:comment "TPEG loc04 height type enum"@en ;
  rdfs:label "TPEG loc04 height type enum"@en ;
  rdfs:subClassOf schema:Enumeration .

<http://datex2.eu/vocab/3/LocationReferencing/TpegLoc04HeightTypeEnum#above>
  a <http://datex2.eu/vocab/3/LocationReferencing/TpegLoc04HeightTypeEnum> ;
  rdfs:comment "Height above specified location."@en ;
  rdfs:label "TPEG loc04 height type enum above"@en .

<http://datex2.eu/vocab/3/LocationReferencing/TpegLoc04HeightTypeEnum#aboveSeaLevel>
  a <http://datex2.eu/vocab/3/LocationReferencing/TpegLoc04HeightTypeEnum> ;
  rdfs:comment "Height above mean sea high water level."@en ;
  rdfs:label "TPEG loc04 height type enum above sea level"@en .

<http://datex2.eu/vocab/3/LocationReferencing/TpegLoc04HeightTypeEnum#aboveStreetLevel>
  a <http://datex2.eu/vocab/3/LocationReferencing/TpegLoc04HeightTypeEnum> ;
  rdfs:comment "Height above street level."@en ;
  rdfs:label "TPEG loc04 height type enum above street level"@en .

<http://datex2.eu/vocab/3/LocationReferencing/TpegLoc04HeightTypeEnum#at>
  a <http://datex2.eu/vocab/3/LocationReferencing/TpegLoc04HeightTypeEnum> ;
  rdfs:comment "At height of specified location."@en ;
  rdfs:label "TPEG loc04 height type enum at"@en .

<http://datex2.eu/vocab/3/LocationReferencing/TpegLoc04HeightTypeEnum#atSeaLevel>
  a <http://datex2.eu/vocab/3/LocationReferencing/TpegLoc04HeightTypeEnum> ;
  rdfs:comment "At mean sea high water level."@en ;
  rdfs:label "TPEG loc04 height type enum at sea level"@en .

<http://datex2.eu/vocab/3/LocationReferencing/TpegLoc04HeightTypeEnum#atStreetLevel>
  a <http://datex2.eu/vocab/3/LocationReferencing/TpegLoc04HeightTypeEnum> ;
  rdfs:comment "At street level."@en ;
  rdfs:label "TPEG loc04 height type enum at street level"@en .

<http://datex2.eu/vocab/3/LocationReferencing/TpegLoc04HeightTypeEnum#below>
  a <http://datex2.eu/vocab/3/LocationReferencing/TpegLoc04HeightTypeEnum> ;
  rdfs:comment "Height below specified location."@en ;
  rdfs:label "TPEG loc04 height type enum below"@en .

<http://datex2.eu/vocab/3/LocationReferencing/TpegLoc04HeightTypeEnum#belowSeaLevel>
  a <http://datex2.eu/vocab/3/LocationReferencing/TpegLoc04HeightTypeEnum> ;
  rdfs:comment "Height below mean sea high water level."@en ;
  rdfs:label "TPEG loc04 height type enum below sea level"@en .

<http://datex2.eu/vocab/3/LocationReferencing/TpegLoc04HeightTypeEnum#belowStreetLevel>
  a <http://datex2.eu/vocab/3/LocationReferencing/TpegLoc04HeightTypeEnum> ;
  rdfs:comment "Height below street level."@en ;
  rdfs:label "TPEG loc04 height type enum below street level"@en .

<http://datex2.eu/vocab/3/LocationReferencing/TpegLoc04HeightTypeEnum#undefined>
  a <http://datex2.eu/vocab/3/LocationReferencing/TpegLoc04HeightTypeEnum> ;
  rdfs:comment "Undefined height reference."@en ;
  rdfs:label "TPEG loc04 height type enum undefined"@en .

<http://datex2.eu/vocab/3/LocationReferencing/TpegLoc04HeightTypeEnum#unknown>
  a <http://datex2.eu/vocab/3/LocationReferencing/TpegLoc04HeightTypeEnum> ;
  rdfs:comment "Unknown height reference."@en ;
  rdfs:label "TPEG loc04 height type enum unknown"@en .

<http://datex2.eu/vocab/3/LocationReferencing/TpegLoc04HeightTypeEnum#other>
  a <http://datex2.eu/vocab/3/LocationReferencing/TpegLoc04HeightTypeEnum> ;
  rdfs:comment "Other than as defined in this enumeration."@en ;
  rdfs:label "TPEG loc04 height type enum other"@en .

<http://datex2.eu/vocab/3/LocationReferencing/HeightTypeEnum>
  a owl:Class ;
  rdfs:comment "Height type enum"@en ;
  rdfs:label "Height type enum"@en ;
  rdfs:subClassOf schema:Enumeration .

<http://datex2.eu/vocab/3/LocationReferencing/HeightTypeEnum#ellipsoidalHeight>
  a <http://datex2.eu/vocab/3/LocationReferencing/HeightTypeEnum> ;
  rdfs:comment "Value measured vertically above the reference ellipsoid"@en ;
  rdfs:label "Height type enum ellipsoidal height"@en .

<http://datex2.eu/vocab/3/LocationReferencing/HeightTypeEnum#gravityRelatedHeight>
  a <http://datex2.eu/vocab/3/LocationReferencing/HeightTypeEnum> ;
  rdfs:comment "Height type corresponding a value measured along direction of gravity above the reference geoid i.e. equipotential surface of the Earth's gravity field which globally approximates mean sea level."@en ;
  rdfs:label "Height type enum gravity related height"@en .

<http://datex2.eu/vocab/3/LocationReferencing/HeightTypeEnum#relativeHeight>
  a <http://datex2.eu/vocab/3/LocationReferencing/HeightTypeEnum> ;
  rdfs:comment "Height type corresponding to value masured vertically above the ground level at this point."@en ;
  rdfs:label "Height type enum relative height"@en .

<http://datex2.eu/vocab/3/LocationReferencing/SubdivisionCode>
  a owl:Class ;
  rdfs:comment "The second part of an ISO 3166-2 country sub-division code (up to 3 characters) which may be used along with a CountryCode to make a full ISO 3166-2 subdivision code."@en ;
  rdfs:label "Subdivision code"@en ;
  rdfs:subClassOf <http://datex2.eu/vocab/3/Common/String> .

<http://datex2.eu/vocab/3/LocationReferencing/AreaPlacesEnum>
  a owl:Class ;
  rdfs:comment "Area places enum"@en ;
  rdfs:label "Area places enum"@en ;
  rdfs:subClassOf schema:Enumeration .

<http://datex2.eu/vocab/3/LocationReferencing/AreaPlacesEnum#atBorders>
  a <http://datex2.eu/vocab/3/LocationReferencing/AreaPlacesEnum> ;
  rdfs:comment "At national borders"@en ;
  rdfs:label "Area places enum at borders"@en .

<http://datex2.eu/vocab/3/LocationReferencing/AreaPlacesEnum#atHighAltitudes>
  a <http://datex2.eu/vocab/3/LocationReferencing/AreaPlacesEnum> ;
  rdfs:comment "At high altitudes"@en ;
  rdfs:label "Area places enum at high altitudes"@en .

<http://datex2.eu/vocab/3/LocationReferencing/AreaPlacesEnum#inBuiltUpAreas>
  a <http://datex2.eu/vocab/3/LocationReferencing/AreaPlacesEnum> ;
  rdfs:comment "In built up areas, i.e. villages, towns and cities"@en ;
  rdfs:label "Area places enum in built up areas"@en .

<http://datex2.eu/vocab/3/LocationReferencing/AreaPlacesEnum#inForestedAreas>
  a <http://datex2.eu/vocab/3/LocationReferencing/AreaPlacesEnum> ;
  rdfs:comment "On sections of the road where it runs through or adjacent to forested areas"@en ;
  rdfs:label "Area places enum in forested areas"@en .

<http://datex2.eu/vocab/3/LocationReferencing/AreaPlacesEnum#inGalleries>
  a <http://datex2.eu/vocab/3/LocationReferencing/AreaPlacesEnum> ;
  rdfs:comment "In galleries"@en ;
  rdfs:label "Area places enum in galleries"@en .

<http://datex2.eu/vocab/3/LocationReferencing/AreaPlacesEnum#inLowLyingAreas>
  a <http://datex2.eu/vocab/3/LocationReferencing/AreaPlacesEnum> ;
  rdfs:comment "In low-lying areas"@en ;
  rdfs:label "Area places enum in low lying areas"@en .

<http://datex2.eu/vocab/3/LocationReferencing/AreaPlacesEnum#inRuralAreas>
  a <http://datex2.eu/vocab/3/LocationReferencing/AreaPlacesEnum> ;
  rdfs:comment "In rural areas, i.e. outside villages, towns and cities"@en ;
  rdfs:label "Area places enum in rural areas"@en .

<http://datex2.eu/vocab/3/LocationReferencing/AreaPlacesEnum#inShadedAreas>
  a <http://datex2.eu/vocab/3/LocationReferencing/AreaPlacesEnum> ;
  rdfs:comment "In shaded areas"@en ;
  rdfs:label "Area places enum in shaded areas"@en .

<http://datex2.eu/vocab/3/LocationReferencing/AreaPlacesEnum#inTheInnerCityAreas>
  a <http://datex2.eu/vocab/3/LocationReferencing/AreaPlacesEnum> ;
  rdfs:comment "In the city centre areas"@en ;
  rdfs:label "Area places enum in the inner city areas"@en .

<http://datex2.eu/vocab/3/LocationReferencing/AreaPlacesEnum#inTunnels>
  a <http://datex2.eu/vocab/3/LocationReferencing/AreaPlacesEnum> ;
  rdfs:comment "In tunnels"@en ;
  rdfs:label "Area places enum in tunnels"@en .

<http://datex2.eu/vocab/3/LocationReferencing/AreaPlacesEnum#onBridges>
  a <http://datex2.eu/vocab/3/LocationReferencing/AreaPlacesEnum> ;
  rdfs:comment "On bridges"@en ;
  rdfs:label "Area places enum on bridges"@en .

<http://datex2.eu/vocab/3/LocationReferencing/AreaPlacesEnum#onDownhillSections>
  a <http://datex2.eu/vocab/3/LocationReferencing/AreaPlacesEnum> ;
  rdfs:comment "On downhill sections of the road"@en ;
  rdfs:label "Area places enum on downhill sections"@en .

<http://datex2.eu/vocab/3/LocationReferencing/AreaPlacesEnum#onElevatedSections>
  a <http://datex2.eu/vocab/3/LocationReferencing/AreaPlacesEnum> ;
  rdfs:comment "On elevated sections of the road"@en ;
  rdfs:label "Area places enum on elevated sections"@en .

<http://datex2.eu/vocab/3/LocationReferencing/AreaPlacesEnum#onEnteringOrLeavingTunnels>
  a <http://datex2.eu/vocab/3/LocationReferencing/AreaPlacesEnum> ;
  rdfs:comment "On entering or leaving tunnels"@en ;
  rdfs:label "Area places enum on entering or leaving tunnels"@en .

<http://datex2.eu/vocab/3/LocationReferencing/AreaPlacesEnum#onFlyovers>
  a <http://datex2.eu/vocab/3/LocationReferencing/AreaPlacesEnum> ;
  rdfs:comment "On flyover sections of the road, i.e. sections of the road which pass over another road"@en ;
  rdfs:label "Area places enum on flyovers"@en .

<http://datex2.eu/vocab/3/LocationReferencing/AreaPlacesEnum#onPasses>
  a <http://datex2.eu/vocab/3/LocationReferencing/AreaPlacesEnum> ;
  rdfs:comment "On mountain passes"@en ;
  rdfs:label "Area places enum on passes"@en .

<http://datex2.eu/vocab/3/LocationReferencing/AreaPlacesEnum#onUndergroundSections>
  a <http://datex2.eu/vocab/3/LocationReferencing/AreaPlacesEnum> ;
  rdfs:comment "On underground sections of the road"@en ;
  rdfs:label "Area places enum on underground sections"@en .

<http://datex2.eu/vocab/3/LocationReferencing/AreaPlacesEnum#onUnderpasses>
  a <http://datex2.eu/vocab/3/LocationReferencing/AreaPlacesEnum> ;
  rdfs:comment "On underpasses, i.e. sections of the road which pass under another road"@en ;
  rdfs:label "Area places enum on underpasses"@en .

<http://datex2.eu/vocab/3/LocationReferencing/OpenlrSideOfRoadEnum>
  a owl:Class ;
  rdfs:comment "Openlr side of road enum"@en ;
  rdfs:label "Openlr side of road enum"@en ;
  rdfs:subClassOf schema:Enumeration .

<http://datex2.eu/vocab/3/LocationReferencing/OpenlrSideOfRoadEnum#onRoadOrUnknown>
  a <http://datex2.eu/vocab/3/LocationReferencing/OpenlrSideOfRoadEnum> ;
  rdfs:comment "On road or unknown"@en ;
  rdfs:label "Openlr side of road enum on road or unknown"@en .

<http://datex2.eu/vocab/3/LocationReferencing/OpenlrSideOfRoadEnum#right>
  a <http://datex2.eu/vocab/3/LocationReferencing/OpenlrSideOfRoadEnum> ;
  rdfs:comment "On the right side of the road."@en ;
  rdfs:label "Openlr side of road enum right"@en .

<http://datex2.eu/vocab/3/LocationReferencing/OpenlrSideOfRoadEnum#left>
  a <http://datex2.eu/vocab/3/LocationReferencing/OpenlrSideOfRoadEnum> ;
  rdfs:comment "On the left side of the road."@en ;
  rdfs:label "Openlr side of road enum left"@en .

<http://datex2.eu/vocab/3/LocationReferencing/OpenlrSideOfRoadEnum#both>
  a <http://datex2.eu/vocab/3/LocationReferencing/OpenlrSideOfRoadEnum> ;
  rdfs:comment "On both sides of the road."@en ;
  rdfs:label "Openlr side of road enum both"@en .

<http://datex2.eu/vocab/3/LocationReferencing/RelativePositionOnCarriagewayEnum>
  a owl:Class ;
  rdfs:comment "Relative position on carriageway enum"@en ;
  rdfs:label "Relative position on carriageway enum"@en ;
  rdfs:subClassOf schema:Enumeration .

<http://datex2.eu/vocab/3/LocationReferencing/RelativePositionOnCarriagewayEnum#inTheCentre>
  a <http://datex2.eu/vocab/3/LocationReferencing/RelativePositionOnCarriagewayEnum> ;
  rdfs:comment "In the centre of the roadway."@en ;
  rdfs:label "Relative position on carriageway enum in the centre"@en .

<http://datex2.eu/vocab/3/LocationReferencing/RelativePositionOnCarriagewayEnum#onTheLeft>
  a <http://datex2.eu/vocab/3/LocationReferencing/RelativePositionOnCarriagewayEnum> ;
  rdfs:comment "On the left of the roadway."@en ;
  rdfs:label "Relative position on carriageway enum on the left"@en .

<http://datex2.eu/vocab/3/LocationReferencing/RelativePositionOnCarriagewayEnum#onTheRight>
  a <http://datex2.eu/vocab/3/LocationReferencing/RelativePositionOnCarriagewayEnum> ;
  rdfs:comment "On the right of the roadway."@en ;
  rdfs:label "Relative position on carriageway enum on the right"@en .

<http://datex2.eu/vocab/3/LocationReferencing/NutsCode>
  a owl:Class ;
  rdfs:comment "A NUTS code (Nomenclature of territorial units for statistics)."@en ;
  rdfs:label "Nuts code"@en ;
  rdfs:subClassOf <http://datex2.eu/vocab/3/Common/String> .

<http://datex2.eu/vocab/3/LocationReferencing/SubdivisionTypeEnum>
  a owl:Class ;
  rdfs:comment "Subdivision type enum"@en ;
  rdfs:label "Subdivision type enum"@en ;
  rdfs:subClassOf schema:Enumeration .

<http://datex2.eu/vocab/3/LocationReferencing/SubdivisionTypeEnum#administrativeAtoll>
  a <http://datex2.eu/vocab/3/LocationReferencing/SubdivisionTypeEnum> ;
  rdfs:comment "Administrative atoll"@en ;
  rdfs:label "Subdivision type enum administrative atoll"@en .

<http://datex2.eu/vocab/3/LocationReferencing/SubdivisionTypeEnum#administrativeRegion>
  a <http://datex2.eu/vocab/3/LocationReferencing/SubdivisionTypeEnum> ;
  rdfs:comment "Administrative region"@en ;
  rdfs:label "Subdivision type enum administrative region"@en .

<http://datex2.eu/vocab/3/LocationReferencing/SubdivisionTypeEnum#administrativeTerritory>
  a <http://datex2.eu/vocab/3/LocationReferencing/SubdivisionTypeEnum> ;
  rdfs:comment "Administrative territory"@en ;
  rdfs:label "Subdivision type enum administrative territory"@en .

<http://datex2.eu/vocab/3/LocationReferencing/SubdivisionTypeEnum#arcticRegion>
  a <http://datex2.eu/vocab/3/LocationReferencing/SubdivisionTypeEnum> ;
  rdfs:comment "Arctic region"@en ;
  rdfs:label "Subdivision type enum arctic region"@en .

<http://datex2.eu/vocab/3/LocationReferencing/SubdivisionTypeEnum#autonomousCity>
  a <http://datex2.eu/vocab/3/LocationReferencing/SubdivisionTypeEnum> ;
  rdfs:comment "Autonomous city"@en ;
  rdfs:label "Subdivision type enum autonomous city"@en .

<http://datex2.eu/vocab/3/LocationReferencing/SubdivisionTypeEnum#autonomousCityInNorthAfrica>
  a <http://datex2.eu/vocab/3/LocationReferencing/SubdivisionTypeEnum> ;
  rdfs:comment "Autonomous city in North Africa"@en ;
  rdfs:label "Subdivision type enum autonomous city in north africa"@en .

<http://datex2.eu/vocab/3/LocationReferencing/SubdivisionTypeEnum#autonomousCommunity>
  a <http://datex2.eu/vocab/3/LocationReferencing/SubdivisionTypeEnum> ;
  rdfs:comment "Autonomous community"@en ;
  rdfs:label "Subdivision type enum autonomous community"@en .

<http://datex2.eu/vocab/3/LocationReferencing/SubdivisionTypeEnum#autonomousDistrict>
  a <http://datex2.eu/vocab/3/LocationReferencing/SubdivisionTypeEnum> ;
  rdfs:comment "Autonomous district"@en ;
  rdfs:label "Subdivision type enum autonomous district"@en .

<http://datex2.eu/vocab/3/LocationReferencing/SubdivisionTypeEnum#autonomousProvince>
  a <http://datex2.eu/vocab/3/LocationReferencing/SubdivisionTypeEnum> ;
  rdfs:comment "Autonomous province"@en ;
  rdfs:label "Subdivision type enum autonomous province"@en .

<http://datex2.eu/vocab/3/LocationReferencing/SubdivisionTypeEnum#autonomousRegion>
  a <http://datex2.eu/vocab/3/LocationReferencing/SubdivisionTypeEnum> ;
  rdfs:comment "Autonomous region"@en ;
  rdfs:label "Subdivision type enum autonomous region"@en .

<http://datex2.eu/vocab/3/LocationReferencing/SubdivisionTypeEnum#canton>
  a <http://datex2.eu/vocab/3/LocationReferencing/SubdivisionTypeEnum> ;
  rdfs:comment "Canton"@en ;
  rdfs:label "Subdivision type enum canton"@en .

<http://datex2.eu/vocab/3/LocationReferencing/SubdivisionTypeEnum#capitalCity>
  a <http://datex2.eu/vocab/3/LocationReferencing/SubdivisionTypeEnum> ;
  rdfs:comment "Capital city"@en ;
  rdfs:label "Subdivision type enum capital city"@en .

<http://datex2.eu/vocab/3/LocationReferencing/SubdivisionTypeEnum#city>
  a <http://datex2.eu/vocab/3/LocationReferencing/SubdivisionTypeEnum> ;
  rdfs:comment "City"@en ;
  rdfs:label "Subdivision type enum city"@en .

<http://datex2.eu/vocab/3/LocationReferencing/SubdivisionTypeEnum#cityMunicipality>
  a <http://datex2.eu/vocab/3/LocationReferencing/SubdivisionTypeEnum> ;
  rdfs:comment "City municipality"@en ;
  rdfs:label "Subdivision type enum city municipality"@en .

<http://datex2.eu/vocab/3/LocationReferencing/SubdivisionTypeEnum#cityOfCountyRight>
  a <http://datex2.eu/vocab/3/LocationReferencing/SubdivisionTypeEnum> ;
  rdfs:comment "City of county right"@en ;
  rdfs:label "Subdivision type enum city of county right"@en .

<http://datex2.eu/vocab/3/LocationReferencing/SubdivisionTypeEnum#commune>
  a <http://datex2.eu/vocab/3/LocationReferencing/SubdivisionTypeEnum> ;
  rdfs:comment "Commune"@en ;
  rdfs:label "Subdivision type enum commune"@en .

<http://datex2.eu/vocab/3/LocationReferencing/SubdivisionTypeEnum#councilArea>
  a <http://datex2.eu/vocab/3/LocationReferencing/SubdivisionTypeEnum> ;
  rdfs:comment "Council area"@en ;
  rdfs:label "Subdivision type enum council area"@en .

<http://datex2.eu/vocab/3/LocationReferencing/SubdivisionTypeEnum#county>
  a <http://datex2.eu/vocab/3/LocationReferencing/SubdivisionTypeEnum> ;
  rdfs:comment "County"@en ;
  rdfs:label "Subdivision type enum county"@en .

<http://datex2.eu/vocab/3/LocationReferencing/SubdivisionTypeEnum#country>
  a <http://datex2.eu/vocab/3/LocationReferencing/SubdivisionTypeEnum> ;
  rdfs:comment "Country"@en ;
  rdfs:label "Subdivision type enum country"@en .

<http://datex2.eu/vocab/3/LocationReferencing/SubdivisionTypeEnum#department>
  a <http://datex2.eu/vocab/3/LocationReferencing/SubdivisionTypeEnum> ;
  rdfs:comment "Department"@en ;
  rdfs:label "Subdivision type enum department"@en .

<http://datex2.eu/vocab/3/LocationReferencing/SubdivisionTypeEnum#dependency>
  a <http://datex2.eu/vocab/3/LocationReferencing/SubdivisionTypeEnum> ;
  rdfs:comment "Dependency"@en ;
  rdfs:label "Subdivision type enum dependency"@en .

<http://datex2.eu/vocab/3/LocationReferencing/SubdivisionTypeEnum#district>
  a <http://datex2.eu/vocab/3/LocationReferencing/SubdivisionTypeEnum> ;
  rdfs:comment "District"@en ;
  rdfs:label "Subdivision type enum district"@en .

<http://datex2.eu/vocab/3/LocationReferencing/SubdivisionTypeEnum#districtMunicipality>
  a <http://datex2.eu/vocab/3/LocationReferencing/SubdivisionTypeEnum> ;
  rdfs:comment "District municipality"@en ;
  rdfs:label "Subdivision type enum district municipality"@en .

<http://datex2.eu/vocab/3/LocationReferencing/SubdivisionTypeEnum#districtWithSpecialStatus>
  a <http://datex2.eu/vocab/3/LocationReferencing/SubdivisionTypeEnum> ;
  rdfs:comment "District with special status"@en ;
  rdfs:label "Subdivision type enum district with special status"@en .

<http://datex2.eu/vocab/3/LocationReferencing/SubdivisionTypeEnum#entity>
  a <http://datex2.eu/vocab/3/LocationReferencing/SubdivisionTypeEnum> ;
  rdfs:comment "Entity"@en ;
  rdfs:label "Subdivision type enum entity"@en .

<http://datex2.eu/vocab/3/LocationReferencing/SubdivisionTypeEnum#geographicalEntity>
  a <http://datex2.eu/vocab/3/LocationReferencing/SubdivisionTypeEnum> ;
  rdfs:comment "Geographical entity"@en ;
  rdfs:label "Subdivision type enum geographical entity"@en .

<http://datex2.eu/vocab/3/LocationReferencing/SubdivisionTypeEnum#governorate>
  a <http://datex2.eu/vocab/3/LocationReferencing/SubdivisionTypeEnum> ;
  rdfs:comment "Governorate"@en ;
  rdfs:label "Subdivision type enum governorate"@en .

<http://datex2.eu/vocab/3/LocationReferencing/SubdivisionTypeEnum#laender>
  a <http://datex2.eu/vocab/3/LocationReferencing/SubdivisionTypeEnum> ;
  rdfs:comment "Länder"@en ;
  rdfs:label "Subdivision type enum laender"@en .

<http://datex2.eu/vocab/3/LocationReferencing/SubdivisionTypeEnum#localCouncil>
  a <http://datex2.eu/vocab/3/LocationReferencing/SubdivisionTypeEnum> ;
  rdfs:comment "Local Council"@en ;
  rdfs:label "Subdivision type enum local council"@en .

<http://datex2.eu/vocab/3/LocationReferencing/SubdivisionTypeEnum#londonBorough>
  a <http://datex2.eu/vocab/3/LocationReferencing/SubdivisionTypeEnum> ;
  rdfs:comment "London borough"@en ;
  rdfs:label "Subdivision type enum london borough"@en .

<http://datex2.eu/vocab/3/LocationReferencing/SubdivisionTypeEnum#metropolitanArea>
  a <http://datex2.eu/vocab/3/LocationReferencing/SubdivisionTypeEnum> ;
  rdfs:comment "Metropolitan area"@en ;
  rdfs:label "Subdivision type enum metropolitan area"@en .

<http://datex2.eu/vocab/3/LocationReferencing/SubdivisionTypeEnum#metropolitanDepartment>
  a <http://datex2.eu/vocab/3/LocationReferencing/SubdivisionTypeEnum> ;
  rdfs:comment "Metropolitan department"@en ;
  rdfs:label "Subdivision type enum metropolitan department"@en .

<http://datex2.eu/vocab/3/LocationReferencing/SubdivisionTypeEnum#metropolitanDistrict>
  a <http://datex2.eu/vocab/3/LocationReferencing/SubdivisionTypeEnum> ;
  rdfs:comment "Metropolitan district"@en ;
  rdfs:label "Subdivision type enum metropolitan district"@en .

<http://datex2.eu/vocab/3/LocationReferencing/SubdivisionTypeEnum#metropolitanRegion>
  a <http://datex2.eu/vocab/3/LocationReferencing/SubdivisionTypeEnum> ;
  rdfs:comment "Metropolitan region"@en ;
  rdfs:label "Subdivision type enum metropolitan region"@en .

<http://datex2.eu/vocab/3/LocationReferencing/SubdivisionTypeEnum#municipality>
  a <http://datex2.eu/vocab/3/LocationReferencing/SubdivisionTypeEnum> ;
  rdfs:comment "Municipality"@en ;
  rdfs:label "Subdivision type enum municipality"@en .

<http://datex2.eu/vocab/3/LocationReferencing/SubdivisionTypeEnum#overseasDepartment>
  a <http://datex2.eu/vocab/3/LocationReferencing/SubdivisionTypeEnum> ;
  rdfs:comment "Overseas department"@en ;
  rdfs:label "Subdivision type enum overseas department"@en .

<http://datex2.eu/vocab/3/LocationReferencing/SubdivisionTypeEnum#overseasRegion>
  a <http://datex2.eu/vocab/3/LocationReferencing/SubdivisionTypeEnum> ;
  rdfs:comment "Overseas region"@en ;
  rdfs:label "Subdivision type enum overseas region"@en .

<http://datex2.eu/vocab/3/LocationReferencing/SubdivisionTypeEnum#overseasTerritorialCollectivity>
  a <http://datex2.eu/vocab/3/LocationReferencing/SubdivisionTypeEnum> ;
  rdfs:comment "Overseas territorial collectivity"@en ;
  rdfs:label "Subdivision type enum overseas territorial collectivity"@en .

<http://datex2.eu/vocab/3/LocationReferencing/SubdivisionTypeEnum#parish>
  a <http://datex2.eu/vocab/3/LocationReferencing/SubdivisionTypeEnum> ;
  rdfs:comment "Parish"@en ;
  rdfs:label "Subdivision type enum parish"@en .

<http://datex2.eu/vocab/3/LocationReferencing/SubdivisionTypeEnum#province>
  a <http://datex2.eu/vocab/3/LocationReferencing/SubdivisionTypeEnum> ;
  rdfs:comment "Province"@en ;
  rdfs:label "Subdivision type enum province"@en .

<http://datex2.eu/vocab/3/LocationReferencing/SubdivisionTypeEnum#quarter>
  a <http://datex2.eu/vocab/3/LocationReferencing/SubdivisionTypeEnum> ;
  rdfs:comment "Quarter"@en ;
  rdfs:label "Subdivision type enum quarter"@en .

<http://datex2.eu/vocab/3/LocationReferencing/SubdivisionTypeEnum#region>
  a <http://datex2.eu/vocab/3/LocationReferencing/SubdivisionTypeEnum> ;
  rdfs:comment "Region"@en ;
  rdfs:label "Subdivision type enum region"@en .

<http://datex2.eu/vocab/3/LocationReferencing/SubdivisionTypeEnum#republic>
  a <http://datex2.eu/vocab/3/LocationReferencing/SubdivisionTypeEnum> ;
  rdfs:comment "Republic"@en ;
  rdfs:label "Subdivision type enum republic"@en .

<http://datex2.eu/vocab/3/LocationReferencing/SubdivisionTypeEnum#republicanCity>
  a <http://datex2.eu/vocab/3/LocationReferencing/SubdivisionTypeEnum> ;
  rdfs:comment "Republic city"@en ;
  rdfs:label "Subdivision type enum republican city"@en .

<http://datex2.eu/vocab/3/LocationReferencing/SubdivisionTypeEnum#selfGovernedPart>
  a <http://datex2.eu/vocab/3/LocationReferencing/SubdivisionTypeEnum> ;
  rdfs:comment "Self-governed part"@en ;
  rdfs:label "Subdivision type enum self governed part"@en .

<http://datex2.eu/vocab/3/LocationReferencing/SubdivisionTypeEnum#specialMunicipality>
  a <http://datex2.eu/vocab/3/LocationReferencing/SubdivisionTypeEnum> ;
  rdfs:comment "Special Municipality"@en ;
  rdfs:label "Subdivision type enum special municipality"@en .

<http://datex2.eu/vocab/3/LocationReferencing/SubdivisionTypeEnum#state>
  a <http://datex2.eu/vocab/3/LocationReferencing/SubdivisionTypeEnum> ;
  rdfs:comment "State"@en ;
  rdfs:label "Subdivision type enum state"@en .

<http://datex2.eu/vocab/3/LocationReferencing/SubdivisionTypeEnum#territorialUnit>
  a <http://datex2.eu/vocab/3/LocationReferencing/SubdivisionTypeEnum> ;
  rdfs:comment "Territorial unit"@en ;
  rdfs:label "Subdivision type enum territorial unit"@en .

<http://datex2.eu/vocab/3/LocationReferencing/SubdivisionTypeEnum#territory>
  a <http://datex2.eu/vocab/3/LocationReferencing/SubdivisionTypeEnum> ;
  rdfs:comment "Territory"@en ;
  rdfs:label "Subdivision type enum territory"@en .

<http://datex2.eu/vocab/3/LocationReferencing/SubdivisionTypeEnum#twoTierCounty>
  a <http://datex2.eu/vocab/3/LocationReferencing/SubdivisionTypeEnum> ;
  rdfs:comment "Two tier country"@en ;
  rdfs:label "Subdivision type enum two tier county"@en .

<http://datex2.eu/vocab/3/LocationReferencing/SubdivisionTypeEnum#unitaryAuthority>
  a <http://datex2.eu/vocab/3/LocationReferencing/SubdivisionTypeEnum> ;
  rdfs:comment "Unitary Authority"@en ;
  rdfs:label "Subdivision type enum unitary authority"@en .

<http://datex2.eu/vocab/3/LocationReferencing/SubdivisionTypeEnum#ward>
  a <http://datex2.eu/vocab/3/LocationReferencing/SubdivisionTypeEnum> ;
  rdfs:comment "Ward"@en ;
  rdfs:label "Subdivision type enum ward"@en .

<http://datex2.eu/vocab/3/LocationReferencing/SubdivisionTypeEnum#other>
  a <http://datex2.eu/vocab/3/LocationReferencing/SubdivisionTypeEnum> ;
  rdfs:comment "Other"@en ;
  rdfs:label "Subdivision type enum other"@en .

<http://datex2.eu/vocab/3/LocationReferencing/NamedAreaTypeEnum>
  a owl:Class ;
  rdfs:comment "Named area type enum"@en ;
  rdfs:label "Named area type enum"@en ;
  rdfs:subClassOf schema:Enumeration .

<http://datex2.eu/vocab/3/LocationReferencing/NamedAreaTypeEnum#applicationRegion>
  a <http://datex2.eu/vocab/3/LocationReferencing/NamedAreaTypeEnum> ;
  rdfs:comment "Application region"@en ;
  rdfs:label "Named area type enum application region"@en .

<http://datex2.eu/vocab/3/LocationReferencing/NamedAreaTypeEnum#continent>
  a <http://datex2.eu/vocab/3/LocationReferencing/NamedAreaTypeEnum> ;
  rdfs:comment "Continent"@en ;
  rdfs:label "Named area type enum continent"@en .

<http://datex2.eu/vocab/3/LocationReferencing/NamedAreaTypeEnum#country>
  a <http://datex2.eu/vocab/3/LocationReferencing/NamedAreaTypeEnum> ;
  rdfs:comment "Country"@en ;
  rdfs:label "Named area type enum country"@en .

<http://datex2.eu/vocab/3/LocationReferencing/NamedAreaTypeEnum#countryGroup>
  a <http://datex2.eu/vocab/3/LocationReferencing/NamedAreaTypeEnum> ;
  rdfs:comment "Group of countries."@en ;
  rdfs:label "Named area type enum country group"@en .

<http://datex2.eu/vocab/3/LocationReferencing/NamedAreaTypeEnum#carParkArea>
  a <http://datex2.eu/vocab/3/LocationReferencing/NamedAreaTypeEnum> ;
  rdfs:comment "Car park area"@en ;
  rdfs:label "Named area type enum car park area"@en .

<http://datex2.eu/vocab/3/LocationReferencing/NamedAreaTypeEnum#carpoolArea>
  a <http://datex2.eu/vocab/3/LocationReferencing/NamedAreaTypeEnum> ;
  rdfs:comment "Carpool area"@en ;
  rdfs:label "Named area type enum carpool area"@en .

<http://datex2.eu/vocab/3/LocationReferencing/NamedAreaTypeEnum#fuzzyArea>
  a <http://datex2.eu/vocab/3/LocationReferencing/NamedAreaTypeEnum> ;
  rdfs:comment "Fuzzy area"@en ;
  rdfs:label "Named area type enum fuzzy area"@en .

<http://datex2.eu/vocab/3/LocationReferencing/NamedAreaTypeEnum#industrialArea>
  a <http://datex2.eu/vocab/3/LocationReferencing/NamedAreaTypeEnum> ;
  rdfs:comment "Industrial area"@en ;
  rdfs:label "Named area type enum industrial area"@en .

<http://datex2.eu/vocab/3/LocationReferencing/NamedAreaTypeEnum#lake>
  a <http://datex2.eu/vocab/3/LocationReferencing/NamedAreaTypeEnum> ;
  rdfs:comment "Lake"@en ;
  rdfs:label "Named area type enum lake"@en .

<http://datex2.eu/vocab/3/LocationReferencing/NamedAreaTypeEnum#meteorologicalArea>
  a <http://datex2.eu/vocab/3/LocationReferencing/NamedAreaTypeEnum> ;
  rdfs:comment "Meteorological area"@en ;
  rdfs:label "Named area type enum meteorological area"@en .

<http://datex2.eu/vocab/3/LocationReferencing/NamedAreaTypeEnum#metropolitanArea>
  a <http://datex2.eu/vocab/3/LocationReferencing/NamedAreaTypeEnum> ;
  rdfs:comment "Metropolitan area"@en ;
  rdfs:label "Named area type enum metropolitan area"@en .

<http://datex2.eu/vocab/3/LocationReferencing/NamedAreaTypeEnum#municipality>
  a <http://datex2.eu/vocab/3/LocationReferencing/NamedAreaTypeEnum> ;
  rdfs:comment "Municipality"@en ;
  rdfs:label "Named area type enum municipality"@en .

<http://datex2.eu/vocab/3/LocationReferencing/NamedAreaTypeEnum#parkAndRideSite>
  a <http://datex2.eu/vocab/3/LocationReferencing/NamedAreaTypeEnum> ;
  rdfs:comment "A park and ride site"@en ;
  rdfs:label "Named area type enum park and ride site"@en .

<http://datex2.eu/vocab/3/LocationReferencing/NamedAreaTypeEnum#ruralCounty>
  a <http://datex2.eu/vocab/3/LocationReferencing/NamedAreaTypeEnum> ;
  rdfs:comment "Rural county"@en ;
  rdfs:label "Named area type enum rural county"@en .

<http://datex2.eu/vocab/3/LocationReferencing/NamedAreaTypeEnum#sea>
  a <http://datex2.eu/vocab/3/LocationReferencing/NamedAreaTypeEnum> ;
  rdfs:comment "Sea"@en ;
  rdfs:label "Named area type enum sea"@en .

<http://datex2.eu/vocab/3/LocationReferencing/NamedAreaTypeEnum#touristArea>
  a <http://datex2.eu/vocab/3/LocationReferencing/NamedAreaTypeEnum> ;
  rdfs:comment "Tourist area"@en ;
  rdfs:label "Named area type enum tourist area"@en .

<http://datex2.eu/vocab/3/LocationReferencing/NamedAreaTypeEnum#trafficArea>
  a <http://datex2.eu/vocab/3/LocationReferencing/NamedAreaTypeEnum> ;
  rdfs:comment "Traffic area"@en ;
  rdfs:label "Named area type enum traffic area"@en .

<http://datex2.eu/vocab/3/LocationReferencing/NamedAreaTypeEnum#urbanCounty>
  a <http://datex2.eu/vocab/3/LocationReferencing/NamedAreaTypeEnum> ;
  rdfs:comment "Urban county"@en ;
  rdfs:label "Named area type enum urban county"@en .

<http://datex2.eu/vocab/3/LocationReferencing/NamedAreaTypeEnum#order1AdministrativeArea>
  a <http://datex2.eu/vocab/3/LocationReferencing/NamedAreaTypeEnum> ;
  rdfs:comment "Order 1 administrative area"@en ;
  rdfs:label "Named area type enum order1 administrative area"@en .

<http://datex2.eu/vocab/3/LocationReferencing/NamedAreaTypeEnum#order2AdministrativeArea>
  a <http://datex2.eu/vocab/3/LocationReferencing/NamedAreaTypeEnum> ;
  rdfs:comment "Order 2 administrative area"@en ;
  rdfs:label "Named area type enum order2 administrative area"@en .

<http://datex2.eu/vocab/3/LocationReferencing/NamedAreaTypeEnum#order3AdministrativeArea>
  a <http://datex2.eu/vocab/3/LocationReferencing/NamedAreaTypeEnum> ;
  rdfs:comment "Order 3 administrative area"@en ;
  rdfs:label "Named area type enum order3 administrative area"@en .

<http://datex2.eu/vocab/3/LocationReferencing/NamedAreaTypeEnum#order4AdministrativeArea>
  a <http://datex2.eu/vocab/3/LocationReferencing/NamedAreaTypeEnum> ;
  rdfs:comment "Order 4 administrative area"@en ;
  rdfs:label "Named area type enum order4 administrative area"@en .

<http://datex2.eu/vocab/3/LocationReferencing/NamedAreaTypeEnum#order5AdministrativeArea>
  a <http://datex2.eu/vocab/3/LocationReferencing/NamedAreaTypeEnum> ;
  rdfs:comment "Order 5 administrative area"@en ;
  rdfs:label "Named area type enum order5 administrative area"@en .

<http://datex2.eu/vocab/3/LocationReferencing/NamedAreaTypeEnum#policeForceControlArea>
  a <http://datex2.eu/vocab/3/LocationReferencing/NamedAreaTypeEnum> ;
  rdfs:comment "Police force control area"@en ;
  rdfs:label "Named area type enum police force control area"@en .

<http://datex2.eu/vocab/3/LocationReferencing/NamedAreaTypeEnum#roadOperatorControlArea>
  a <http://datex2.eu/vocab/3/LocationReferencing/NamedAreaTypeEnum> ;
  rdfs:comment "Road operator control area"@en ;
  rdfs:label "Named area type enum road operator control area"@en .

<http://datex2.eu/vocab/3/LocationReferencing/NamedAreaTypeEnum#waterArea>
  a <http://datex2.eu/vocab/3/LocationReferencing/NamedAreaTypeEnum> ;
  rdfs:comment "Water area"@en ;
  rdfs:label "Named area type enum water area"@en .

<http://datex2.eu/vocab/3/LocationReferencing/OpenlrFormOfWayEnum>
  a owl:Class ;
  rdfs:comment "Openlr form of way enum"@en ;
  rdfs:label "Openlr form of way enum"@en ;
  rdfs:subClassOf schema:Enumeration .

<http://datex2.eu/vocab/3/LocationReferencing/OpenlrFormOfWayEnum#undefined>
  a <http://datex2.eu/vocab/3/LocationReferencing/OpenlrFormOfWayEnum> ;
  rdfs:comment "Undefined"@en ;
  rdfs:label "Openlr form of way enum undefined"@en .

<http://datex2.eu/vocab/3/LocationReferencing/OpenlrFormOfWayEnum#motorway>
  a <http://datex2.eu/vocab/3/LocationReferencing/OpenlrFormOfWayEnum> ;
  rdfs:comment "Motorway"@en ;
  rdfs:label "Openlr form of way enum motorway"@en .

<http://datex2.eu/vocab/3/LocationReferencing/OpenlrFormOfWayEnum#multipleCarriageway>
  a <http://datex2.eu/vocab/3/LocationReferencing/OpenlrFormOfWayEnum> ;
  rdfs:comment "Multiple carriageway"@en ;
  rdfs:label "Openlr form of way enum multiple carriageway"@en .

<http://datex2.eu/vocab/3/LocationReferencing/OpenlrFormOfWayEnum#singleCarriageway>
  a <http://datex2.eu/vocab/3/LocationReferencing/OpenlrFormOfWayEnum> ;
  rdfs:comment "Single carriageway"@en ;
  rdfs:label "Openlr form of way enum single carriageway"@en .

<http://datex2.eu/vocab/3/LocationReferencing/OpenlrFormOfWayEnum#roundabout>
  a <http://datex2.eu/vocab/3/LocationReferencing/OpenlrFormOfWayEnum> ;
  rdfs:comment "Roundabout"@en ;
  rdfs:label "Openlr form of way enum roundabout"@en .

<http://datex2.eu/vocab/3/LocationReferencing/OpenlrFormOfWayEnum#slipRoad>
  a <http://datex2.eu/vocab/3/LocationReferencing/OpenlrFormOfWayEnum> ;
  rdfs:comment "Slip road"@en ;
  rdfs:label "Openlr form of way enum slip road"@en .

<http://datex2.eu/vocab/3/LocationReferencing/OpenlrFormOfWayEnum#trafficSquare>
  a <http://datex2.eu/vocab/3/LocationReferencing/OpenlrFormOfWayEnum> ;
  rdfs:comment "Traffic square"@en ;
  rdfs:label "Openlr form of way enum traffic square"@en .

<http://datex2.eu/vocab/3/LocationReferencing/OpenlrFormOfWayEnum#other>
  a <http://datex2.eu/vocab/3/LocationReferencing/OpenlrFormOfWayEnum> ;
  rdfs:comment "Other"@en ;
  rdfs:label "Openlr form of way enum other"@en .

<http://datex2.eu/vocab/3/LocationReferencing/NutsCodeTypeEnum>
  a owl:Class ;
  rdfs:comment "Nuts code type enum"@en ;
  rdfs:label "Nuts code type enum"@en ;
  rdfs:subClassOf schema:Enumeration .

<http://datex2.eu/vocab/3/LocationReferencing/NutsCodeTypeEnum#nuts1Code>
  a <http://datex2.eu/vocab/3/LocationReferencing/NutsCodeTypeEnum> ;
  rdfs:comment "NUTS 1 code"@en ;
  rdfs:label "Nuts code type enum nuts1 code"@en .

<http://datex2.eu/vocab/3/LocationReferencing/NutsCodeTypeEnum#nuts2Code>
  a <http://datex2.eu/vocab/3/LocationReferencing/NutsCodeTypeEnum> ;
  rdfs:comment "NUTS 2 code"@en ;
  rdfs:label "Nuts code type enum nuts2 code"@en .

<http://datex2.eu/vocab/3/LocationReferencing/NutsCodeTypeEnum#nuts3Code>
  a <http://datex2.eu/vocab/3/LocationReferencing/NutsCodeTypeEnum> ;
  rdfs:comment "NUTS 3 code"@en ;
  rdfs:label "Nuts code type enum nuts3 code"@en .

<http://datex2.eu/vocab/3/LocationReferencing/NutsCodeTypeEnum#lau1Code>
  a <http://datex2.eu/vocab/3/LocationReferencing/NutsCodeTypeEnum> ;
  rdfs:comment "LAU 1 code"@en ;
  rdfs:label "Nuts code type enum lau1 code"@en .

<http://datex2.eu/vocab/3/LocationReferencing/NutsCodeTypeEnum#lau2Code>
  a <http://datex2.eu/vocab/3/LocationReferencing/NutsCodeTypeEnum> ;
  rdfs:comment "LAU 2 code"@en ;
  rdfs:label "Nuts code type enum lau2 code"@en .

<http://datex2.eu/vocab/3/LocationReferencing/InfrastructureDescriptorEnum>
  a owl:Class ;
  rdfs:comment "Infrastructure descriptor enum"@en ;
  rdfs:label "Infrastructure descriptor enum"@en ;
  rdfs:subClassOf schema:Enumeration .

<http://datex2.eu/vocab/3/LocationReferencing/InfrastructureDescriptorEnum#atMotorwayInterchange>
  a <http://datex2.eu/vocab/3/LocationReferencing/InfrastructureDescriptorEnum> ;
  rdfs:comment "At a motorway interchange."@en ;
  rdfs:label "Infrastructure descriptor enum at motorway interchange"@en .

<http://datex2.eu/vocab/3/LocationReferencing/InfrastructureDescriptorEnum#atRestArea>
  a <http://datex2.eu/vocab/3/LocationReferencing/InfrastructureDescriptorEnum> ;
  rdfs:comment "At rest area off the carriageway."@en ;
  rdfs:label "Infrastructure descriptor enum at rest area"@en .

<http://datex2.eu/vocab/3/LocationReferencing/InfrastructureDescriptorEnum#atServiceArea>
  a <http://datex2.eu/vocab/3/LocationReferencing/InfrastructureDescriptorEnum> ;
  rdfs:comment "At service area."@en ;
  rdfs:label "Infrastructure descriptor enum at service area"@en .

<http://datex2.eu/vocab/3/LocationReferencing/InfrastructureDescriptorEnum#atTollPlaza>
  a <http://datex2.eu/vocab/3/LocationReferencing/InfrastructureDescriptorEnum> ;
  rdfs:comment "At toll plaza."@en ;
  rdfs:label "Infrastructure descriptor enum at toll plaza"@en .

<http://datex2.eu/vocab/3/LocationReferencing/InfrastructureDescriptorEnum#atTunnelEntryOrExit>
  a <http://datex2.eu/vocab/3/LocationReferencing/InfrastructureDescriptorEnum> ;
  rdfs:comment "At entry or exit of tunnel."@en ;
  rdfs:label "Infrastructure descriptor enum at tunnel entry or exit"@en .

<http://datex2.eu/vocab/3/LocationReferencing/InfrastructureDescriptorEnum#inGallery>
  a <http://datex2.eu/vocab/3/LocationReferencing/InfrastructureDescriptorEnum> ;
  rdfs:comment "In gallery."@en ;
  rdfs:label "Infrastructure descriptor enum in gallery"@en .

<http://datex2.eu/vocab/3/LocationReferencing/InfrastructureDescriptorEnum#inTunnel>
  a <http://datex2.eu/vocab/3/LocationReferencing/InfrastructureDescriptorEnum> ;
  rdfs:comment "In tunnel."@en ;
  rdfs:label "Infrastructure descriptor enum in tunnel"@en .

<http://datex2.eu/vocab/3/LocationReferencing/InfrastructureDescriptorEnum#onBridge>
  a <http://datex2.eu/vocab/3/LocationReferencing/InfrastructureDescriptorEnum> ;
  rdfs:comment "On bridge."@en ;
  rdfs:label "Infrastructure descriptor enum on bridge"@en .

<http://datex2.eu/vocab/3/LocationReferencing/InfrastructureDescriptorEnum#onConnector>
  a <http://datex2.eu/vocab/3/LocationReferencing/InfrastructureDescriptorEnum> ;
  rdfs:comment "On connecting carriageway between two different roads or road sections."@en ;
  rdfs:label "Infrastructure descriptor enum on connector"@en .

<http://datex2.eu/vocab/3/LocationReferencing/InfrastructureDescriptorEnum#onElevatedSection>
  a <http://datex2.eu/vocab/3/LocationReferencing/InfrastructureDescriptorEnum> ;
  rdfs:comment "On elevated section of road."@en ;
  rdfs:label "Infrastructure descriptor enum on elevated section"@en .

<http://datex2.eu/vocab/3/LocationReferencing/InfrastructureDescriptorEnum#onFlyover>
  a <http://datex2.eu/vocab/3/LocationReferencing/InfrastructureDescriptorEnum> ;
  rdfs:comment "On flyover, i.e. on section of road over another road."@en ;
  rdfs:label "Infrastructure descriptor enum on flyover"@en .

<http://datex2.eu/vocab/3/LocationReferencing/InfrastructureDescriptorEnum#onIceRoad>
  a <http://datex2.eu/vocab/3/LocationReferencing/InfrastructureDescriptorEnum> ;
  rdfs:comment "On ice road."@en ;
  rdfs:label "Infrastructure descriptor enum on ice road"@en .

<http://datex2.eu/vocab/3/LocationReferencing/InfrastructureDescriptorEnum#onLevelCrossing>
  a <http://datex2.eu/vocab/3/LocationReferencing/InfrastructureDescriptorEnum> ;
  rdfs:comment "On level-crossing."@en ;
  rdfs:label "Infrastructure descriptor enum on level crossing"@en .

<http://datex2.eu/vocab/3/LocationReferencing/InfrastructureDescriptorEnum#onLinkRoad>
  a <http://datex2.eu/vocab/3/LocationReferencing/InfrastructureDescriptorEnum> ;
  rdfs:comment "On road section linking two different roads."@en ;
  rdfs:label "Infrastructure descriptor enum on link road"@en .

<http://datex2.eu/vocab/3/LocationReferencing/InfrastructureDescriptorEnum#onRoundabout>
  a <http://datex2.eu/vocab/3/LocationReferencing/InfrastructureDescriptorEnum> ;
  rdfs:comment "On roundabout."@en ;
  rdfs:label "Infrastructure descriptor enum on roundabout"@en .

<http://datex2.eu/vocab/3/LocationReferencing/InfrastructureDescriptorEnum#onTheRoadway>
  a <http://datex2.eu/vocab/3/LocationReferencing/InfrastructureDescriptorEnum> ;
  rdfs:comment "On the roadway."@en ;
  rdfs:label "Infrastructure descriptor enum on the roadway"@en .

<http://datex2.eu/vocab/3/LocationReferencing/InfrastructureDescriptorEnum#onUndergroundSection>
  a <http://datex2.eu/vocab/3/LocationReferencing/InfrastructureDescriptorEnum> ;
  rdfs:comment "On underground section of road."@en ;
  rdfs:label "Infrastructure descriptor enum on underground section"@en .

<http://datex2.eu/vocab/3/LocationReferencing/InfrastructureDescriptorEnum#onUnderpass>
  a <http://datex2.eu/vocab/3/LocationReferencing/InfrastructureDescriptorEnum> ;
  rdfs:comment "On underpass, i.e. section of road which passes under another road."@en ;
  rdfs:label "Infrastructure descriptor enum on underpass"@en .

<http://datex2.eu/vocab/3/LocationReferencing/InfrastructureDescriptorEnum#withinJunction>
  a <http://datex2.eu/vocab/3/LocationReferencing/InfrastructureDescriptorEnum> ;
  rdfs:comment "On the main carriageway within a junction between exit slip road and entry slip road."@en ;
  rdfs:label "Infrastructure descriptor enum within junction"@en .

<http://datex2.eu/vocab/3/LocationReferencing/TpegLoc03JunctionPointDescriptorSubtypeEnum>
  a owl:Class ;
  rdfs:comment "TPEG loc03 junction point descriptor subtype enum"@en ;
  rdfs:label "TPEG loc03 junction point descriptor subtype enum"@en ;
  rdfs:subClassOf schema:Enumeration .

<http://datex2.eu/vocab/3/LocationReferencing/TpegLoc03JunctionPointDescriptorSubtypeEnum#junctionName>
  a <http://datex2.eu/vocab/3/LocationReferencing/TpegLoc03JunctionPointDescriptorSubtypeEnum> ;
  rdfs:comment "Name of a road network junction where two or more roads join."@en ;
  rdfs:label "TPEG loc03 junction point descriptor subtype enum junction name"@en .

<http://datex2.eu/vocab/3/LocationReferencing/TpegLoc03AreaDescriptorSubtypeEnum>
  a owl:Class ;
  rdfs:comment "TPEG loc03 area descriptor subtype enum"@en ;
  rdfs:label "TPEG loc03 area descriptor subtype enum"@en ;
  rdfs:subClassOf schema:Enumeration .

<http://datex2.eu/vocab/3/LocationReferencing/TpegLoc03AreaDescriptorSubtypeEnum#administrativeAreaName>
  a <http://datex2.eu/vocab/3/LocationReferencing/TpegLoc03AreaDescriptorSubtypeEnum> ;
  rdfs:comment "Name of an administrative area."@en ;
  rdfs:label "TPEG loc03 area descriptor subtype enum administrative area name"@en .

<http://datex2.eu/vocab/3/LocationReferencing/TpegLoc03AreaDescriptorSubtypeEnum#administrativeReferenceName>
  a <http://datex2.eu/vocab/3/LocationReferencing/TpegLoc03AreaDescriptorSubtypeEnum> ;
  rdfs:comment "Reference name by which administrative area is known."@en ;
  rdfs:label "TPEG loc03 area descriptor subtype enum administrative reference name"@en .

<http://datex2.eu/vocab/3/LocationReferencing/TpegLoc03AreaDescriptorSubtypeEnum#areaName>
  a <http://datex2.eu/vocab/3/LocationReferencing/TpegLoc03AreaDescriptorSubtypeEnum> ;
  rdfs:comment "Name of an area."@en ;
  rdfs:label "TPEG loc03 area descriptor subtype enum area name"@en .

<http://datex2.eu/vocab/3/LocationReferencing/TpegLoc03AreaDescriptorSubtypeEnum#countyName>
  a <http://datex2.eu/vocab/3/LocationReferencing/TpegLoc03AreaDescriptorSubtypeEnum> ;
  rdfs:comment "Name of a county (administrative sub-division)."@en ;
  rdfs:label "TPEG loc03 area descriptor subtype enum county name"@en .

<http://datex2.eu/vocab/3/LocationReferencing/TpegLoc03AreaDescriptorSubtypeEnum#lakeName>
  a <http://datex2.eu/vocab/3/LocationReferencing/TpegLoc03AreaDescriptorSubtypeEnum> ;
  rdfs:comment "Name of a lake."@en ;
  rdfs:label "TPEG loc03 area descriptor subtype enum lake name"@en .

<http://datex2.eu/vocab/3/LocationReferencing/TpegLoc03AreaDescriptorSubtypeEnum#nationName>
  a <http://datex2.eu/vocab/3/LocationReferencing/TpegLoc03AreaDescriptorSubtypeEnum> ;
  rdfs:comment "Name of a nation (e.g. Wales) which is a sub-division of a ISO recognised country."@en ;
  rdfs:label "TPEG loc03 area descriptor subtype enum nation name"@en .

<http://datex2.eu/vocab/3/LocationReferencing/TpegLoc03AreaDescriptorSubtypeEnum#policeForceControlAreaName>
  a <http://datex2.eu/vocab/3/LocationReferencing/TpegLoc03AreaDescriptorSubtypeEnum> ;
  rdfs:comment "Name of a police force control area."@en ;
  rdfs:label "TPEG loc03 area descriptor subtype enum police force control area name"@en .

<http://datex2.eu/vocab/3/LocationReferencing/TpegLoc03AreaDescriptorSubtypeEnum#regionName>
  a <http://datex2.eu/vocab/3/LocationReferencing/TpegLoc03AreaDescriptorSubtypeEnum> ;
  rdfs:comment "Name of a geographic region."@en ;
  rdfs:label "TPEG loc03 area descriptor subtype enum region name"@en .

<http://datex2.eu/vocab/3/LocationReferencing/TpegLoc03AreaDescriptorSubtypeEnum#seaName>
  a <http://datex2.eu/vocab/3/LocationReferencing/TpegLoc03AreaDescriptorSubtypeEnum> ;
  rdfs:comment "Name of a sea."@en ;
  rdfs:label "TPEG loc03 area descriptor subtype enum sea name"@en .

<http://datex2.eu/vocab/3/LocationReferencing/TpegLoc03AreaDescriptorSubtypeEnum#townName>
  a <http://datex2.eu/vocab/3/LocationReferencing/TpegLoc03AreaDescriptorSubtypeEnum> ;
  rdfs:comment "Name of a town."@en ;
  rdfs:label "TPEG loc03 area descriptor subtype enum town name"@en .

<http://datex2.eu/vocab/3/LocationReferencing/TpegLoc03AreaDescriptorSubtypeEnum#other>
  a <http://datex2.eu/vocab/3/LocationReferencing/TpegLoc03AreaDescriptorSubtypeEnum> ;
  rdfs:comment "Other than as defined in this enumeration."@en ;
  rdfs:label "TPEG loc03 area descriptor subtype enum other"@en .

<http://datex2.eu/vocab/3/LocationReferencing/AreaLocation>
  a owl:Class ;
  rdfs:comment "Location representing a geographic or geometric defined area which may be qualified by height information to provide additional geospatial discrimination (e.g. for snow in an area but only above a certain altitude)."@en ;
  rdfs:label "Area location"@en ;
  rdfs:subClassOf <http://datex2.eu/vocab/3/LocationReferencing/Location> .

<http://datex2.eu/vocab/3/LocationReferencing/Location>
  a owl:Class ;
  rdfs:comment "The specification of a location either on a network (as a point or a linear location) or as an area. This may be provided in one or more referencing systems."@en ;
  rdfs:label "Location"@en ;
  rdfs:subClassOf <http://datex2.eu/vocab/3/LocationReferencing/LocationReference> .

<http://datex2.eu/vocab/3/LocationReferencing/LinearLocation>
  a owl:Class ;
  rdfs:comment "Location representing a linear section with optional directionality defined between two points. "@en ;
  rdfs:label "Linear location"@en ;
  rdfs:subClassOf <http://datex2.eu/vocab/3/LocationReferencing/NetworkLocation> .

<http://datex2.eu/vocab/3/LocationReferencing/NetworkLocation>
  a owl:Class ;
  rdfs:comment "The specification of a location on a network (as a point or a linear location)."@en ;
  rdfs:label "Network location"@en ;
  rdfs:subClassOf <http://datex2.eu/vocab/3/LocationReferencing/Location> .

<http://datex2.eu/vocab/3/LocationReferencing/PointLocation>
  a owl:Class ;
  rdfs:comment "Location representing a single geospatial point."@en ;
  rdfs:label "Point location"@en ;
  rdfs:subClassOf <http://datex2.eu/vocab/3/LocationReferencing/NetworkLocation> .

<http://datex2.eu/vocab/3/LocationReferencing/SingleRoadLinearLocation>
  a owl:Class ;
  rdfs:comment "Location representing a linear section along a single road with optional directionality defined between two points on the same road. No matter the kind of linear reference it uses, the constraint of using only a single road must be preserved."@en ;
  rdfs:label "Single road linear location"@en ;
  rdfs:subClassOf <http://datex2.eu/vocab/3/LocationReferencing/LinearLocation> .

<http://datex2.eu/vocab/3/LocationReferencing/AreaDestination>
  a owl:Class ;
  rdfs:comment "The specification of the destination of a defined route or itinerary which is an area."@en ;
  rdfs:label "Area destination"@en ;
  rdfs:subClassOf <http://datex2.eu/vocab/3/LocationReferencing/Destination> .

<http://datex2.eu/vocab/3/LocationReferencing/Destination>
  a owl:Class ;
  rdfs:comment "The specification of a destination. This may be either a point location or an area location."@en ;
  rdfs:label "Destination"@en .

<http://datex2.eu/vocab/3/LocationReferencing/ExternalReferencing>
  a owl:Class ;
  rdfs:comment "A location defined by reference to an external/other referencing system."@en ;
  rdfs:label "External referencing"@en .

<http://datex2.eu/vocab/3/LocationReferencing/Itinerary>
  a owl:Class ;
  rdfs:comment "Multiple (i.e. more than one) physically separate locations arranged as an ordered set that defines an itinerary or route."@en ;
  rdfs:label "Itinerary"@en ;
  rdfs:subClassOf <http://datex2.eu/vocab/3/LocationReferencing/LocationReference> .

<http://datex2.eu/vocab/3/LocationReferencing/LocationReference>
  a owl:Class ;
  rdfs:comment "Represents one or more physically separate locations. Multiple locations may be related, as in an itinerary or route, or may be unrelated. One LocationReference should not use multiple Location objects to represent the same physical location."@en ;
  rdfs:label "Location reference"@en .

<http://datex2.eu/vocab/3/LocationReferencing/ItineraryByIndexedLocations>
  a owl:Class ;
  rdfs:comment "Multiple physically separate locations arranged as an ordered set that defines an itinerary or route. The index qualifier indicates the order."@en ;
  rdfs:label "Itinerary by indexed locations"@en ;
  rdfs:subClassOf <http://datex2.eu/vocab/3/LocationReferencing/Itinerary> .

<http://datex2.eu/vocab/3/LocationReferencing/ItineraryByReference>
  a owl:Class ;
  rdfs:comment "Multiple (i.e. more than one) physically separate locations which are ordered that constitute an itinerary or route where they are defined by reference to a predefined itinerary."@en ;
  rdfs:label "Itinerary by reference"@en ;
  rdfs:subClassOf <http://datex2.eu/vocab/3/LocationReferencing/Itinerary> .

<http://datex2.eu/vocab/3/LocationReferencing/LocationByReference>
  a owl:Class ;
  rdfs:comment "A location defined by reference to a predefined location."@en ;
  rdfs:label "Location by reference"@en ;
  rdfs:subClassOf <http://datex2.eu/vocab/3/LocationReferencing/Location> .

<http://datex2.eu/vocab/3/LocationReferencing/LocationGroup>
  a owl:Class ;
  rdfs:comment "Multiple (i.e. more than one) physically separate locations which have no specific order."@en ;
  rdfs:label "Location group"@en ;
  rdfs:subClassOf <http://datex2.eu/vocab/3/LocationReferencing/LocationReference> .

<http://datex2.eu/vocab/3/LocationReferencing/LocationGroupByList>
  a owl:Class ;
  rdfs:comment "A group of (i.e. more than one) physically separate locations which have no specific order and where each location is explicitly listed."@en ;
  rdfs:label "Location group by list"@en ;
  rdfs:subClassOf <http://datex2.eu/vocab/3/LocationReferencing/LocationGroup> .

<http://datex2.eu/vocab/3/LocationReferencing/LocationGroupByReference>
  a owl:Class ;
  rdfs:comment "A group of (i.e. more than one) physically separate locations which have no specific order that are defined by reference to a predefined non ordered location group."@en ;
  rdfs:label "Location group by reference"@en ;
  rdfs:subClassOf <http://datex2.eu/vocab/3/LocationReferencing/LocationGroup> .

<http://datex2.eu/vocab/3/LocationReferencing/OffsetDistance>
  a owl:Class ;
  rdfs:comment "The non-negative offset distance from the ALERT-C referenced point to the actual point."@en ;
  rdfs:label "Offset distance"@en .

<http://datex2.eu/vocab/3/LocationReferencing/PointDestination>
  a owl:Class ;
  rdfs:comment "The specification of the destination of a defined route or itinerary which is a point."@en ;
  rdfs:label "Point destination"@en ;
  rdfs:subClassOf <http://datex2.eu/vocab/3/LocationReferencing/Destination> .

<http://datex2.eu/vocab/3/LocationReferencing/AlertCLinear>
  a owl:Class ;
  rdfs:comment "A linear section along a road defined between two points on the road by reference to a pre-defined ALERT-C location table."@en ;
  rdfs:label "ALERT-C linear"@en .

<http://datex2.eu/vocab/3/LocationReferencing/AlertCPoint>
  a owl:Class ;
  rdfs:comment "A single point on the road network defined by reference to a pre-defined ALERT-C location table and which has an associated direction of traffic flow."@en ;
  rdfs:label "ALERT-C point"@en .

<http://datex2.eu/vocab/3/LocationReferencing/AlertCDirection>
  a owl:Class ;
  rdfs:comment "The direction of traffic flow along the road to which the information relates."@en ;
  rdfs:label "ALERT-C direction"@en .

<http://datex2.eu/vocab/3/LocationReferencing/AlertCLocation>
  a owl:Class ;
  rdfs:comment "Identification of a specific point, linear or area location in an ALERT-C location table."@en ;
  rdfs:label "ALERT-C location"@en .

<http://datex2.eu/vocab/3/LocationReferencing/AlertCMethod2PrimaryPointLocation>
  a owl:Class ;
  rdfs:comment "The point (called Primary point) which is either a single point or at the downstream end of a linear road section. The point is specified by a reference to a point in a pre-defined ALERT-C location table."@en ;
  rdfs:label "ALERT-C method2 primary point location"@en .

<http://datex2.eu/vocab/3/LocationReferencing/AlertCMethod2SecondaryPointLocation>
  a owl:Class ;
  rdfs:comment "The point (called Secondary point) which is at the upstream end of a linear road section. The point is specified by a reference to a point in a pre-defined ALERT-C location table."@en ;
  rdfs:label "ALERT-C method2 secondary point location"@en .

<http://datex2.eu/vocab/3/LocationReferencing/AlertCMethod4PrimaryPointLocation>
  a owl:Class ;
  rdfs:comment "The point (called Primary point) which is either a single point or at the downstream end of a linear road section. The point is specified by a reference to a point in a pre-defined ALERT-C location table plus a non-negative offset distance."@en ;
  rdfs:label "ALERT-C method4 primary point location"@en .

<http://datex2.eu/vocab/3/LocationReferencing/AlertCMethod4SecondaryPointLocation>
  a owl:Class ;
  rdfs:comment "The point (called Secondary point) which is at the upstream end of a linear road section. The point is specified by a reference to a point in a pre-defined Alert-C location table plus a non-negative offset distance."@en ;
  rdfs:label "ALERT-C method4 secondary point location"@en .

<http://datex2.eu/vocab/3/LocationReferencing/AlertCArea>
  a owl:Class ;
  rdfs:comment "An area defined by reference to a predefined ALERT-C location table."@en ;
  rdfs:label "ALERT-C area"@en .

<http://datex2.eu/vocab/3/LocationReferencing/AlertCLinearByCode>
  a owl:Class ;
  rdfs:comment "A linear section along a road defined by reference to a linear section in a pre-defined ALERT-C location table."@en ;
  rdfs:label "ALERT-C linear by code"@en ;
  rdfs:subClassOf <http://datex2.eu/vocab/3/LocationReferencing/AlertCLinear> .

<http://datex2.eu/vocab/3/LocationReferencing/AlertCMethod2Linear>
  a owl:Class ;
  rdfs:comment "A linear section along a road between two points, primary and secondary, which are pre-defined in an ALERT-C location table. Direction is FROM the secondary point TO the primary point, i.e. the primary point is downstream of the secondary point."@en ;
  rdfs:label "ALERT-C method2 linear"@en ;
  rdfs:subClassOf <http://datex2.eu/vocab/3/LocationReferencing/AlertCLinear> .

<http://datex2.eu/vocab/3/LocationReferencing/AlertCMethod2Point>
  a owl:Class ;
  rdfs:comment "A single point on the road network defined by reference to a point in a pre-defined ALERT-C location table and which has an associated direction of traffic flow."@en ;
  rdfs:label "ALERT-C method2 point"@en ;
  rdfs:subClassOf <http://datex2.eu/vocab/3/LocationReferencing/AlertCPoint> .

<http://datex2.eu/vocab/3/LocationReferencing/AlertCMethod4Linear>
  a owl:Class ;
  rdfs:comment "A linear section along a road between two points, primary and secondary, which are pre-defined ALERT-C locations plus offset distance. Direction is FROM the secondary point TO the primary point, i.e. the primary point is downstream of the secondary point."@en ;
  rdfs:label "ALERT-C method4 linear"@en ;
  rdfs:subClassOf <http://datex2.eu/vocab/3/LocationReferencing/AlertCLinear> .

<http://datex2.eu/vocab/3/LocationReferencing/AlertCMethod4Point>
  a owl:Class ;
  rdfs:comment "A single point on the road network defined by reference to a point in a pre-defined ALERT-C location table plus an offset distance and which has an associated direction of traffic flow."@en ;
  rdfs:label "ALERT-C method4 point"@en ;
  rdfs:subClassOf <http://datex2.eu/vocab/3/LocationReferencing/AlertCPoint> .

<http://datex2.eu/vocab/3/LocationReferencing/GmlLinearRing>
  a owl:Class ;
  rdfs:comment "Closed line string not self-intersecting (i.e. having as last point the first point)"@en ;
  rdfs:label "Gml linear ring"@en ;
  rdfs:subClassOf <http://datex2.eu/vocab/3/LocationReferencing/GmlLineString> .

<http://datex2.eu/vocab/3/LocationReferencing/GmlLineString>
  a owl:Class ;
  rdfs:comment "Line string based on GML (EN ISO 19136) definition: a curve defined by a series of two or more coordinate tuples. Unlike GML may be self-intersecting. If srsName attribute is not present, posList is assumed to use \"ETRS89-LatLonh\" reference system."@en ;
  rdfs:label "Gml line string"@en .

<http://datex2.eu/vocab/3/LocationReferencing/GmlMultiPolygon>
  a owl:Class ;
  rdfs:comment "An area defined by a set of polygons acording to GML (EN ISO 19136)."@en ;
  rdfs:label "Gml multi polygon"@en .

<http://datex2.eu/vocab/3/LocationReferencing/GmlPolygon>
  a owl:Class ;
  rdfs:comment "Planar surface defined by 1 exterior boundary and 0 or more interior boundaries"@en ;
  rdfs:label "Gml polygon"@en .

<http://datex2.eu/vocab/3/LocationReferencing/LinearWithinLinearElement>
  a owl:Class ;
  rdfs:comment "A linear section along a linear element where the linear element is either a part of or the whole of a linear object (i.e. a road), consistent with ISO 19148 definitions. "@en ;
  rdfs:label "Linear within linear element"@en .

<http://datex2.eu/vocab/3/LocationReferencing/LinearElementByLineString>
  a owl:Class ;
  rdfs:comment "A linear element defined by a line string (class GmlLineString)."@en ;
  rdfs:label "Linear element by line string"@en ;
  rdfs:subClassOf <http://datex2.eu/vocab/3/LocationReferencing/LinearElement> .

<http://datex2.eu/vocab/3/LocationReferencing/LinearElement>
  a owl:Class ;
  rdfs:comment "A linear element along a single linear object, consistent with EN ISO 19148 definitions. "@en ;
  rdfs:label "Linear element"@en .

<http://datex2.eu/vocab/3/LocationReferencing/DistanceAlongLinearElement>
  a owl:Class ;
  rdfs:comment "Distance of a point along a linear element either measured from the start node or a defined referent on that linear element, where the start node is relative to the element definition rather than the direction of traffic flow."@en ;
  rdfs:label "Distance along linear element"@en .

<http://datex2.eu/vocab/3/LocationReferencing/DistanceFromLinearElementReferent>
  a owl:Class ;
  rdfs:comment "Distance of a point along a linear element measured from a \"from referent\" on the linear element, in the sense relative to the linear element definition rather than the direction of traffic flow or optionally towards a \"towards referent\"."@en ;
  rdfs:label "Distance from linear element referent"@en ;
  rdfs:subClassOf <http://datex2.eu/vocab/3/LocationReferencing/DistanceAlongLinearElement> .

<http://datex2.eu/vocab/3/LocationReferencing/DistanceFromLinearElementStart>
  a owl:Class ;
  rdfs:comment "Distance of a point along a linear element measured from the start node of the linear element, where start node is relative to the element definition rather than the direction of traffic flow."@en ;
  rdfs:label "Distance from linear element start"@en ;
  rdfs:subClassOf <http://datex2.eu/vocab/3/LocationReferencing/DistanceAlongLinearElement> .

<http://datex2.eu/vocab/3/LocationReferencing/LinearElementByCode>
  a owl:Class ;
  rdfs:comment "A linear element along a single linear object defined by its identifier or code in a road network reference model (specified in LinearElement class) which segments the road network according to specific business rules."@en ;
  rdfs:label "Linear element by code"@en ;
  rdfs:subClassOf <http://datex2.eu/vocab/3/LocationReferencing/LinearElement> .

<http://datex2.eu/vocab/3/LocationReferencing/LinearElementByPoints>
  a owl:Class ;
  rdfs:comment "A linear element along a single linear object defined by its start and end points."@en ;
  rdfs:label "Linear element by points"@en ;
  rdfs:subClassOf <http://datex2.eu/vocab/3/LocationReferencing/LinearElement> .

<http://datex2.eu/vocab/3/LocationReferencing/PercentageDistanceAlongLinearElement>
  a owl:Class ;
  rdfs:comment "Distance of a point along a linear element measured from the start node expressed as a percentage of the whole length of the linear element, where start node is relative to the element definition rather than the direction of traffic flow."@en ;
  rdfs:label "Percentage distance along linear element"@en ;
  rdfs:subClassOf <http://datex2.eu/vocab/3/LocationReferencing/DistanceAlongLinearElement> .

<http://datex2.eu/vocab/3/LocationReferencing/PointAlongLinearElement>
  a owl:Class ;
  rdfs:comment "A point on a linear element where the linear element is either a part of or the whole of a linear object (i.e. a road), consistent with EN ISO 19148 definitions. "@en ;
  rdfs:label "Point along linear element"@en .

<http://datex2.eu/vocab/3/LocationReferencing/Referent>
  a owl:Class ;
  rdfs:comment "A referent on a linear object that has a known location such as a node, a reference marker (e.g. a marker-post), an intersection etc."@en ;
  rdfs:label "Referent"@en .

<http://datex2.eu/vocab/3/LocationReferencing/AltitudeConfidence>
  a owl:Class ;
  rdfs:comment "Evaluation of the altitude confidence assessed according to ETSI ISO 102894-2"@en ;
  rdfs:label "Altitude confidence"@en .

<http://datex2.eu/vocab/3/LocationReferencing/HeightCoordinate>
  a owl:Class ;
  rdfs:comment "Third coordinate for points defined geodetically"@en ;
  rdfs:label "Height coordinate"@en .

<http://datex2.eu/vocab/3/LocationReferencing/PointByCoordinates>
  a owl:Class ;
  rdfs:comment "A single point defined only by a coordinate set with an optional bearing direction."@en ;
  rdfs:label "Point by coordinates"@en .

<http://datex2.eu/vocab/3/LocationReferencing/PositionAccuracy>
  a owl:Class ;
  rdfs:comment "Horizontal position accuracy parameters defined according to EN 16803-1"@en ;
  rdfs:label "Position accuracy"@en .

<http://datex2.eu/vocab/3/LocationReferencing/PositionConfidenceEllipse>
  a owl:Class ;
  rdfs:comment "Confidence ellipse position defined in a shape of ellipse with a predefined confidence level (e.g. 95 %). The centre of the ellipse shape corresponds to the reference position point for which the position accuracy is evaluated."@en ;
  rdfs:label "Position confidence ellipse"@en .

<http://datex2.eu/vocab/3/LocationReferencing/PointCoordinates>
  a owl:Class ;
  rdfs:comment "A pair of planar coordinates defining the geodetic position of a single point using the European Terrestrial Reference System 1989 (ETRS89)."@en ;
  rdfs:label "Point coordinates"@en .

<http://datex2.eu/vocab/3/LocationReferencing/Lane>
  a owl:Class ;
  rdfs:comment "Indicates a specific lane or group of lanes."@en ;
  rdfs:label "Lane"@en .

<http://datex2.eu/vocab/3/LocationReferencing/RoadInformation>
  a owl:Class ;
  rdfs:comment "Information on a road"@en ;
  rdfs:label "Road information"@en .

<http://datex2.eu/vocab/3/LocationReferencing/Carriageway>
  a owl:Class ;
  rdfs:comment "Supplementary positional information which details carriageway and lane locations. Several instances may exist where the element being described extends over more than one carriageway."@en ;
  rdfs:label "Carriageway"@en .

<http://datex2.eu/vocab/3/LocationReferencing/SupplementaryPositionalDescription>
  a owl:Class ;
  rdfs:comment "A collection of supplementary positional information which improves the precision of the location."@en ;
  rdfs:label "Supplementary positional description"@en .

<http://datex2.eu/vocab/3/LocationReferencing/TpegAreaLocation>
  a owl:Class ;
  rdfs:comment "A geographic or geometric area defined by a TPEG-Loc structure which may include height information for additional geospatial discrimination."@en ;
  rdfs:label "TPEG area location"@en .

<http://datex2.eu/vocab/3/LocationReferencing/TpegGeometricArea>
  a owl:Class ;
  rdfs:comment "A geometric area defined by a centre point and a radius."@en ;
  rdfs:label "TPEG geometric area"@en ;
  rdfs:subClassOf <http://datex2.eu/vocab/3/LocationReferencing/TpegAreaLocation> .

<http://datex2.eu/vocab/3/LocationReferencing/TpegHeight>
  a owl:Class ;
  rdfs:comment "Height information which provides additional discrimination for the applicable area."@en ;
  rdfs:label "TPEG height"@en .

<http://datex2.eu/vocab/3/LocationReferencing/TpegNamedOnlyArea>
  a owl:Class ;
  rdfs:comment "An area defined by a well-known name."@en ;
  rdfs:label "TPEG named only area"@en ;
  rdfs:subClassOf <http://datex2.eu/vocab/3/LocationReferencing/TpegAreaLocation> .

<http://datex2.eu/vocab/3/LocationReferencing/TpegAreaDescriptor>
  a owl:Class ;
  rdfs:comment "A descriptor for describing an area location."@en ;
  rdfs:label "TPEG area descriptor"@en ;
  rdfs:subClassOf <http://datex2.eu/vocab/3/LocationReferencing/TpegDescriptor> .

<http://datex2.eu/vocab/3/LocationReferencing/TpegDescriptor>
  a owl:Class ;
  rdfs:comment "A collection of information providing descriptive references to locations using the TPEG-Loc location referencing approach."@en ;
  rdfs:label "TPEG descriptor"@en .

<http://datex2.eu/vocab/3/LocationReferencing/TpegIlcPointDescriptor>
  a owl:Class ;
  rdfs:comment "A descriptor for describing a junction by defining the intersecting roads."@en ;
  rdfs:label "TPEG ILC point descriptor"@en ;
  rdfs:subClassOf <http://datex2.eu/vocab/3/LocationReferencing/TpegPointDescriptor> .

<http://datex2.eu/vocab/3/LocationReferencing/TpegPointDescriptor>
  a owl:Class ;
  rdfs:comment "A descriptor for describing a point location."@en ;
  rdfs:label "TPEG point descriptor"@en ;
  rdfs:subClassOf <http://datex2.eu/vocab/3/LocationReferencing/TpegDescriptor> .

<http://datex2.eu/vocab/3/LocationReferencing/TpegJunctionPointDescriptor>
  a owl:Class ;
  rdfs:comment "A descriptor for describing a point at a junction on a road network."@en ;
  rdfs:label "TPEG junction point descriptor"@en ;
  rdfs:subClassOf <http://datex2.eu/vocab/3/LocationReferencing/TpegPointDescriptor> .

<http://datex2.eu/vocab/3/LocationReferencing/TpegOtherPointDescriptor>
  a owl:Class ;
  rdfs:comment "General descriptor for describing a point."@en ;
  rdfs:label "TPEG other point descriptor"@en ;
  rdfs:subClassOf <http://datex2.eu/vocab/3/LocationReferencing/TpegPointDescriptor> .

<http://datex2.eu/vocab/3/LocationReferencing/TpegLinearLocation>
  a owl:Class ;
  rdfs:comment "A linear section along a single road defined between two points on the same road by a TPEG-Loc structure."@en ;
  rdfs:label "TPEG linear location"@en .

<http://datex2.eu/vocab/3/LocationReferencing/TpegFramedPoint>
  a owl:Class ;
  rdfs:comment "A point on the road network which is framed between two other points on the same road."@en ;
  rdfs:label "TPEG framed point"@en ;
  rdfs:subClassOf <http://datex2.eu/vocab/3/LocationReferencing/TpegPointLocation> .

<http://datex2.eu/vocab/3/LocationReferencing/TpegPointLocation>
  a owl:Class ;
  rdfs:comment "A single point on the road network defined by a TPEG-Loc structure and which has an associated direction of traffic flow."@en ;
  rdfs:label "TPEG point location"@en .

<http://datex2.eu/vocab/3/LocationReferencing/TpegPoint>
  a owl:Class ;
  rdfs:comment "A point on the road network which is either a junction point or a non junction point."@en ;
  rdfs:label "TPEG point"@en .

<http://datex2.eu/vocab/3/LocationReferencing/TpegSimplePoint>
  a owl:Class ;
  rdfs:comment "A point on the road network which is not bounded by any other points on the road network."@en ;
  rdfs:label "TPEG simple point"@en ;
  rdfs:subClassOf <http://datex2.eu/vocab/3/LocationReferencing/TpegPointLocation> .

<http://datex2.eu/vocab/3/LocationReferencing/TpegJunction>
  a owl:Class ;
  rdfs:comment "A point on the road network which is a road junction point."@en ;
  rdfs:label "TPEG junction"@en ;
  rdfs:subClassOf <http://datex2.eu/vocab/3/LocationReferencing/TpegPoint> .

<http://datex2.eu/vocab/3/LocationReferencing/TpegNonJunctionPoint>
  a owl:Class ;
  rdfs:comment "A point on the road network which is not a road junction point."@en ;
  rdfs:label "TPEG non junction point"@en ;
  rdfs:subClassOf <http://datex2.eu/vocab/3/LocationReferencing/TpegPoint> .

<http://datex2.eu/vocab/3/LocationReferencing/OpenlrBaseReferencePoint>
  a owl:Class ;
  rdfs:comment "Base class used to hold data about a reference point."@en ;
  rdfs:label "Openlr base reference point"@en .

<http://datex2.eu/vocab/3/LocationReferencing/OpenlrLineAttributes>
  a owl:Class ;
  rdfs:comment "Line attributes are part of a location reference point and consists of functional road class (FRC),form of way (FOW) and bearing (BEAR) data."@en ;
  rdfs:label "Openlr line attributes"@en .

<http://datex2.eu/vocab/3/LocationReferencing/OpenlrOffsets>
  a owl:Class ;
  rdfs:comment "Offsets are used to locate the start and end of a location more precisely than bounding to the nodes in a network."@en ;
  rdfs:label "Openlr offsets"@en .

<http://datex2.eu/vocab/3/LocationReferencing/OpenlrPathAttributes>
  a owl:Class ;
  rdfs:comment "Properties of the path from the associated location reference point to the next location reference point, which are specified to assist correct identification of the point in an external map data source."@en ;
  rdfs:label "Openlr path attributes"@en .

<http://datex2.eu/vocab/3/LocationReferencing/OpenlrAreaLocationReference>
  a owl:Class ;
  rdfs:comment "A two-dimensional part of the surface of the earth which is bounded by a closed curve. An area location may cover parts of the road network but does not necessarily need to. It is represented according to the OpenLR standard for Area Locations"@en ;
  rdfs:label "Openlr area location reference"@en .

<http://datex2.eu/vocab/3/LocationReferencing/OpenlrCircleLocationReference>
  a owl:Class ;
  rdfs:comment "The OpenLR method of area definition by providing a center position and a radius"@en ;
  rdfs:label "Openlr circle location reference"@en ;
  rdfs:subClassOf <http://datex2.eu/vocab/3/LocationReferencing/OpenlrAreaLocationReference> .

<http://datex2.eu/vocab/3/LocationReferencing/OpenlrClosedLineLocationReference>
  a owl:Class ;
  rdfs:comment """The OpenLR method of area definition by providing a closed path (i.e. a circuit) in the road network.
The boundary always consists of road segments"""@en ;
  rdfs:label "Openlr closed line location reference"@en ;
  rdfs:subClassOf <http://datex2.eu/vocab/3/LocationReferencing/OpenlrAreaLocationReference> .

<http://datex2.eu/vocab/3/LocationReferencing/OpenlrGridLocationReference>
  a owl:Class ;
  rdfs:comment "Area defined using an OpenLR™ method consisting in defining it by a tessellation of rectangles"@en ;
  rdfs:label "Openlr grid location reference"@en ;
  rdfs:subClassOf <http://datex2.eu/vocab/3/LocationReferencing/OpenlrAreaLocationReference> .

<http://datex2.eu/vocab/3/LocationReferencing/OpenlrPolygonCorners>
  a owl:Class ;
  rdfs:comment "A geodetic coordinate Tuple that defines the vertices of the underlying geometrical polygon."@en ;
  rdfs:label "Openlr polygon corners"@en .

<http://datex2.eu/vocab/3/LocationReferencing/OpenlrPolygonLocationReference>
  a owl:Class ;
  rdfs:comment "The OpenLR method of area definition by providing points that bound the area"@en ;
  rdfs:label "Openlr polygon location reference"@en ;
  rdfs:subClassOf <http://datex2.eu/vocab/3/LocationReferencing/OpenlrAreaLocationReference> .

<http://datex2.eu/vocab/3/LocationReferencing/OpenlrRectangle>
  a owl:Class ;
  rdfs:comment "Area delimited by a rectangle defined by the geodetic co-ordinates of the two ends of its diagonal from south-west to north-east (the rectangle having two sides that are parallel to lines of latitude)"@en ;
  rdfs:label "Openlr rectangle"@en .

<http://datex2.eu/vocab/3/LocationReferencing/OpenlrRectangleLocationReference>
  a owl:Class ;
  rdfs:comment "The openLR method of area definition by providing a rectangular shape defined by two geo-coordinate pairs"@en ;
  rdfs:label "Openlr rectangle location reference"@en ;
  rdfs:subClassOf <http://datex2.eu/vocab/3/LocationReferencing/OpenlrAreaLocationReference> .

<http://datex2.eu/vocab/3/LocationReferencing/OpenlrLinear>
  a owl:Class ;
  rdfs:comment "OpenLR line location reference"@en ;
  rdfs:label "Openlr linear"@en .

<http://datex2.eu/vocab/3/LocationReferencing/OpenlrLineLocationReference>
  a owl:Class ;
  rdfs:comment "A line location reference is defined by an ordered sequence of location reference points and a terminating last location reference point."@en ;
  rdfs:label "Openlr line location reference"@en .

<http://datex2.eu/vocab/3/LocationReferencing/OpenlrBasePointLocation>
  a owl:Class ;
  rdfs:comment "Holds common data that are used both in OpenlrPointAccessPoint and OpenlrPointAlongLine."@en ;
  rdfs:label "Openlr base point location"@en ;
  rdfs:subClassOf <http://datex2.eu/vocab/3/LocationReferencing/OpenlrPointLocationReference> .

<http://datex2.eu/vocab/3/LocationReferencing/OpenlrPointLocationReference>
  a owl:Class ;
  rdfs:comment "A point location is a zero-dimensional element in a map that specifies a geometric location."@en ;
  rdfs:label "Openlr point location reference"@en .

<http://datex2.eu/vocab/3/LocationReferencing/OpenlrGeoCoordinate>
  a owl:Class ;
  rdfs:comment "A geo-coordinate pair is a position in a map defined by its longitude and latitude coordinate values."@en ;
  rdfs:label "Openlr geo coordinate"@en ;
  rdfs:subClassOf <http://datex2.eu/vocab/3/LocationReferencing/OpenlrPointLocationReference> .

<http://datex2.eu/vocab/3/LocationReferencing/OpenlrLastLocationReferencePoint>
  a owl:Class ;
  rdfs:comment "The sequence of location reference points is terminated by a last location reference point."@en ;
  rdfs:label "Openlr last location reference point"@en ;
  rdfs:subClassOf <http://datex2.eu/vocab/3/LocationReferencing/OpenlrBaseReferencePoint> .

<http://datex2.eu/vocab/3/LocationReferencing/OpenlrLocationReferencePoint>
  a owl:Class ;
  rdfs:comment "The basis of a location reference is a sequence of location reference points (LRPs)."@en ;
  rdfs:label "Openlr location reference point"@en ;
  rdfs:subClassOf <http://datex2.eu/vocab/3/LocationReferencing/OpenlrBaseReferencePoint> .

<http://datex2.eu/vocab/3/LocationReferencing/OpenlrPointAlongLine>
  a owl:Class ;
  rdfs:comment "Point along a line"@en ;
  rdfs:label "Openlr point along line"@en ;
  rdfs:subClassOf <http://datex2.eu/vocab/3/LocationReferencing/OpenlrBasePointLocation> .

<http://datex2.eu/vocab/3/LocationReferencing/OpenlrPointAttributes>
  a owl:Class ;
  rdfs:comment "Holds common data that are used both in OpenlrPointAccessPoint and OpenlrPointAlongLine."@en ;
  rdfs:label "Openlr point attributes"@en .

<http://datex2.eu/vocab/3/LocationReferencing/OpenlrPoiWithAccessPoint>
  a owl:Class ;
  rdfs:comment "A point of interest (POI) along a line with access is a point location which is defined by a linear reference path, an offset value (defining the access point) from the starting node of this path and a coordinate pair that defines the POI itself."@en ;
  rdfs:label "Openlr poi with access point"@en ;
  rdfs:subClassOf <http://datex2.eu/vocab/3/LocationReferencing/OpenlrBasePointLocation> .

<http://datex2.eu/vocab/3/LocationReferencing/IsoNamedArea>
  a owl:Class ;
  rdfs:comment "The ISO 3166-2 representation for the named area."@en ;
  rdfs:label "Iso named area"@en ;
  rdfs:subClassOf <http://datex2.eu/vocab/3/LocationReferencing/NamedArea> .

<http://datex2.eu/vocab/3/LocationReferencing/NamedArea>
  a owl:Class ;
  rdfs:comment "An area defined by a name and/or in terms of known boundaries, such as country or county boundaries or allocated control area of particular authority. The attributes do not form a union; instead, the smallest intersection forms the resulting area."@en ;
  rdfs:label "Named area"@en ;
  rdfs:subClassOf <http://datex2.eu/vocab/3/Common/NamedArea> .

<http://datex2.eu/vocab/3/LocationReferencing/NutsNamedArea>
  a owl:Class ;
  rdfs:comment "The NUTS-Code representation for the named area (Nomenclature of territorial units for statistics) or its LAU code representation (Local Administrative Unit)."@en ;
  rdfs:label "Nuts named area"@en ;
  rdfs:subClassOf <http://datex2.eu/vocab/3/LocationReferencing/NamedArea> .

<http://datex2.eu/vocab/3/LocationReferencing/PredefinedItinerary>
  a owl:Class ;
  rdfs:comment "An identifiable versioned instance of a predefined itinerary."@en ;
  rdfs:label "Predefined itinerary"@en ;
  rdfs:subClassOf <http://datex2.eu/vocab/3/LocationReferencing/PredefinedLocationReference> .

<http://datex2.eu/vocab/3/LocationReferencing/PredefinedLocationReference>
  a owl:Class ;
  rdfs:comment "A location reference which is predefined and may be realised by a predefined itinerary, non-ordered group of locations or single location."@en ;
  rdfs:label "Predefined location reference"@en .

<http://datex2.eu/vocab/3/LocationReferencing/PredefinedLocation>
  a owl:Class ;
  rdfs:comment "An identifiable versioned instance of a single predefined location."@en ;
  rdfs:label "Predefined location"@en ;
  rdfs:subClassOf <http://datex2.eu/vocab/3/LocationReferencing/PredefinedLocationReference> .

<http://datex2.eu/vocab/3/LocationReferencing/PredefinedLocationGroup>
  a owl:Class ;
  rdfs:comment "An identifiable versioned instance of a predefined group of non-ordered locations (i.e. more than one)."@en ;
  rdfs:label "Predefined location group"@en ;
  rdfs:subClassOf <http://datex2.eu/vocab/3/LocationReferencing/PredefinedLocationReference> .

<http://datex2.eu/vocab/3/LocationReferencing/PredefinedLocationsPublication>
  a owl:Class ;
  rdfs:comment "A publication containing one or more groups of predefined locations organised either as itineraries, non-ordered groups or as individual locations."@en ;
  rdfs:label "Predefined locations publication"@en ;
  rdfs:subClassOf <http://datex2.eu/vocab/3/Common/PayloadPublication> .

<http://datex2.eu/vocab/3/LocationReferencing/areasAtWhichApplicable>
  a owl:DatatypeProperty ;
  rdfs:comment "Places, in generic terms, at which the corresponding information applies."@en ;
  rdfs:domain <http://datex2.eu/vocab/3/LocationReferencing/AreaLocation> ;
  rdfs:label "Areas at which applicable"@en ;
  rdfs:range <http://datex2.eu/vocab/3/LocationReferencing/AreaPlacesEnum> .

<http://datex2.eu/vocab/3/LocationReferencing/externalLocationCode>
  a owl:DatatypeProperty ;
  rdfs:comment "A code in the external referencing system which defines the location."@en ;
  rdfs:domain <http://datex2.eu/vocab/3/LocationReferencing/ExternalReferencing> ;
  rdfs:label "External location code"@en ;
  rdfs:range <http://datex2.eu/vocab/3/Common/String> .

<http://datex2.eu/vocab/3/LocationReferencing/externalReferencingSystem>
  a owl:DatatypeProperty ;
  rdfs:comment "Identification of the external/other location referencing system."@en ;
  rdfs:domain <http://datex2.eu/vocab/3/LocationReferencing/ExternalReferencing> ;
  rdfs:label "External referencing system"@en ;
  rdfs:range <http://datex2.eu/vocab/3/Common/String> .

<http://datex2.eu/vocab/3/LocationReferencing/predefinedItineraryReference>
  a owl:DatatypeProperty ;
  rdfs:comment "A reference to a versioned instance of a predefined itinerary as specified in a PredefinedLocationsPublication."@en ;
  rdfs:domain <http://datex2.eu/vocab/3/LocationReferencing/ItineraryByReference> ;
  rdfs:label "Predefined itinerary reference"@en ;
  rdfs:range <http://datex2.eu/vocab/3/Common/VersionedReference> .

<http://datex2.eu/vocab/3/LocationReferencing/predefinedLocationReference>
  a owl:DatatypeProperty ;
  rdfs:comment "A reference to a versioned predefined location."@en ;
  rdfs:domain <http://datex2.eu/vocab/3/LocationReferencing/LocationByReference> ;
  rdfs:label "Predefined location reference"@en ;
  rdfs:range <http://datex2.eu/vocab/3/Common/VersionedReference> .

<http://datex2.eu/vocab/3/LocationReferencing/predefinedLocationGroupReference>
  a owl:DatatypeProperty ;
  rdfs:comment "A reference to a versioned instance of a predefined location group as specified in a PredefinedLocationsPublication."@en ;
  rdfs:domain <http://datex2.eu/vocab/3/LocationReferencing/LocationGroupByReference> ;
  rdfs:label "Predefined location group reference"@en ;
  rdfs:range <http://datex2.eu/vocab/3/Common/VersionedReference> .

<http://datex2.eu/vocab/3/LocationReferencing/offsetDistance>
  a owl:DatatypeProperty ;
  rdfs:comment "The non-negative offset distance from the ALERT-C referenced point to the actual point. The ALERT-C locations in the primary and secondary locations must always encompass the linear section being specified, thus offset distance is towards the other point."@en ;
  rdfs:domain <http://datex2.eu/vocab/3/LocationReferencing/OffsetDistance> ;
  rdfs:label "Offset distance"@en ;
  rdfs:range <http://datex2.eu/vocab/3/Common/MetresAsNonNegativeInteger> .

<http://datex2.eu/vocab/3/LocationReferencing/alertCLocationCountryCode>
  a owl:DatatypeProperty ;
  rdfs:comment "ALERT-C country code as defined in IEC 62106."@en, "ALERT-C country code as defined IEC 62106."@en ;
  rdfs:domain <http://datex2.eu/vocab/3/LocationReferencing/AlertCLinear>, <http://datex2.eu/vocab/3/LocationReferencing/AlertCPoint>, <http://datex2.eu/vocab/3/LocationReferencing/AlertCArea> ;
  rdfs:label "ALERT-C location country code"@en ;
  rdfs:range <http://datex2.eu/vocab/3/Common/String> .

<http://datex2.eu/vocab/3/LocationReferencing/alertCLocationTableNumber>
  a owl:DatatypeProperty ;
  rdfs:comment "Number allocated to an ALERT-C table in a country. Ref. EN ISO 14819-3 for the allocation of a location table number."@en ;
  rdfs:domain <http://datex2.eu/vocab/3/LocationReferencing/AlertCLinear>, <http://datex2.eu/vocab/3/LocationReferencing/AlertCPoint>, <http://datex2.eu/vocab/3/LocationReferencing/AlertCArea> ;
  rdfs:label "ALERT-C location table number"@en ;
  rdfs:range <http://datex2.eu/vocab/3/Common/String> .

<http://datex2.eu/vocab/3/LocationReferencing/alertCLocationTableVersion>
  a owl:DatatypeProperty ;
  rdfs:comment "Version number associated with an ALERT-C table reference."@en ;
  rdfs:domain <http://datex2.eu/vocab/3/LocationReferencing/AlertCLinear>, <http://datex2.eu/vocab/3/LocationReferencing/AlertCPoint>, <http://datex2.eu/vocab/3/LocationReferencing/AlertCArea> ;
  rdfs:label "ALERT-C location table version"@en ;
  rdfs:range <http://datex2.eu/vocab/3/Common/String> .

<http://datex2.eu/vocab/3/LocationReferencing/alertCAffectedDirection>
  a owl:DatatypeProperty ;
  rdfs:comment "The direction(s) of traffic flow to which the situation, traffic data or information is related."@en ;
  rdfs:domain <http://datex2.eu/vocab/3/LocationReferencing/AlertCDirection> ;
  rdfs:label "ALERT-C affected direction"@en ;
  rdfs:range <http://datex2.eu/vocab/3/LocationReferencing/LinearDirectionEnum> .

<http://datex2.eu/vocab/3/LocationReferencing/alertCDirectionCoded>
  a owl:DatatypeProperty ;
  rdfs:comment "Direction of navigation with respect to secondary to primary location (RDS direction)"@en ;
  rdfs:domain <http://datex2.eu/vocab/3/LocationReferencing/AlertCDirection> ;
  rdfs:label "ALERT-C direction coded"@en ;
  rdfs:range <http://datex2.eu/vocab/3/LocationReferencing/AlertCDirectionEnum> .

<http://datex2.eu/vocab/3/LocationReferencing/alertCDirectionNamed>
  a owl:DatatypeProperty ;
  rdfs:comment "ALERT-C name of a direction e.g. Brussels -> Lille."@en ;
  rdfs:domain <http://datex2.eu/vocab/3/LocationReferencing/AlertCDirection> ;
  rdfs:label "ALERT-C direction named"@en ;
  rdfs:range <http://datex2.eu/vocab/3/Common/MultilingualString> .

<http://datex2.eu/vocab/3/LocationReferencing/alertCLocationName>
  a owl:DatatypeProperty ;
  rdfs:comment "Name of ALERT-C location."@en ;
  rdfs:domain <http://datex2.eu/vocab/3/LocationReferencing/AlertCLocation> ;
  rdfs:label "ALERT-C location name"@en ;
  rdfs:range <http://datex2.eu/vocab/3/Common/MultilingualString> .

<http://datex2.eu/vocab/3/LocationReferencing/specificLocation>
  a owl:DatatypeProperty ;
  rdfs:comment "Unique code within the ALERT-C location table which identifies the specific point, linear or area location."@en ;
  rdfs:domain <http://datex2.eu/vocab/3/LocationReferencing/AlertCLocation> ;
  rdfs:label "Specific location"@en ;
  rdfs:range <http://datex2.eu/vocab/3/LocationReferencing/AlertCLocationCode> .

<http://datex2.eu/vocab/3/LocationReferencing/posList>
  a owl:DatatypeProperty ;
  rdfs:comment "List of coordinate tuples define the geometry of this GmlLineString. There must be at least 2 tuples of coordinates. Form depends on coordinate reference system; typical form is space-separated pairs of latitude and longitude."@en ;
  rdfs:domain <http://datex2.eu/vocab/3/LocationReferencing/GmlLineString> ;
  rdfs:label "Pos list"@en ;
  rdfs:range <http://datex2.eu/vocab/3/LocationReferencing/GmlPosList> .

<http://datex2.eu/vocab/3/LocationReferencing/srsDimension>
  a owl:DatatypeProperty ;
  rdfs:comment "Provides the size of the tuple of coordinates of each point. This number is 2 or 3. By default when omitted the dimension shall be interpreted as 2."@en ;
  rdfs:domain <http://datex2.eu/vocab/3/LocationReferencing/GmlLineString> ;
  rdfs:label "Srs dimension"@en ;
  rdfs:range <http://datex2.eu/vocab/3/Common/NonNegativeInteger> .

<http://datex2.eu/vocab/3/LocationReferencing/srsName>
  a owl:DatatypeProperty ;
  rdfs:comment "Specifies the Coordinate Reference System (CRS) used to interpret the coordinates in this GmlLineString"@en ;
  rdfs:domain <http://datex2.eu/vocab/3/LocationReferencing/GmlLineString> ;
  rdfs:label "Srs name"@en ;
  rdfs:range <http://datex2.eu/vocab/3/Common/String> .

<http://datex2.eu/vocab/3/LocationReferencing/gmlAreaName>
  a owl:DatatypeProperty ;
  rdfs:comment "Name of the multi-polygon area"@en ;
  rdfs:domain <http://datex2.eu/vocab/3/LocationReferencing/GmlMultiPolygon> ;
  rdfs:label "Gml area name"@en ;
  rdfs:range <http://datex2.eu/vocab/3/Common/MultilingualString> .

<http://datex2.eu/vocab/3/LocationReferencing/administrativeAreaOfLinearSection>
  a owl:DatatypeProperty ;
  rdfs:comment "Identification of the road administration area which contains the specified linear section."@en ;
  rdfs:domain <http://datex2.eu/vocab/3/LocationReferencing/LinearWithinLinearElement> ;
  rdfs:label "Administrative area of linear section"@en ;
  rdfs:range <http://datex2.eu/vocab/3/Common/MultilingualString> .

<http://datex2.eu/vocab/3/LocationReferencing/directionOnLinearSection>
  a owl:DatatypeProperty ;
  rdfs:comment "The direction of traffic flow on the linear section in terms of general destination direction."@en ;
  rdfs:domain <http://datex2.eu/vocab/3/LocationReferencing/LinearWithinLinearElement> ;
  rdfs:label "Direction on linear section"@en ;
  rdfs:range <http://datex2.eu/vocab/3/LocationReferencing/DirectionEnum> .

<http://datex2.eu/vocab/3/LocationReferencing/directionRelativeOnLinearSection>
  a owl:DatatypeProperty ;
  rdfs:comment "The direction of traffic flow on the linear section relative to the direction in which the linear element is defined."@en ;
  rdfs:domain <http://datex2.eu/vocab/3/LocationReferencing/LinearWithinLinearElement> ;
  rdfs:label "Direction relative on linear section"@en ;
  rdfs:range <http://datex2.eu/vocab/3/LocationReferencing/LinearDirectionEnum> .

<http://datex2.eu/vocab/3/LocationReferencing/heightGradeOfLinearSection>
  a owl:DatatypeProperty ;
  rdfs:comment "Identification of whether the linear section that is part of the linear element is at, above or below the normal elevation of a linear element of that type (e.g. road or road section) at that location, typically used to indicate \"grade\" separation."@en ;
  rdfs:domain <http://datex2.eu/vocab/3/LocationReferencing/LinearWithinLinearElement> ;
  rdfs:label "Height grade of linear section"@en ;
  rdfs:range <http://datex2.eu/vocab/3/LocationReferencing/HeightGradeEnum> .

<http://datex2.eu/vocab/3/LocationReferencing/distanceAlong>
  a owl:DatatypeProperty ;
  rdfs:comment "A measure of distance along a linear element."@en ;
  rdfs:domain <http://datex2.eu/vocab/3/LocationReferencing/DistanceFromLinearElementReferent>, <http://datex2.eu/vocab/3/LocationReferencing/DistanceFromLinearElementStart> ;
  rdfs:label "Distance along"@en ;
  rdfs:range <http://datex2.eu/vocab/3/Common/MetresAsFloat> .

<http://datex2.eu/vocab/3/LocationReferencing/linearElementNature>
  a owl:DatatypeProperty ;
  rdfs:comment "An indication of the nature of the linear element."@en ;
  rdfs:domain <http://datex2.eu/vocab/3/LocationReferencing/LinearElement> ;
  rdfs:label "Linear element nature"@en ;
  rdfs:range <http://datex2.eu/vocab/3/LocationReferencing/LinearElementNatureEnum> .

<http://datex2.eu/vocab/3/LocationReferencing/linearElementReferenceModel>
  a owl:DatatypeProperty ;
  rdfs:comment "The identifier of a road network reference model which segments the road network according to specific business rules."@en ;
  rdfs:domain <http://datex2.eu/vocab/3/LocationReferencing/LinearElement> ;
  rdfs:label "Linear element reference model"@en ;
  rdfs:range <http://datex2.eu/vocab/3/Common/String> .

<http://datex2.eu/vocab/3/LocationReferencing/linearElementReferenceModelVersion>
  a owl:DatatypeProperty ;
  rdfs:comment "The version of the identified road network reference model."@en ;
  rdfs:domain <http://datex2.eu/vocab/3/LocationReferencing/LinearElement> ;
  rdfs:label "Linear element reference model version"@en ;
  rdfs:range <http://datex2.eu/vocab/3/Common/String> .

<http://datex2.eu/vocab/3/LocationReferencing/roadName>
  a owl:DatatypeProperty ;
  rdfs:comment "Name of the road"@en, "The name of the road"@en ;
  rdfs:domain <http://datex2.eu/vocab/3/LocationReferencing/LinearElement>, <http://datex2.eu/vocab/3/LocationReferencing/RoadInformation> ;
  rdfs:label "Road name"@en ;
  rdfs:range <http://datex2.eu/vocab/3/Common/MultilingualString>, <http://datex2.eu/vocab/3/Common/String> .

<http://datex2.eu/vocab/3/LocationReferencing/roadNumber>
  a owl:DatatypeProperty ;
  rdfs:comment "Identifier/number of the road"@en, "The road number designated by the road authority"@en ;
  rdfs:domain <http://datex2.eu/vocab/3/LocationReferencing/LinearElement>, <http://datex2.eu/vocab/3/LocationReferencing/RoadInformation> ;
  rdfs:label "Road number"@en ;
  rdfs:range <http://datex2.eu/vocab/3/Common/String> .

<http://datex2.eu/vocab/3/LocationReferencing/linearElementIdentifier>
  a owl:DatatypeProperty ;
  rdfs:comment "An identifier or code of a linear element (or link) in the road network reference model that is specified in the LinearElement class. "@en ;
  rdfs:domain <http://datex2.eu/vocab/3/LocationReferencing/LinearElementByCode> ;
  rdfs:label "Linear element identifier"@en ;
  rdfs:range <http://datex2.eu/vocab/3/Common/String> .

<http://datex2.eu/vocab/3/LocationReferencing/percentageDistanceAlong>
  a owl:DatatypeProperty ;
  rdfs:comment "A measure of distance along a linear element from the start of the element expressed as a percentage of the total length of the linear object."@en ;
  rdfs:domain <http://datex2.eu/vocab/3/LocationReferencing/PercentageDistanceAlongLinearElement> ;
  rdfs:label "Percentage distance along"@en ;
  rdfs:range <http://datex2.eu/vocab/3/Common/Percentage> .

<http://datex2.eu/vocab/3/LocationReferencing/administrativeAreaOfPoint>
  a owl:DatatypeProperty ;
  rdfs:comment "Identification of the road administration area which contains the specified point."@en ;
  rdfs:domain <http://datex2.eu/vocab/3/LocationReferencing/PointAlongLinearElement> ;
  rdfs:label "Administrative area of point"@en ;
  rdfs:range <http://datex2.eu/vocab/3/Common/MultilingualString> .

<http://datex2.eu/vocab/3/LocationReferencing/directionAtPoint>
  a owl:DatatypeProperty ;
  rdfs:comment "The direction of traffic flow at the specified point in terms of general destination direction."@en ;
  rdfs:domain <http://datex2.eu/vocab/3/LocationReferencing/PointAlongLinearElement> ;
  rdfs:label "Direction at point"@en ;
  rdfs:range <http://datex2.eu/vocab/3/LocationReferencing/DirectionEnum> .

<http://datex2.eu/vocab/3/LocationReferencing/directionRelativeAtPoint>
  a owl:DatatypeProperty ;
  rdfs:comment "The direction of traffic flow at the specified point relative to the direction in which the linear element is defined."@en ;
  rdfs:domain <http://datex2.eu/vocab/3/LocationReferencing/PointAlongLinearElement> ;
  rdfs:label "Direction relative at point"@en ;
  rdfs:range <http://datex2.eu/vocab/3/LocationReferencing/LinearDirectionEnum> .

<http://datex2.eu/vocab/3/LocationReferencing/heightGradeOfPoint>
  a owl:DatatypeProperty ;
  rdfs:comment "Identification of whether the point on the linear element is at, above or below the normal elevation of a linear element of that type (e.g. road or road section) at that location, typically used to indicate \"grade\" separation."@en ;
  rdfs:domain <http://datex2.eu/vocab/3/LocationReferencing/PointAlongLinearElement> ;
  rdfs:label "Height grade of point"@en ;
  rdfs:range <http://datex2.eu/vocab/3/LocationReferencing/HeightGradeEnum> .

<http://datex2.eu/vocab/3/LocationReferencing/referentDescription>
  a owl:DatatypeProperty ;
  rdfs:comment "Description of the referent."@en ;
  rdfs:domain <http://datex2.eu/vocab/3/LocationReferencing/Referent> ;
  rdfs:label "Referent description"@en ;
  rdfs:range <http://datex2.eu/vocab/3/Common/MultilingualString> .

<http://datex2.eu/vocab/3/LocationReferencing/referentIdentifier>
  a owl:DatatypeProperty ;
  rdfs:comment "The identifier of the referent, unique on the specified linear element (i.e. road or part of)."@en ;
  rdfs:domain <http://datex2.eu/vocab/3/LocationReferencing/Referent> ;
  rdfs:label "Referent identifier"@en ;
  rdfs:range <http://datex2.eu/vocab/3/Common/String> .

<http://datex2.eu/vocab/3/LocationReferencing/referentName>
  a owl:DatatypeProperty ;
  rdfs:comment "The name of the referent, e.g. a junction or intersection name."@en ;
  rdfs:domain <http://datex2.eu/vocab/3/LocationReferencing/Referent> ;
  rdfs:label "Referent name"@en ;
  rdfs:range <http://datex2.eu/vocab/3/Common/String> .

<http://datex2.eu/vocab/3/LocationReferencing/referentType>
  a owl:DatatypeProperty ;
  rdfs:comment "The type of the referent."@en ;
  rdfs:domain <http://datex2.eu/vocab/3/LocationReferencing/Referent> ;
  rdfs:label "Referent type"@en ;
  rdfs:range <http://datex2.eu/vocab/3/LocationReferencing/ReferentTypeEnum> .

<http://datex2.eu/vocab/3/LocationReferencing/altitudeAccuracyCodedError>
  a owl:DatatypeProperty ;
  rdfs:comment "Error code in case the altitude confidence is out of range or cannot be determined"@en ;
  rdfs:domain <http://datex2.eu/vocab/3/LocationReferencing/AltitudeConfidence> ;
  rdfs:label "Altitude accuracy coded error"@en ;
  rdfs:range <http://datex2.eu/vocab/3/LocationReferencing/PositionConfidenceCodedErrorEnum> .

<http://datex2.eu/vocab/3/LocationReferencing/altitudeAccuracyCodedValue>
  a owl:DatatypeProperty ;
  rdfs:comment "Absolute accuracy of reported value of a geographical point for a confidence level expressed by a coded scale."@en ;
  rdfs:domain <http://datex2.eu/vocab/3/LocationReferencing/AltitudeConfidence> ;
  rdfs:label "Altitude accuracy coded value"@en ;
  rdfs:range <http://datex2.eu/vocab/3/LocationReferencing/AltitudeAccuracyEnum> .

<http://datex2.eu/vocab/3/LocationReferencing/heightType>
  a owl:DatatypeProperty ;
  rdfs:comment "Type of measured height.When it is omitted it is supposed to be the ellipsoidal height."@en, "A descriptive identification of relative height using TPEG-Loc location referencing."@en ;
  rdfs:domain <http://datex2.eu/vocab/3/LocationReferencing/HeightCoordinate>, <http://datex2.eu/vocab/3/LocationReferencing/TpegHeight> ;
  rdfs:label "Height type"@en ;
  rdfs:range <http://datex2.eu/vocab/3/LocationReferencing/HeightTypeEnum>, <http://datex2.eu/vocab/3/LocationReferencing/TpegLoc04HeightTypeEnum> .

<http://datex2.eu/vocab/3/LocationReferencing/heightValue>
  a owl:DatatypeProperty ;
  rdfs:comment "Value in metres for the height measured vertically at to the planar coordinates the point corresponding."@en ;
  rdfs:domain <http://datex2.eu/vocab/3/LocationReferencing/HeightCoordinate> ;
  rdfs:label "Height value"@en ;
  rdfs:range <http://datex2.eu/vocab/3/Common/MetresAsFloat> .

<http://datex2.eu/vocab/3/LocationReferencing/bearing>
  a owl:DatatypeProperty ;
  rdfs:comment "A bearing at the point measured in degrees (0 - 359). Unless otherwise specified the reference direction corresponding to 0 degrees is North."@en ;
  rdfs:domain <http://datex2.eu/vocab/3/LocationReferencing/PointByCoordinates> ;
  rdfs:label "Bearing"@en ;
  rdfs:range <http://datex2.eu/vocab/3/Common/AngleInDegrees> .

<http://datex2.eu/vocab/3/LocationReferencing/accuracyPercentile50>
  a owl:DatatypeProperty ;
  rdfs:comment "Accuracy defined by the 50th percentile of the cumulative distribution of position errors."@en ;
  rdfs:domain <http://datex2.eu/vocab/3/LocationReferencing/PositionAccuracy> ;
  rdfs:label "Accuracy percentile50"@en ;
  rdfs:range <http://datex2.eu/vocab/3/Common/MetresAsFloat> .

<http://datex2.eu/vocab/3/LocationReferencing/accuracyPercentile75>
  a owl:DatatypeProperty ;
  rdfs:comment "Accuracy defined by the 75th percentile of the cumulative distribution of position errors"@en ;
  rdfs:domain <http://datex2.eu/vocab/3/LocationReferencing/PositionAccuracy> ;
  rdfs:label "Accuracy percentile75"@en ;
  rdfs:range <http://datex2.eu/vocab/3/Common/MetresAsFloat> .

<http://datex2.eu/vocab/3/LocationReferencing/accuracyPercentile95>
  a owl:DatatypeProperty ;
  rdfs:comment "Accuracy defined by the 95th percentile of the cumulative distribution of position errors"@en ;
  rdfs:domain <http://datex2.eu/vocab/3/LocationReferencing/PositionAccuracy> ;
  rdfs:label "Accuracy percentile95"@en ;
  rdfs:range <http://datex2.eu/vocab/3/Common/MetresAsFloat> .

<http://datex2.eu/vocab/3/LocationReferencing/semiMajorAxisLength>
  a owl:DatatypeProperty ;
  rdfs:comment "Half of length of the major axis, i.e. distance between the centre point and major axis point of the position accuracy ellipse."@en ;
  rdfs:domain <http://datex2.eu/vocab/3/LocationReferencing/PositionConfidenceEllipse> ;
  rdfs:label "Semi major axis length"@en ;
  rdfs:range <http://datex2.eu/vocab/3/Common/MetresAsFloat> .

<http://datex2.eu/vocab/3/LocationReferencing/semiMajorAxisLengthCodedError>
  a owl:DatatypeProperty ;
  rdfs:comment "Provides a coded error in case the semi-major axis length is not defined"@en ;
  rdfs:domain <http://datex2.eu/vocab/3/LocationReferencing/PositionConfidenceEllipse> ;
  rdfs:label "Semi major axis length coded error"@en ;
  rdfs:range <http://datex2.eu/vocab/3/LocationReferencing/PositionConfidenceCodedErrorEnum> .

<http://datex2.eu/vocab/3/LocationReferencing/semiMajorAxisOrientation>
  a owl:DatatypeProperty ;
  rdfs:comment "Orientation direction of the ellipse major axis of the position accuracy ellipse with regards to the geographic north."@en ;
  rdfs:domain <http://datex2.eu/vocab/3/LocationReferencing/PositionConfidenceEllipse> ;
  rdfs:label "Semi major axis orientation"@en ;
  rdfs:range <http://datex2.eu/vocab/3/Common/AngleInDegrees> .

<http://datex2.eu/vocab/3/LocationReferencing/semiMajorAxisOrientationError>
  a owl:DatatypeProperty ;
  rdfs:comment "Indicates whether the ellipse orientation is unavailable (True) or not (False)"@en ;
  rdfs:domain <http://datex2.eu/vocab/3/LocationReferencing/PositionConfidenceEllipse> ;
  rdfs:label "Semi major axis orientation error"@en ;
  rdfs:range <http://datex2.eu/vocab/3/Common/Boolean> .

<http://datex2.eu/vocab/3/LocationReferencing/semiMinorAxisLength>
  a owl:DatatypeProperty ;
  rdfs:comment "Half of length of the minor axis, i.e. distance between the centre point and minor axis point of the position accuracy ellipse"@en ;
  rdfs:domain <http://datex2.eu/vocab/3/LocationReferencing/PositionConfidenceEllipse> ;
  rdfs:label "Semi minor axis length"@en ;
  rdfs:range <http://datex2.eu/vocab/3/Common/MetresAsFloat> .

<http://datex2.eu/vocab/3/LocationReferencing/semiMinorAxisLengthCodedError>
  a owl:DatatypeProperty ;
  rdfs:comment "Provides a coded error in case the semi-minor axis length is not defined"@en ;
  rdfs:domain <http://datex2.eu/vocab/3/LocationReferencing/PositionConfidenceEllipse> ;
  rdfs:label "Semi minor axis length coded error"@en ;
  rdfs:range <http://datex2.eu/vocab/3/LocationReferencing/PositionConfidenceCodedErrorEnum> .

<http://datex2.eu/vocab/3/LocationReferencing/latitude>
  a owl:DatatypeProperty ;
  rdfs:comment "Latitude in decimal degrees using the European Terrestrial Reference System 1989 (ETRS89)."@en ;
  rdfs:domain <http://datex2.eu/vocab/3/LocationReferencing/PointCoordinates> ;
  rdfs:label "Latitude"@en ;
  rdfs:range <http://datex2.eu/vocab/3/Common/Float> .

<http://datex2.eu/vocab/3/LocationReferencing/longitude>
  a owl:DatatypeProperty ;
  rdfs:comment "Longitude in decimal degrees using the European Terrestrial Reference System 1989 (ETRS89)."@en ;
  rdfs:domain <http://datex2.eu/vocab/3/LocationReferencing/PointCoordinates> ;
  rdfs:label "Longitude"@en ;
  rdfs:range <http://datex2.eu/vocab/3/Common/Float> .

<http://datex2.eu/vocab/3/LocationReferencing/laneNumber>
  a owl:DatatypeProperty ;
  rdfs:comment "The number of the lane, where 1 is nearest the hard shoulder/verge and the numbers increase towards the central reservation/road axis."@en ;
  rdfs:domain <http://datex2.eu/vocab/3/LocationReferencing/Lane> ;
  rdfs:label "Lane number"@en ;
  rdfs:range <http://datex2.eu/vocab/3/Common/Integer> .

<http://datex2.eu/vocab/3/LocationReferencing/laneUsage>
  a owl:DatatypeProperty ;
  rdfs:comment "Indicates the specific lane to which the location relates."@en ;
  rdfs:domain <http://datex2.eu/vocab/3/LocationReferencing/Lane> ;
  rdfs:label "Lane usage"@en ;
  rdfs:range <http://datex2.eu/vocab/3/LocationReferencing/LaneEnum> .

<http://datex2.eu/vocab/3/LocationReferencing/roadDestination>
  a owl:DatatypeProperty ;
  rdfs:comment "A destination associated with this road."@en ;
  rdfs:domain <http://datex2.eu/vocab/3/LocationReferencing/RoadInformation> ;
  rdfs:label "Road destination"@en ;
  rdfs:range <http://datex2.eu/vocab/3/Common/String> .

<http://datex2.eu/vocab/3/LocationReferencing/carriageway>
  a owl:DatatypeProperty ;
  rdfs:comment "Indicates the section of carriageway to which the location relates."@en ;
  rdfs:domain <http://datex2.eu/vocab/3/LocationReferencing/Carriageway> ;
  rdfs:label "Carriageway"@en ;
  rdfs:range <http://datex2.eu/vocab/3/LocationReferencing/CarriagewayEnum> .

<http://datex2.eu/vocab/3/LocationReferencing/originalNumberOfLanes>
  a owl:DatatypeProperty ;
  rdfs:comment "Normal number of lanes, potentially available for moving traffic, before reduction due to situations. Hard shoulder should not be counted unless it is sometimes used operationally for moving traffic."@en ;
  rdfs:domain <http://datex2.eu/vocab/3/LocationReferencing/Carriageway> ;
  rdfs:label "Original number of lanes"@en ;
  rdfs:range <http://datex2.eu/vocab/3/Common/Integer> .

<http://datex2.eu/vocab/3/LocationReferencing/directionPurpose>
  a owl:DatatypeProperty ;
  rdfs:comment "Identifies the main purpose of the road at the location"@en ;
  rdfs:domain <http://datex2.eu/vocab/3/LocationReferencing/SupplementaryPositionalDescription> ;
  rdfs:label "Direction purpose"@en ;
  rdfs:range <http://datex2.eu/vocab/3/LocationReferencing/DirectionPurposeEnum> .

<http://datex2.eu/vocab/3/LocationReferencing/geographicDescriptor>
  a owl:DatatypeProperty ;
  rdfs:comment "Descriptor which identifies a geographic characteristic to help identify the specific location"@en ;
  rdfs:domain <http://datex2.eu/vocab/3/LocationReferencing/SupplementaryPositionalDescription> ;
  rdfs:label "Geographic descriptor"@en ;
  rdfs:range <http://datex2.eu/vocab/3/LocationReferencing/GeographicCharacteristicEnum> .

<http://datex2.eu/vocab/3/LocationReferencing/infrastructureDescriptor>
  a owl:DatatypeProperty ;
  rdfs:comment "Descriptor which identifies infrastructure to help identify the specific location."@en ;
  rdfs:domain <http://datex2.eu/vocab/3/LocationReferencing/SupplementaryPositionalDescription> ;
  rdfs:label "Infrastructure descriptor"@en ;
  rdfs:range <http://datex2.eu/vocab/3/LocationReferencing/InfrastructureDescriptorEnum> .

<http://datex2.eu/vocab/3/LocationReferencing/lengthAffected>
  a owl:DatatypeProperty ;
  rdfs:comment "This indicates the length (measured in metres) of carriageway (and lanes) affected by the associated traffic element."@en ;
  rdfs:domain <http://datex2.eu/vocab/3/LocationReferencing/SupplementaryPositionalDescription> ;
  rdfs:label "Length affected"@en ;
  rdfs:range <http://datex2.eu/vocab/3/Common/MetresAsFloat> .

<http://datex2.eu/vocab/3/LocationReferencing/locationDescription>
  a owl:DatatypeProperty ;
  rdfs:comment "Supplementary human-readable description of the location"@en ;
  rdfs:domain <http://datex2.eu/vocab/3/LocationReferencing/SupplementaryPositionalDescription> ;
  rdfs:label "Location description"@en ;
  rdfs:range <http://datex2.eu/vocab/3/Common/MultilingualString> .

<http://datex2.eu/vocab/3/LocationReferencing/locationPrecision>
  a owl:DatatypeProperty ;
  rdfs:comment "Indicates that the location is given with a precision which is better than the stated value in metres."@en ;
  rdfs:domain <http://datex2.eu/vocab/3/LocationReferencing/SupplementaryPositionalDescription> ;
  rdfs:label "Location precision"@en ;
  rdfs:range <http://datex2.eu/vocab/3/Common/MetresAsNonNegativeInteger> .

<http://datex2.eu/vocab/3/LocationReferencing/positionOnCarriageway>
  a owl:DatatypeProperty ;
  rdfs:comment "Relative position across carriageway"@en ;
  rdfs:domain <http://datex2.eu/vocab/3/LocationReferencing/SupplementaryPositionalDescription> ;
  rdfs:label "Position on carriageway"@en ;
  rdfs:range <http://datex2.eu/vocab/3/LocationReferencing/RelativePositionOnCarriagewayEnum> .

<http://datex2.eu/vocab/3/LocationReferencing/sequentialRampNumber>
  a owl:DatatypeProperty ;
  rdfs:comment "The sequential number of an exit/entrance ramp from a given location in a given direction (normally used to indicate a specific exit/entrance in a complex junction/intersection)."@en ;
  rdfs:domain <http://datex2.eu/vocab/3/LocationReferencing/SupplementaryPositionalDescription> ;
  rdfs:label "Sequential ramp number"@en ;
  rdfs:range <http://datex2.eu/vocab/3/Common/NonNegativeInteger> .

<http://datex2.eu/vocab/3/LocationReferencing/tpegAreaLocationType>
  a owl:DatatypeProperty ;
  rdfs:comment "The type of TPEG location."@en ;
  rdfs:domain <http://datex2.eu/vocab/3/LocationReferencing/TpegAreaLocation> ;
  rdfs:label "TPEG area location type"@en ;
  rdfs:range <http://datex2.eu/vocab/3/LocationReferencing/TpegLoc01AreaLocationSubtypeEnum> .

<http://datex2.eu/vocab/3/LocationReferencing/radius>
  a owl:DatatypeProperty ;
  rdfs:comment "The radius of the corresponding circular area"@en ;
  rdfs:domain <http://datex2.eu/vocab/3/LocationReferencing/TpegGeometricArea> ;
  rdfs:label "Radius"@en ;
  rdfs:range <http://datex2.eu/vocab/3/Common/MetresAsNonNegativeInteger> .

<http://datex2.eu/vocab/3/LocationReferencing/height>
  a owl:DatatypeProperty ;
  rdfs:comment "A measurement of height in metres"@en ;
  rdfs:domain <http://datex2.eu/vocab/3/LocationReferencing/TpegHeight> ;
  rdfs:label "Height"@en ;
  rdfs:range <http://datex2.eu/vocab/3/Common/MetresAsFloat> .

<http://datex2.eu/vocab/3/LocationReferencing/tpegAreaDescriptorType>
  a owl:DatatypeProperty ;
  rdfs:comment "The nature of the descriptor used to define the location under consideration (derived from the TPEG Loc table 03)."@en ;
  rdfs:domain <http://datex2.eu/vocab/3/LocationReferencing/TpegAreaDescriptor> ;
  rdfs:label "TPEG area descriptor type"@en ;
  rdfs:range <http://datex2.eu/vocab/3/LocationReferencing/TpegLoc03AreaDescriptorSubtypeEnum> .

<http://datex2.eu/vocab/3/LocationReferencing/descriptor>
  a owl:DatatypeProperty ;
  rdfs:comment "A text string which describes or elaborates the location."@en ;
  rdfs:domain <http://datex2.eu/vocab/3/LocationReferencing/TpegDescriptor> ;
  rdfs:label "Descriptor"@en ;
  rdfs:range <http://datex2.eu/vocab/3/Common/MultilingualString> .

<http://datex2.eu/vocab/3/LocationReferencing/tpegIlcPointDescriptorType>
  a owl:DatatypeProperty ;
  rdfs:comment "The nature of the descriptor used to define the location under consideration (derived from the TPEG Loc table 03)."@en ;
  rdfs:domain <http://datex2.eu/vocab/3/LocationReferencing/TpegIlcPointDescriptor> ;
  rdfs:label "TPEG ILC point descriptor type"@en ;
  rdfs:range <http://datex2.eu/vocab/3/LocationReferencing/TpegLoc03IlcPointDescriptorSubtypeEnum> .

<http://datex2.eu/vocab/3/LocationReferencing/tpegJunctionPointDescriptorType>
  a owl:DatatypeProperty ;
  rdfs:comment "The nature of the descriptor used to define the location under consideration (derived from the TPEG Loc table 03)."@en ;
  rdfs:domain <http://datex2.eu/vocab/3/LocationReferencing/TpegJunctionPointDescriptor> ;
  rdfs:label "TPEG junction point descriptor type"@en ;
  rdfs:range <http://datex2.eu/vocab/3/LocationReferencing/TpegLoc03JunctionPointDescriptorSubtypeEnum> .

<http://datex2.eu/vocab/3/LocationReferencing/tpegOtherPointDescriptorType>
  a owl:DatatypeProperty ;
  rdfs:comment "The nature of the descriptor used to define the location under consideration (derived from the TPEG Loc table 03)."@en ;
  rdfs:domain <http://datex2.eu/vocab/3/LocationReferencing/TpegOtherPointDescriptor> ;
  rdfs:label "TPEG other point descriptor type"@en ;
  rdfs:range <http://datex2.eu/vocab/3/LocationReferencing/TpegLoc03OtherPointDescriptorSubtypeEnum> .

<http://datex2.eu/vocab/3/LocationReferencing/tpegDirection>
  a owl:DatatypeProperty ;
  rdfs:comment "The direction of traffic flow."@en ;
  rdfs:domain <http://datex2.eu/vocab/3/LocationReferencing/TpegLinearLocation>, <http://datex2.eu/vocab/3/LocationReferencing/TpegPointLocation> ;
  rdfs:label "TPEG direction"@en ;
  rdfs:range <http://datex2.eu/vocab/3/LocationReferencing/DirectionEnum> .

<http://datex2.eu/vocab/3/LocationReferencing/tpegLinearLocationType>
  a owl:DatatypeProperty ;
  rdfs:comment "The type of TPEG location."@en ;
  rdfs:domain <http://datex2.eu/vocab/3/LocationReferencing/TpegLinearLocation> ;
  rdfs:label "TPEG linear location type"@en ;
  rdfs:range <http://datex2.eu/vocab/3/LocationReferencing/TpegLoc01LinearLocationSubtypeEnum> .

<http://datex2.eu/vocab/3/LocationReferencing/tpegFramedPointLocationType>
  a owl:DatatypeProperty ;
  rdfs:comment "The type of TPEG location."@en ;
  rdfs:domain <http://datex2.eu/vocab/3/LocationReferencing/TpegFramedPoint> ;
  rdfs:label "TPEG framed point location type"@en ;
  rdfs:range <http://datex2.eu/vocab/3/LocationReferencing/TpegLoc01FramedPointLocationSubtypeEnum> .

<http://datex2.eu/vocab/3/LocationReferencing/tpegSimplePointLocationType>
  a owl:DatatypeProperty ;
  rdfs:comment "The type of TPEG location."@en ;
  rdfs:domain <http://datex2.eu/vocab/3/LocationReferencing/TpegSimplePoint> ;
  rdfs:label "TPEG simple point location type"@en ;
  rdfs:range <http://datex2.eu/vocab/3/LocationReferencing/TpegLoc01SimplePointLocationSubtypeEnum> .

<http://datex2.eu/vocab/3/LocationReferencing/openlrBearing>
  a owl:DatatypeProperty ;
  rdfs:comment "defines the bearing field as an integer value between 0 and 359"@en ;
  rdfs:domain <http://datex2.eu/vocab/3/LocationReferencing/OpenlrLineAttributes> ;
  rdfs:label "Openlr bearing"@en ;
  rdfs:range <http://datex2.eu/vocab/3/Common/AngleInDegrees> .

<http://datex2.eu/vocab/3/LocationReferencing/openlrFormOfWay>
  a owl:DatatypeProperty ;
  rdfs:comment "A classification based on the importance of the role that the Road Element (or Ferry Connection) performs in the connectivity of the total road network. (EN ISO 14825 § 7.2.88)"@en ;
  rdfs:domain <http://datex2.eu/vocab/3/LocationReferencing/OpenlrLineAttributes> ;
  rdfs:label "Openlr form of way"@en ;
  rdfs:range <http://datex2.eu/vocab/3/LocationReferencing/OpenlrFormOfWayEnum> .

<http://datex2.eu/vocab/3/LocationReferencing/openlrFunctionalRoadClass>
  a owl:DatatypeProperty ;
  rdfs:comment "Certain aspects of the physical form that a Road Element takes. It is based on a number of certain physical and traffic properties. (EN ISO 14825 § 7.2.85)"@en ;
  rdfs:domain <http://datex2.eu/vocab/3/LocationReferencing/OpenlrLineAttributes> ;
  rdfs:label "Openlr functional road class"@en ;
  rdfs:range <http://datex2.eu/vocab/3/LocationReferencing/OpenlrFunctionalRoadClassEnum> .

<http://datex2.eu/vocab/3/LocationReferencing/openlrNegativeOffset>
  a owl:DatatypeProperty ;
  rdfs:comment "The negative offset along the line of the location measured along the line reference path between the end point of the location reference and the ending node of the line reference path."@en ;
  rdfs:domain <http://datex2.eu/vocab/3/LocationReferencing/OpenlrOffsets> ;
  rdfs:label "Openlr negative offset"@en ;
  rdfs:range <http://datex2.eu/vocab/3/Common/MetresAsNonNegativeInteger> .

<http://datex2.eu/vocab/3/LocationReferencing/openlrPositiveOffset>
  a owl:DatatypeProperty ;
  rdfs:comment "The positive offset along the line of the location measured along the line reference path between the start point of the location reference and the starting node of the line reference path."@en ;
  rdfs:domain <http://datex2.eu/vocab/3/LocationReferencing/OpenlrOffsets> ;
  rdfs:label "Openlr positive offset"@en ;
  rdfs:range <http://datex2.eu/vocab/3/Common/MetresAsNonNegativeInteger> .

<http://datex2.eu/vocab/3/LocationReferencing/openlrDistanceToNextLRPoint>
  a owl:DatatypeProperty ;
  rdfs:comment "The DNP attribute measures the distance in meters between two consecutive location reference-points along the location reference path described in the corresponding enumeration"@en ;
  rdfs:domain <http://datex2.eu/vocab/3/LocationReferencing/OpenlrPathAttributes> ;
  rdfs:label "Openlr distance to next l r point"@en ;
  rdfs:range <http://datex2.eu/vocab/3/Common/NonNegativeInteger> .

<http://datex2.eu/vocab/3/LocationReferencing/openlrLowestFrcToNextLRPoint>
  a owl:DatatypeProperty ;
  rdfs:comment "The lowest FRC to the next point indicates the lowest functional road class used in the location reference path to the next LR-point."@en ;
  rdfs:domain <http://datex2.eu/vocab/3/LocationReferencing/OpenlrPathAttributes> ;
  rdfs:label "Openlr lowest frc to next l r point"@en ;
  rdfs:range <http://datex2.eu/vocab/3/LocationReferencing/OpenlrFunctionalRoadClassEnum> .

<http://datex2.eu/vocab/3/LocationReferencing/openlrRadius>
  a owl:DatatypeProperty ;
  rdfs:comment "The radius of the corresponding circular area."@en ;
  rdfs:domain <http://datex2.eu/vocab/3/LocationReferencing/OpenlrCircleLocationReference> ;
  rdfs:label "Openlr radius"@en ;
  rdfs:range <http://datex2.eu/vocab/3/Common/MetresAsNonNegativeInteger> .

<http://datex2.eu/vocab/3/LocationReferencing/openlrNumColumns>
  a owl:DatatypeProperty ;
  rdfs:comment "The number that the base rectangle should be multiplied in the east direction"@en ;
  rdfs:domain <http://datex2.eu/vocab/3/LocationReferencing/OpenlrGridLocationReference> ;
  rdfs:label "Openlr num columns"@en ;
  rdfs:range <http://datex2.eu/vocab/3/Common/NonNegativeInteger> .

<http://datex2.eu/vocab/3/LocationReferencing/openlrNumRows>
  a owl:DatatypeProperty ;
  rdfs:comment "The number that the base rectangle should be multiplied in the north direction"@en ;
  rdfs:domain <http://datex2.eu/vocab/3/LocationReferencing/OpenlrGridLocationReference> ;
  rdfs:label "Openlr num rows"@en ;
  rdfs:range <http://datex2.eu/vocab/3/Common/NonNegativeInteger> .

<http://datex2.eu/vocab/3/LocationReferencing/openlrOrientation>
  a owl:DatatypeProperty ;
  rdfs:comment "Orientation of the driving direction in relation with the direction of the underlying linear"@en ;
  rdfs:domain <http://datex2.eu/vocab/3/LocationReferencing/OpenlrBasePointLocation>, <http://datex2.eu/vocab/3/LocationReferencing/OpenlrPointAttributes> ;
  rdfs:label "Openlr orientation"@en ;
  rdfs:range <http://datex2.eu/vocab/3/LocationReferencing/OpenlrOrientationEnum> .

<http://datex2.eu/vocab/3/LocationReferencing/openlrSideOfRoad>
  a owl:DatatypeProperty ;
  rdfs:comment "Provides the of road where the corresponding point lies."@en ;
  rdfs:domain <http://datex2.eu/vocab/3/LocationReferencing/OpenlrBasePointLocation>, <http://datex2.eu/vocab/3/LocationReferencing/OpenlrPointAttributes> ;
  rdfs:label "Openlr side of road"@en ;
  rdfs:range <http://datex2.eu/vocab/3/LocationReferencing/OpenlrSideOfRoadEnum> .

<http://datex2.eu/vocab/3/LocationReferencing/subdivisionCode>
  a owl:DatatypeProperty ;
  rdfs:comment "The second part of an ISO 3166-2 subdivision code for the named area, which may be used along with the country attribute from the parent class to make a full ISO 3166-2 subdivision code."@en ;
  rdfs:domain <http://datex2.eu/vocab/3/LocationReferencing/IsoNamedArea> ;
  rdfs:label "Subdivision code"@en ;
  rdfs:range <http://datex2.eu/vocab/3/LocationReferencing/SubdivisionCode> .

<http://datex2.eu/vocab/3/LocationReferencing/subdivisionType>
  a owl:DatatypeProperty ;
  rdfs:comment "The ISO 3166-2 subdivison type for the named area."@en ;
  rdfs:domain <http://datex2.eu/vocab/3/LocationReferencing/IsoNamedArea> ;
  rdfs:label "Subdivision type"@en ;
  rdfs:range <http://datex2.eu/vocab/3/LocationReferencing/SubdivisionTypeEnum> .

<http://datex2.eu/vocab/3/LocationReferencing/areaName>
  a owl:DatatypeProperty ;
  rdfs:comment "The name of the area."@en ;
  rdfs:domain <http://datex2.eu/vocab/3/LocationReferencing/NamedArea> ;
  rdfs:label "Area name"@en ;
  rdfs:range <http://datex2.eu/vocab/3/Common/MultilingualString> .

<http://datex2.eu/vocab/3/LocationReferencing/country>
  a owl:DatatypeProperty ;
  rdfs:comment "EN ISO 3166-1 two-character country code."@en ;
  rdfs:domain <http://datex2.eu/vocab/3/LocationReferencing/NamedArea> ;
  rdfs:label "Country"@en ;
  rdfs:range <http://datex2.eu/vocab/3/Common/CountryCode> .

<http://datex2.eu/vocab/3/LocationReferencing/namedAreaType>
  a owl:DatatypeProperty ;
  rdfs:comment "The type of the area."@en ;
  rdfs:domain <http://datex2.eu/vocab/3/LocationReferencing/NamedArea> ;
  rdfs:label "Named area type"@en ;
  rdfs:range <http://datex2.eu/vocab/3/LocationReferencing/NamedAreaTypeEnum> .

<http://datex2.eu/vocab/3/LocationReferencing/nutsCode>
  a owl:DatatypeProperty ;
  rdfs:comment "The NUTS code for the named area."@en ;
  rdfs:domain <http://datex2.eu/vocab/3/LocationReferencing/NutsNamedArea> ;
  rdfs:label "Nuts code"@en ;
  rdfs:range <http://datex2.eu/vocab/3/LocationReferencing/NutsCode> .

<http://datex2.eu/vocab/3/LocationReferencing/nutsCodeType>
  a owl:DatatypeProperty ;
  rdfs:comment "The NUTS code type for the named area."@en ;
  rdfs:domain <http://datex2.eu/vocab/3/LocationReferencing/NutsNamedArea> ;
  rdfs:label "Nuts code type"@en ;
  rdfs:range <http://datex2.eu/vocab/3/LocationReferencing/NutsCodeTypeEnum> .

<http://datex2.eu/vocab/3/LocationReferencing/predefinedItineraryName>
  a owl:DatatypeProperty ;
  rdfs:comment "A name assigned to the predefined itinerary."@en ;
  rdfs:domain <http://datex2.eu/vocab/3/LocationReferencing/PredefinedItinerary> ;
  rdfs:label "Predefined itinerary name"@en ;
  rdfs:range <http://datex2.eu/vocab/3/Common/MultilingualString> .

<http://datex2.eu/vocab/3/LocationReferencing/predefinedLocationName>
  a owl:DatatypeProperty ;
  rdfs:comment "A name assigned to the predefined location (e.g. extracted out of the network operator's gazetteer)."@en ;
  rdfs:domain <http://datex2.eu/vocab/3/LocationReferencing/PredefinedLocation> ;
  rdfs:label "Predefined location name"@en ;
  rdfs:range <http://datex2.eu/vocab/3/Common/MultilingualString> .

<http://datex2.eu/vocab/3/LocationReferencing/predefinedLocationGroupName>
  a owl:DatatypeProperty ;
  rdfs:comment "A name assigned to the predefined group of non-ordered locations."@en ;
  rdfs:domain <http://datex2.eu/vocab/3/LocationReferencing/PredefinedLocationGroup> ;
  rdfs:label "Predefined location group name"@en ;
  rdfs:range <http://datex2.eu/vocab/3/Common/MultilingualString> .

<http://datex2.eu/vocab/3/LocationReferencing/hasalertCArea>
  a owl:ObjectProperty ;
  rdfs:domain <http://datex2.eu/vocab/3/LocationReferencing/AreaLocation> ;
  rdfs:label "ALERT-C area"@en ;
  rdfs:range <http://datex2.eu/vocab/3/LocationReferencing/AlertCArea> .

<http://datex2.eu/vocab/3/LocationReferencing/hasgmlMultiPolygon>
  a owl:ObjectProperty ;
  rdfs:domain <http://datex2.eu/vocab/3/LocationReferencing/AreaLocation> ;
  rdfs:label "Gml multi polygon"@en ;
  rdfs:range <http://datex2.eu/vocab/3/LocationReferencing/GmlMultiPolygon> .

<http://datex2.eu/vocab/3/LocationReferencing/hastpegAreaLocation>
  a owl:ObjectProperty ;
  rdfs:domain <http://datex2.eu/vocab/3/LocationReferencing/AreaLocation> ;
  rdfs:label "TPEG area location"@en ;
  rdfs:range <http://datex2.eu/vocab/3/LocationReferencing/TpegAreaLocation> .

<http://datex2.eu/vocab/3/LocationReferencing/hasopenlrAreaLocationReference>
  a owl:ObjectProperty ;
  rdfs:domain <http://datex2.eu/vocab/3/LocationReferencing/AreaLocation> ;
  rdfs:label "Openlr area location reference"@en ;
  rdfs:range <http://datex2.eu/vocab/3/LocationReferencing/OpenlrAreaLocationReference> .

<http://datex2.eu/vocab/3/LocationReferencing/hasnamedArea>
  a owl:ObjectProperty ;
  rdfs:domain <http://datex2.eu/vocab/3/LocationReferencing/AreaLocation>, <http://datex2.eu/vocab/3/LocationReferencing/SupplementaryPositionalDescription> ;
  rdfs:label "Named area"@en ;
  rdfs:range <http://datex2.eu/vocab/3/LocationReferencing/NamedArea> .

<http://datex2.eu/vocab/3/LocationReferencing/hasgmlLineString>
  a owl:ObjectProperty ;
  rdfs:domain <http://datex2.eu/vocab/3/LocationReferencing/LinearLocation>, <http://datex2.eu/vocab/3/LocationReferencing/LinearElementByLineString> ;
  rdfs:label "Gml line string"@en ;
  rdfs:range <http://datex2.eu/vocab/3/LocationReferencing/GmlLineString> .

<http://datex2.eu/vocab/3/LocationReferencing/hassecondarySupplementaryDescription>
  a owl:ObjectProperty ;
  rdfs:comment "Supplementary description that applies to the secondary end of the linear location. Use when properties change along the Linear. For a one-way linear the secondary end should be the destination end."@en ;
  rdfs:domain <http://datex2.eu/vocab/3/LocationReferencing/LinearLocation> ;
  rdfs:label "Secondary supplementary description"@en ;
  rdfs:range <http://datex2.eu/vocab/3/LocationReferencing/SupplementaryPositionalDescription> .

<http://datex2.eu/vocab/3/LocationReferencing/hasopenlrLinear>
  a owl:ObjectProperty ;
  rdfs:domain <http://datex2.eu/vocab/3/LocationReferencing/LinearLocation> ;
  rdfs:label "Openlr linear"@en ;
  rdfs:range <http://datex2.eu/vocab/3/LocationReferencing/OpenlrLinear> .

<http://datex2.eu/vocab/3/LocationReferencing/hasalertCPoint>
  a owl:ObjectProperty ;
  rdfs:comment "The point location expressed using AlertC. Multiple instances of AlertCPoint shall represent the same real-world geographic feature."@en ;
  rdfs:domain <http://datex2.eu/vocab/3/LocationReferencing/PointLocation> ;
  rdfs:label "ALERT-C point"@en ;
  rdfs:range <http://datex2.eu/vocab/3/LocationReferencing/AlertCPoint> .

<http://datex2.eu/vocab/3/LocationReferencing/haspointAlongLinearElement>
  a owl:ObjectProperty ;
  rdfs:domain <http://datex2.eu/vocab/3/LocationReferencing/PointLocation> ;
  rdfs:label "Point along linear element"@en ;
  rdfs:range <http://datex2.eu/vocab/3/LocationReferencing/PointAlongLinearElement> .

<http://datex2.eu/vocab/3/LocationReferencing/haspointByCoordinates>
  a owl:ObjectProperty ;
  rdfs:domain <http://datex2.eu/vocab/3/LocationReferencing/PointLocation> ;
  rdfs:label "Point by coordinates"@en ;
  rdfs:range <http://datex2.eu/vocab/3/LocationReferencing/PointByCoordinates> .

<http://datex2.eu/vocab/3/LocationReferencing/hastpegPointLocation>
  a owl:ObjectProperty ;
  rdfs:domain <http://datex2.eu/vocab/3/LocationReferencing/PointLocation> ;
  rdfs:label "TPEG point location"@en ;
  rdfs:range <http://datex2.eu/vocab/3/LocationReferencing/TpegPointLocation> .

<http://datex2.eu/vocab/3/LocationReferencing/hasopenlrPointLocationReference>
  a owl:ObjectProperty ;
  rdfs:domain <http://datex2.eu/vocab/3/LocationReferencing/PointLocation> ;
  rdfs:label "Openlr point location reference"@en ;
  rdfs:range <http://datex2.eu/vocab/3/LocationReferencing/OpenlrPointLocationReference> .

<http://datex2.eu/vocab/3/LocationReferencing/hasalertCLinear>
  a owl:ObjectProperty ;
  rdfs:comment "The linear location expressed using AlertC. Multiple instances of AlertCLinear shall represent the same real-world geographic feature."@en ;
  rdfs:domain <http://datex2.eu/vocab/3/LocationReferencing/SingleRoadLinearLocation> ;
  rdfs:label "ALERT-C linear"@en ;
  rdfs:range <http://datex2.eu/vocab/3/LocationReferencing/AlertCLinear> .

<http://datex2.eu/vocab/3/LocationReferencing/haslinearWithinLinearElement>
  a owl:ObjectProperty ;
  rdfs:domain <http://datex2.eu/vocab/3/LocationReferencing/SingleRoadLinearLocation> ;
  rdfs:label "Linear within linear element"@en ;
  rdfs:range <http://datex2.eu/vocab/3/LocationReferencing/LinearWithinLinearElement> .

<http://datex2.eu/vocab/3/LocationReferencing/hastpegLinearLocation>
  a owl:ObjectProperty ;
  rdfs:domain <http://datex2.eu/vocab/3/LocationReferencing/SingleRoadLinearLocation> ;
  rdfs:label "TPEG linear location"@en ;
  rdfs:range <http://datex2.eu/vocab/3/LocationReferencing/TpegLinearLocation> .

<http://datex2.eu/vocab/3/LocationReferencing/hasareaLocation>
  a owl:ObjectProperty ;
  rdfs:domain <http://datex2.eu/vocab/3/LocationReferencing/AreaDestination>, <http://datex2.eu/vocab/3/LocationReferencing/AlertCArea> ;
  rdfs:label "Area location"@en ;
  rdfs:range <http://datex2.eu/vocab/3/LocationReferencing/AreaLocation>, <http://datex2.eu/vocab/3/LocationReferencing/AlertCLocation> ;
  rdfs:comment "Area location defined by a specific Alert-C location."@en .

<http://datex2.eu/vocab/3/LocationReferencing/hasrouteDestination>
  a owl:ObjectProperty ;
  rdfs:comment "Destination of a route or final location in an itinerary."@en ;
  rdfs:domain <http://datex2.eu/vocab/3/LocationReferencing/Itinerary> ;
  rdfs:label "Route destination"@en ;
  rdfs:range <http://datex2.eu/vocab/3/LocationReferencing/Destination> .

<http://datex2.eu/vocab/3/LocationReferencing/haslocationContainedInItinerary>
  a owl:ObjectProperty ;
  rdfs:comment "A location contained in an itinerary (i.e. an ordered set of locations defining a route or itinerary)."@en ;
  rdfs:domain <http://datex2.eu/vocab/3/LocationReferencing/ItineraryByIndexedLocations> ;
  rdfs:label "Location contained in itinerary"@en ;
  rdfs:range <http://datex2.eu/vocab/3/LocationReferencing/Location> .

<http://datex2.eu/vocab/3/LocationReferencing/hasdestination>
  a owl:ObjectProperty ;
  rdfs:domain <http://datex2.eu/vocab/3/LocationReferencing/NetworkLocation> ;
  rdfs:label "Destination"@en ;
  rdfs:range <http://datex2.eu/vocab/3/LocationReferencing/Destination> .

<http://datex2.eu/vocab/3/LocationReferencing/hassupplementaryPositionalDescription>
  a owl:ObjectProperty ;
  rdfs:domain <http://datex2.eu/vocab/3/LocationReferencing/NetworkLocation> ;
  rdfs:label "Supplementary positional description"@en ;
  rdfs:range <http://datex2.eu/vocab/3/LocationReferencing/SupplementaryPositionalDescription> .

<http://datex2.eu/vocab/3/LocationReferencing/haslocationContainedInGroup>
  a owl:ObjectProperty ;
  rdfs:comment "A location contained in a non-ordered group of locations."@en ;
  rdfs:domain <http://datex2.eu/vocab/3/LocationReferencing/LocationGroupByList> ;
  rdfs:label "Location contained in group"@en ;
  rdfs:range <http://datex2.eu/vocab/3/LocationReferencing/Location> .

<http://datex2.eu/vocab/3/LocationReferencing/haspointLocation>
  a owl:ObjectProperty ;
  rdfs:domain <http://datex2.eu/vocab/3/LocationReferencing/PointDestination> ;
  rdfs:label "Point location"@en ;
  rdfs:range <http://datex2.eu/vocab/3/LocationReferencing/PointLocation> .

<http://datex2.eu/vocab/3/LocationReferencing/hasexternalReferencing>
  a owl:ObjectProperty ;
  rdfs:domain <http://datex2.eu/vocab/3/LocationReferencing/Location> ;
  rdfs:label "External referencing"@en ;
  rdfs:range <http://datex2.eu/vocab/3/LocationReferencing/ExternalReferencing> .

<http://datex2.eu/vocab/3/LocationReferencing/hascoordinatesForDisplay>
  a owl:ObjectProperty ;
  rdfs:comment "Coordinates that may be used by clients for visual display on user interfaces."@en ;
  rdfs:domain <http://datex2.eu/vocab/3/LocationReferencing/Location> ;
  rdfs:label "Coordinates for display"@en ;
  rdfs:range <http://datex2.eu/vocab/3/LocationReferencing/PointCoordinates> .

<http://datex2.eu/vocab/3/LocationReferencing/hasalertCLocation>
  a owl:ObjectProperty ;
  rdfs:domain <http://datex2.eu/vocab/3/LocationReferencing/AlertCMethod2PrimaryPointLocation>, <http://datex2.eu/vocab/3/LocationReferencing/AlertCMethod2SecondaryPointLocation>, <http://datex2.eu/vocab/3/LocationReferencing/AlertCMethod4PrimaryPointLocation>, <http://datex2.eu/vocab/3/LocationReferencing/AlertCMethod4SecondaryPointLocation> ;
  rdfs:label "ALERT-C location"@en ;
  rdfs:range <http://datex2.eu/vocab/3/LocationReferencing/AlertCLocation> .

<http://datex2.eu/vocab/3/LocationReferencing/hasoffsetDistance>
  a owl:ObjectProperty ;
  rdfs:domain <http://datex2.eu/vocab/3/LocationReferencing/AlertCMethod4PrimaryPointLocation>, <http://datex2.eu/vocab/3/LocationReferencing/AlertCMethod4SecondaryPointLocation> ;
  rdfs:label "Offset distance"@en ;
  rdfs:range <http://datex2.eu/vocab/3/LocationReferencing/OffsetDistance> .

<http://datex2.eu/vocab/3/LocationReferencing/hasalertCDirection>
  a owl:ObjectProperty ;
  rdfs:domain <http://datex2.eu/vocab/3/LocationReferencing/AlertCLinearByCode>, <http://datex2.eu/vocab/3/LocationReferencing/AlertCMethod2Linear>, <http://datex2.eu/vocab/3/LocationReferencing/AlertCMethod2Point>, <http://datex2.eu/vocab/3/LocationReferencing/AlertCMethod4Linear>, <http://datex2.eu/vocab/3/LocationReferencing/AlertCMethod4Point> ;
  rdfs:label "ALERT-C direction"@en ;
  rdfs:range <http://datex2.eu/vocab/3/LocationReferencing/AlertCDirection> .

<http://datex2.eu/vocab/3/LocationReferencing/haslocationCodeForLinearLocation>
  a owl:ObjectProperty ;
  rdfs:comment "Linear location defined by a specific Alert-C location."@en ;
  rdfs:domain <http://datex2.eu/vocab/3/LocationReferencing/AlertCLinearByCode> ;
  rdfs:label "Location code for linear location"@en ;
  rdfs:range <http://datex2.eu/vocab/3/LocationReferencing/AlertCLocation> .

<http://datex2.eu/vocab/3/LocationReferencing/hasalertCMethod2PrimaryPointLocation>
  a owl:ObjectProperty ;
  rdfs:domain <http://datex2.eu/vocab/3/LocationReferencing/AlertCMethod2Linear>, <http://datex2.eu/vocab/3/LocationReferencing/AlertCMethod2Point> ;
  rdfs:label "ALERT-C method2 primary point location"@en ;
  rdfs:range <http://datex2.eu/vocab/3/LocationReferencing/AlertCMethod2PrimaryPointLocation> .

<http://datex2.eu/vocab/3/LocationReferencing/hasalertCMethod2SecondaryPointLocation>
  a owl:ObjectProperty ;
  rdfs:domain <http://datex2.eu/vocab/3/LocationReferencing/AlertCMethod2Linear> ;
  rdfs:label "ALERT-C method2 secondary point location"@en ;
  rdfs:range <http://datex2.eu/vocab/3/LocationReferencing/AlertCMethod2SecondaryPointLocation> .

<http://datex2.eu/vocab/3/LocationReferencing/hasalertCMethod4PrimaryPointLocation>
  a owl:ObjectProperty ;
  rdfs:domain <http://datex2.eu/vocab/3/LocationReferencing/AlertCMethod4Linear>, <http://datex2.eu/vocab/3/LocationReferencing/AlertCMethod4Point> ;
  rdfs:label "ALERT-C method4 primary point location"@en ;
  rdfs:range <http://datex2.eu/vocab/3/LocationReferencing/AlertCMethod4PrimaryPointLocation> .

<http://datex2.eu/vocab/3/LocationReferencing/hasalertCMethod4SecondaryPointLocation>
  a owl:ObjectProperty ;
  rdfs:domain <http://datex2.eu/vocab/3/LocationReferencing/AlertCMethod4Linear> ;
  rdfs:label "ALERT-C method4 secondary point location"@en ;
  rdfs:range <http://datex2.eu/vocab/3/LocationReferencing/AlertCMethod4SecondaryPointLocation> .

<http://datex2.eu/vocab/3/LocationReferencing/hasgmlPolygon>
  a owl:ObjectProperty ;
  rdfs:domain <http://datex2.eu/vocab/3/LocationReferencing/GmlMultiPolygon> ;
  rdfs:label "Gml polygon"@en ;
  rdfs:range <http://datex2.eu/vocab/3/LocationReferencing/GmlPolygon> .

<http://datex2.eu/vocab/3/LocationReferencing/hasinterior>
  a owl:ObjectProperty ;
  rdfs:comment "A boundary of internal patches of a polygonal surface consisting of a ring feature"@en ;
  rdfs:domain <http://datex2.eu/vocab/3/LocationReferencing/GmlPolygon> ;
  rdfs:label "Interior"@en ;
  rdfs:range <http://datex2.eu/vocab/3/LocationReferencing/GmlLinearRing> .

<http://datex2.eu/vocab/3/LocationReferencing/hasexterior>
  a owl:ObjectProperty ;
  rdfs:comment "A boundary of a polygonal surface consisting of a ring i.e. in the normal 2D case, a closed polygonal line distinguished as exterior. Such a polygonal line has at least 4 pairs of coordinates"@en ;
  rdfs:domain <http://datex2.eu/vocab/3/LocationReferencing/GmlPolygon> ;
  rdfs:label "Exterior"@en ;
  rdfs:range <http://datex2.eu/vocab/3/LocationReferencing/GmlLinearRing> .

<http://datex2.eu/vocab/3/LocationReferencing/hasfromPoint>
  a owl:ObjectProperty ;
  rdfs:comment "A point on the linear element that defines the start node of the linear section."@en ;
  rdfs:domain <http://datex2.eu/vocab/3/LocationReferencing/LinearWithinLinearElement> ;
  rdfs:label "From point"@en ;
  rdfs:range <http://datex2.eu/vocab/3/LocationReferencing/DistanceAlongLinearElement> .

<http://datex2.eu/vocab/3/LocationReferencing/hastoPoint>
  a owl:ObjectProperty ;
  rdfs:comment "A point on the linear element that defines the end node of the linear section."@en ;
  rdfs:domain <http://datex2.eu/vocab/3/LocationReferencing/LinearWithinLinearElement> ;
  rdfs:label "To point"@en ;
  rdfs:range <http://datex2.eu/vocab/3/LocationReferencing/DistanceAlongLinearElement> .

<http://datex2.eu/vocab/3/LocationReferencing/haslinearElement>
  a owl:ObjectProperty ;
  rdfs:domain <http://datex2.eu/vocab/3/LocationReferencing/LinearWithinLinearElement>, <http://datex2.eu/vocab/3/LocationReferencing/PointAlongLinearElement> ;
  rdfs:label "Linear element"@en ;
  rdfs:range <http://datex2.eu/vocab/3/LocationReferencing/LinearElement> .

<http://datex2.eu/vocab/3/LocationReferencing/hasfromReferent>
  a owl:ObjectProperty ;
  rdfs:comment "A known location along the linear element from which the distanceAlong is measured, termed the \"fromReferent\" in EN ISO 19148. "@en ;
  rdfs:domain <http://datex2.eu/vocab/3/LocationReferencing/DistanceFromLinearElementReferent> ;
  rdfs:label "From referent"@en ;
  rdfs:range <http://datex2.eu/vocab/3/LocationReferencing/Referent> .

<http://datex2.eu/vocab/3/LocationReferencing/hastowardsReferent>
  a owl:ObjectProperty ;
  rdfs:comment "A known location along the linear element towards which the distanceAlong is measured, termed the \"towardsReferent\" in EN ISO 19148."@en ;
  rdfs:domain <http://datex2.eu/vocab/3/LocationReferencing/DistanceFromLinearElementReferent> ;
  rdfs:label "Towards referent"@en ;
  rdfs:range <http://datex2.eu/vocab/3/LocationReferencing/Referent> .

<http://datex2.eu/vocab/3/LocationReferencing/hasendPointOfLinearElement>
  a owl:ObjectProperty ;
  rdfs:comment "The referent at a known location on the linear object which defines the end of the linear element."@en ;
  rdfs:domain <http://datex2.eu/vocab/3/LocationReferencing/LinearElementByPoints> ;
  rdfs:label "End point of linear element"@en ;
  rdfs:range <http://datex2.eu/vocab/3/LocationReferencing/Referent> .

<http://datex2.eu/vocab/3/LocationReferencing/hasstartPointOfLinearElement>
  a owl:ObjectProperty ;
  rdfs:comment "The referent at a known location on the linear object which defines the start of the linear element."@en ;
  rdfs:domain <http://datex2.eu/vocab/3/LocationReferencing/LinearElementByPoints> ;
  rdfs:label "Start point of linear element"@en ;
  rdfs:range <http://datex2.eu/vocab/3/LocationReferencing/Referent> .

<http://datex2.eu/vocab/3/LocationReferencing/hasintermediatePointOnLinearElement>
  a owl:ObjectProperty ;
  rdfs:comment "A referent at a known location on the linear object which is neither the start or end of the linear element."@en ;
  rdfs:domain <http://datex2.eu/vocab/3/LocationReferencing/LinearElementByPoints> ;
  rdfs:label "Intermediate point on linear element"@en ;
  rdfs:range <http://datex2.eu/vocab/3/LocationReferencing/Referent> .

<http://datex2.eu/vocab/3/LocationReferencing/hasdistanceAlongLinearElement>
  a owl:ObjectProperty ;
  rdfs:domain <http://datex2.eu/vocab/3/LocationReferencing/PointAlongLinearElement> ;
  rdfs:label "Distance along linear element"@en ;
  rdfs:range <http://datex2.eu/vocab/3/LocationReferencing/DistanceAlongLinearElement> .

<http://datex2.eu/vocab/3/LocationReferencing/haspointCoordinates>
  a owl:ObjectProperty ;
  rdfs:domain <http://datex2.eu/vocab/3/LocationReferencing/Referent>, <http://datex2.eu/vocab/3/LocationReferencing/PointByCoordinates>, <http://datex2.eu/vocab/3/LocationReferencing/TpegJunction>, <http://datex2.eu/vocab/3/LocationReferencing/TpegNonJunctionPoint> ;
  rdfs:label "Point coordinates"@en ;
  rdfs:range <http://datex2.eu/vocab/3/LocationReferencing/PointCoordinates> .

<http://datex2.eu/vocab/3/LocationReferencing/hasaltitudeConfidence>
  a owl:ObjectProperty ;
  rdfs:domain <http://datex2.eu/vocab/3/LocationReferencing/HeightCoordinate> ;
  rdfs:label "Altitude confidence"@en ;
  rdfs:range <http://datex2.eu/vocab/3/LocationReferencing/AltitudeConfidence> .

<http://datex2.eu/vocab/3/LocationReferencing/hasverticalPositionAccuracy>
  a owl:ObjectProperty ;
  rdfs:comment "Defines the vertical position accuracy according to EN16803-1"@en ;
  rdfs:domain <http://datex2.eu/vocab/3/LocationReferencing/HeightCoordinate> ;
  rdfs:label "Vertical position accuracy"@en ;
  rdfs:range <http://datex2.eu/vocab/3/LocationReferencing/PositionAccuracy> .

<http://datex2.eu/vocab/3/LocationReferencing/hasheightCoordinate>
  a owl:ObjectProperty ;
  rdfs:domain <http://datex2.eu/vocab/3/LocationReferencing/PointCoordinates> ;
  rdfs:label "Height coordinate"@en ;
  rdfs:range <http://datex2.eu/vocab/3/LocationReferencing/HeightCoordinate> .

<http://datex2.eu/vocab/3/LocationReferencing/hashorizontalPositionAccuracy>
  a owl:ObjectProperty ;
  rdfs:comment "Defines the horizontal position accuracy according EN 16803-1"@en ;
  rdfs:domain <http://datex2.eu/vocab/3/LocationReferencing/PointCoordinates> ;
  rdfs:label "Horizontal position accuracy"@en ;
  rdfs:range <http://datex2.eu/vocab/3/LocationReferencing/PositionAccuracy> .

<http://datex2.eu/vocab/3/LocationReferencing/haspositionConfidenceEllipse>
  a owl:ObjectProperty ;
  rdfs:domain <http://datex2.eu/vocab/3/LocationReferencing/PointCoordinates> ;
  rdfs:label "Position confidence ellipse"@en ;
  rdfs:range <http://datex2.eu/vocab/3/LocationReferencing/PositionConfidenceEllipse> .

<http://datex2.eu/vocab/3/LocationReferencing/haslane>
  a owl:ObjectProperty ;
  rdfs:domain <http://datex2.eu/vocab/3/LocationReferencing/Carriageway> ;
  rdfs:label "Lane"@en ;
  rdfs:range <http://datex2.eu/vocab/3/LocationReferencing/Lane> .

<http://datex2.eu/vocab/3/LocationReferencing/hasroadInformation>
  a owl:ObjectProperty ;
  rdfs:comment "Information on a set of one or more roads. The location could correspond to a part of the road identified, the whole stretch of road identified, or a combination of multiple road sections."@en ;
  rdfs:domain <http://datex2.eu/vocab/3/LocationReferencing/SupplementaryPositionalDescription> ;
  rdfs:label "Road information"@en ;
  rdfs:range <http://datex2.eu/vocab/3/LocationReferencing/RoadInformation> .

<http://datex2.eu/vocab/3/LocationReferencing/hascarriageway>
  a owl:ObjectProperty ;
  rdfs:domain <http://datex2.eu/vocab/3/LocationReferencing/SupplementaryPositionalDescription> ;
  rdfs:label "Carriageway"@en ;
  rdfs:range <http://datex2.eu/vocab/3/LocationReferencing/Carriageway> .

<http://datex2.eu/vocab/3/LocationReferencing/hastpegHeight>
  a owl:ObjectProperty ;
  rdfs:domain <http://datex2.eu/vocab/3/LocationReferencing/TpegAreaLocation> ;
  rdfs:label "TPEG height"@en ;
  rdfs:range <http://datex2.eu/vocab/3/LocationReferencing/TpegHeight> .

<http://datex2.eu/vocab/3/LocationReferencing/hascentrePoint>
  a owl:ObjectProperty ;
  rdfs:comment "Centre point of a circular geometric area."@en ;
  rdfs:domain <http://datex2.eu/vocab/3/LocationReferencing/TpegGeometricArea> ;
  rdfs:label "Centre point"@en ;
  rdfs:range <http://datex2.eu/vocab/3/LocationReferencing/PointCoordinates> .

<http://datex2.eu/vocab/3/LocationReferencing/hasname>
  a owl:ObjectProperty ;
  rdfs:comment "Name of area."@en, "A name which identifies a junction point on the road network"@en, "A descriptive name which helps to identify the non-junction point. At least one descriptor must identify the road on which the point is located, i.e. must be of type 'linkName' or 'localLinkName'."@en ;
  rdfs:domain <http://datex2.eu/vocab/3/LocationReferencing/TpegGeometricArea>, <http://datex2.eu/vocab/3/LocationReferencing/TpegNamedOnlyArea>, <http://datex2.eu/vocab/3/LocationReferencing/TpegJunction>, <http://datex2.eu/vocab/3/LocationReferencing/TpegNonJunctionPoint> ;
  rdfs:label "Name"@en ;
  rdfs:range <http://datex2.eu/vocab/3/LocationReferencing/TpegAreaDescriptor>, <http://datex2.eu/vocab/3/LocationReferencing/TpegJunctionPointDescriptor>, <http://datex2.eu/vocab/3/LocationReferencing/TpegOtherPointDescriptor> .

<http://datex2.eu/vocab/3/LocationReferencing/hasto>
  a owl:ObjectProperty ;
  rdfs:comment "The location at the down stream end of the linear section of road."@en, "The location at the downstream end of the section of road which frames the TPEGFramedPoint."@en ;
  rdfs:domain <http://datex2.eu/vocab/3/LocationReferencing/TpegLinearLocation>, <http://datex2.eu/vocab/3/LocationReferencing/TpegFramedPoint> ;
  rdfs:label "To"@en ;
  rdfs:range <http://datex2.eu/vocab/3/LocationReferencing/TpegPoint> .

<http://datex2.eu/vocab/3/LocationReferencing/hasfrom>
  a owl:ObjectProperty ;
  rdfs:comment "The location at the up stream end of the linear section of road."@en, "The location at the upstream end of the section of road which frames the TPEGFramedPoint."@en ;
  rdfs:domain <http://datex2.eu/vocab/3/LocationReferencing/TpegLinearLocation>, <http://datex2.eu/vocab/3/LocationReferencing/TpegFramedPoint> ;
  rdfs:label "From"@en ;
  rdfs:range <http://datex2.eu/vocab/3/LocationReferencing/TpegPoint> .

<http://datex2.eu/vocab/3/LocationReferencing/hasframedPoint>
  a owl:ObjectProperty ;
  rdfs:comment "A single non-junction point on the road network which is framed between two other specified points on the road network."@en ;
  rdfs:domain <http://datex2.eu/vocab/3/LocationReferencing/TpegFramedPoint> ;
  rdfs:label "Framed point"@en ;
  rdfs:range <http://datex2.eu/vocab/3/LocationReferencing/TpegNonJunctionPoint> .

<http://datex2.eu/vocab/3/LocationReferencing/haspoint>
  a owl:ObjectProperty ;
  rdfs:comment "A single point defined by a coordinate set and TPEG descriptors."@en ;
  rdfs:domain <http://datex2.eu/vocab/3/LocationReferencing/TpegSimplePoint> ;
  rdfs:label "Point"@en ;
  rdfs:range <http://datex2.eu/vocab/3/LocationReferencing/TpegPoint> .

<http://datex2.eu/vocab/3/LocationReferencing/hasilc>
  a owl:ObjectProperty ;
  rdfs:comment "A descriptor for describing a junction by identifying the intersecting roads at a road junction."@en ;
  rdfs:domain <http://datex2.eu/vocab/3/LocationReferencing/TpegJunction> ;
  rdfs:label "Ilc"@en ;
  rdfs:range <http://datex2.eu/vocab/3/LocationReferencing/TpegIlcPointDescriptor> .

<http://datex2.eu/vocab/3/LocationReferencing/hasotherName>
  a owl:ObjectProperty ;
  rdfs:comment "A descriptive name which helps to identify the junction point."@en ;
  rdfs:domain <http://datex2.eu/vocab/3/LocationReferencing/TpegJunction> ;
  rdfs:label "Other name"@en ;
  rdfs:range <http://datex2.eu/vocab/3/LocationReferencing/TpegOtherPointDescriptor> .

<http://datex2.eu/vocab/3/LocationReferencing/hasopenlrCoordinates>
  a owl:ObjectProperty ;
  rdfs:comment "Provides coordinates for the base point of the OpenLR path"@en, "Corresponding coordinates of vertices that define a polygon."@en, "Corresponding coordinates of an OpenLR point defined by its only coordinates."@en, "The coordinate of the actual point of interest"@en ;
  rdfs:domain <http://datex2.eu/vocab/3/LocationReferencing/OpenlrBaseReferencePoint>, <http://datex2.eu/vocab/3/LocationReferencing/OpenlrPolygonCorners>, <http://datex2.eu/vocab/3/LocationReferencing/OpenlrGeoCoordinate>, <http://datex2.eu/vocab/3/LocationReferencing/OpenlrPoiWithAccessPoint> ;
  rdfs:label "Openlr coordinates"@en ;
  rdfs:range <http://datex2.eu/vocab/3/LocationReferencing/PointCoordinates> .

<http://datex2.eu/vocab/3/LocationReferencing/hasopenlrLineAttributes>
  a owl:ObjectProperty ;
  rdfs:comment "Properties of the line towards the topologically adjacent OpenLR location referencing point, on the shortest path to that point."@en ;
  rdfs:domain <http://datex2.eu/vocab/3/LocationReferencing/OpenlrBaseReferencePoint> ;
  rdfs:label "Openlr line attributes"@en ;
  rdfs:range <http://datex2.eu/vocab/3/LocationReferencing/OpenlrLineAttributes> .

<http://datex2.eu/vocab/3/LocationReferencing/hasopenlrGeoCoordinate>
  a owl:ObjectProperty ;
  rdfs:domain <http://datex2.eu/vocab/3/LocationReferencing/OpenlrCircleLocationReference> ;
  rdfs:label "Openlr geo coordinate"@en ;
  rdfs:range <http://datex2.eu/vocab/3/LocationReferencing/OpenlrGeoCoordinate> .

<http://datex2.eu/vocab/3/LocationReferencing/hasopenlrLastLine>
  a owl:ObjectProperty ;
  rdfs:comment "Provides the line attributes for the last line section closing the polygon."@en ;
  rdfs:domain <http://datex2.eu/vocab/3/LocationReferencing/OpenlrClosedLineLocationReference> ;
  rdfs:label "Openlr last line"@en ;
  rdfs:range <http://datex2.eu/vocab/3/LocationReferencing/OpenlrLastLocationReferencePoint> .

<http://datex2.eu/vocab/3/LocationReferencing/hasopenlrLocationReferencePoint>
  a owl:ObjectProperty ;
  rdfs:domain <http://datex2.eu/vocab/3/LocationReferencing/OpenlrClosedLineLocationReference>, <http://datex2.eu/vocab/3/LocationReferencing/OpenlrLineLocationReference>, <http://datex2.eu/vocab/3/LocationReferencing/OpenlrBasePointLocation> ;
  rdfs:label "Openlr location reference point"@en ;
  rdfs:range <http://datex2.eu/vocab/3/LocationReferencing/OpenlrLocationReferencePoint> ;
  rdfs:comment "Allows defining the first point of the OpenLR path"@en .

<http://datex2.eu/vocab/3/LocationReferencing/hasopenlrRectangle>
  a owl:ObjectProperty ;
  rdfs:domain <http://datex2.eu/vocab/3/LocationReferencing/OpenlrGridLocationReference>, <http://datex2.eu/vocab/3/LocationReferencing/OpenlrRectangleLocationReference> ;
  rdfs:label "Openlr rectangle"@en ;
  rdfs:range <http://datex2.eu/vocab/3/LocationReferencing/OpenlrRectangle> .

<http://datex2.eu/vocab/3/LocationReferencing/hasopenlrPolygonCorners>
  a owl:ObjectProperty ;
  rdfs:domain <http://datex2.eu/vocab/3/LocationReferencing/OpenlrPolygonLocationReference> ;
  rdfs:label "Openlr polygon corners"@en ;
  rdfs:range <http://datex2.eu/vocab/3/LocationReferencing/OpenlrPolygonCorners> .

<http://datex2.eu/vocab/3/LocationReferencing/hasopenlrLowerLeft>
  a owl:ObjectProperty ;
  rdfs:comment "The lower left corner of the rectangle."@en ;
  rdfs:domain <http://datex2.eu/vocab/3/LocationReferencing/OpenlrRectangle> ;
  rdfs:label "Openlr lower left"@en ;
  rdfs:range <http://datex2.eu/vocab/3/LocationReferencing/PointCoordinates> .

<http://datex2.eu/vocab/3/LocationReferencing/hasopenlrUpperRight>
  a owl:ObjectProperty ;
  rdfs:comment "The upper right corner of the rectangle."@en ;
  rdfs:domain <http://datex2.eu/vocab/3/LocationReferencing/OpenlrRectangle> ;
  rdfs:label "Openlr upper right"@en ;
  rdfs:range <http://datex2.eu/vocab/3/LocationReferencing/PointCoordinates> .

<http://datex2.eu/vocab/3/LocationReferencing/hasfirstDirection>
  a owl:ObjectProperty ;
  rdfs:comment "First OpenLR reference in first/main direction."@en ;
  rdfs:domain <http://datex2.eu/vocab/3/LocationReferencing/OpenlrLinear> ;
  rdfs:label "First direction"@en ;
  rdfs:range <http://datex2.eu/vocab/3/LocationReferencing/OpenlrLineLocationReference> .

<http://datex2.eu/vocab/3/LocationReferencing/hasoppositeDirection>
  a owl:ObjectProperty ;
  rdfs:comment "If both direction, this is the reference in the opposite direction against firstDirection."@en ;
  rdfs:domain <http://datex2.eu/vocab/3/LocationReferencing/OpenlrLinear> ;
  rdfs:label "Opposite direction"@en ;
  rdfs:range <http://datex2.eu/vocab/3/LocationReferencing/OpenlrLineLocationReference> .

<http://datex2.eu/vocab/3/LocationReferencing/hasopenlrOffsets>
  a owl:ObjectProperty ;
  rdfs:comment "Allows for adding offsets to the line location path defined by nodes when the starting (respectively ending) point does not coincide with a node."@en, "Provides optional offsets relative to the path"@en ;
  rdfs:domain <http://datex2.eu/vocab/3/LocationReferencing/OpenlrLineLocationReference>, <http://datex2.eu/vocab/3/LocationReferencing/OpenlrBasePointLocation> ;
  rdfs:label "Openlr offsets"@en ;
  rdfs:range <http://datex2.eu/vocab/3/LocationReferencing/OpenlrOffsets> .

<http://datex2.eu/vocab/3/LocationReferencing/hasopenlrLastLocationReferencePoint>
  a owl:ObjectProperty ;
  rdfs:domain <http://datex2.eu/vocab/3/LocationReferencing/OpenlrLineLocationReference>, <http://datex2.eu/vocab/3/LocationReferencing/OpenlrBasePointLocation> ;
  rdfs:label "Openlr last location reference point"@en ;
  rdfs:range <http://datex2.eu/vocab/3/LocationReferencing/OpenlrLastLocationReferencePoint> ;
  rdfs:comment "Allows defining the last point of the OpenLR path"@en .

<http://datex2.eu/vocab/3/LocationReferencing/hasopenlrPathAttributes>
  a owl:ObjectProperty ;
  rdfs:comment "Additional path attributes relative to the next point"@en ;
  rdfs:domain <http://datex2.eu/vocab/3/LocationReferencing/OpenlrLocationReferencePoint> ;
  rdfs:label "Openlr path attributes"@en ;
  rdfs:range <http://datex2.eu/vocab/3/LocationReferencing/OpenlrPathAttributes> .

<http://datex2.eu/vocab/3/LocationReferencing/hasitinerary>
  a owl:ObjectProperty ;
  rdfs:domain <http://datex2.eu/vocab/3/LocationReferencing/PredefinedItinerary> ;
  rdfs:label "Itinerary"@en ;
  rdfs:range <http://datex2.eu/vocab/3/LocationReferencing/Itinerary> .

<http://datex2.eu/vocab/3/LocationReferencing/haspredefinedLocation>
  a owl:ObjectProperty ;
  rdfs:domain <http://datex2.eu/vocab/3/LocationReferencing/PredefinedItinerary>, <http://datex2.eu/vocab/3/LocationReferencing/PredefinedLocationGroup> ;
  rdfs:label "Predefined location"@en ;
  rdfs:range <http://datex2.eu/vocab/3/LocationReferencing/PredefinedLocation> .

<http://datex2.eu/vocab/3/LocationReferencing/haslocation>
  a owl:ObjectProperty ;
  rdfs:domain <http://datex2.eu/vocab/3/LocationReferencing/PredefinedLocation> ;
  rdfs:label "Location"@en ;
  rdfs:range <http://datex2.eu/vocab/3/LocationReferencing/Location> .

<http://datex2.eu/vocab/3/LocationReferencing/haslocationGroup>
  a owl:ObjectProperty ;
  rdfs:domain <http://datex2.eu/vocab/3/LocationReferencing/PredefinedLocationGroup> ;
  rdfs:label "Location group"@en ;
  rdfs:range <http://datex2.eu/vocab/3/LocationReferencing/LocationGroup> .

<http://datex2.eu/vocab/3/LocationReferencing/hasheaderInformation>
  a owl:ObjectProperty ;
  rdfs:domain <http://datex2.eu/vocab/3/LocationReferencing/PredefinedLocationsPublication> ;
  rdfs:label "Header information"@en ;
  rdfs:range <http://datex2.eu/vocab/3/Common/HeaderInformation> .

<http://datex2.eu/vocab/3/LocationReferencing/haspredefinedLocationReference>
  a owl:ObjectProperty ;
  rdfs:domain <http://datex2.eu/vocab/3/LocationReferencing/PredefinedLocationsPublication> ;
  rdfs:label "Predefined location reference"@en ;
  rdfs:range <http://datex2.eu/vocab/3/LocationReferencing/PredefinedLocationReference> .