@prefix : <http://cdm.ovh/rsm/adapters/geosparql_adapter#> .
@prefix owl: <http://www.w3.org/2002/07/owl#> .
@prefix rdf: <http://www.w3.org/1999/02/22-rdf-syntax-ns#> .
@prefix xml: <http://www.w3.org/XML/1998/namespace> .
@prefix xsd: <http://www.w3.org/2001/XMLSchema#> .
@prefix rdfs: <http://www.w3.org/2000/01/rdf-schema#> .
@prefix skos: <https://www.w3.org/2004/02/skos/core#> .
@base <http://cdm.ovh/rsm/adapters/geosparql_adapter> .

<http://cdm.ovh/rsm/adapters/geosparql_adapter> rdf:type owl:Ontology ;
                                                 rdfs:comment "Adapter vocabulary for connecting various parts of RSM with GeoSPARQL 1.1."@en ;
                                                 rdfs:label "GeoSPARQL adapter for CDM/RSM"@en .

#################################################################
#    Annotation properties
#################################################################

###  http://purl.org/dc/elements/1.1/source
<http://purl.org/dc/elements/1.1/source> rdf:type owl:AnnotationProperty .


###  http://www.w3.org/2004/02/skos/core#altLabel
<http://www.w3.org/2004/02/skos/core#altLabel> rdf:type owl:AnnotationProperty .


###  http://www.w3.org/2004/02/skos/core#definition
<http://www.w3.org/2004/02/skos/core#definition> rdf:type owl:AnnotationProperty .


###  http://www.w3.org/2004/02/skos/core#prefLabel
<http://www.w3.org/2004/02/skos/core#prefLabel> rdf:type owl:AnnotationProperty .


#################################################################
#    Object Properties
#################################################################

###  http://cdm.ovh/rsm/adapters/geosparql_adapter#hasGeometry
:hasGeometry rdf:type owl:ObjectProperty ;
             rdfs:subPropertyOf <http://www.opengis.net/ont/geosparql#hasGeometry> ;
             rdfs:comment "A spatial representation for a given Feature. As in GeoSPARQL, a feature can be associated with more than one geometry (valid at different times, or provided by different surveys...)."@en .


###  http://cdm.ovh/rsm/adapters/geosparql_adapter#hasNominalGeometry
:hasNominalGeometry rdf:type owl:ObjectProperty ;
                    rdfs:subPropertyOf :hasGeometry ,
                                       <http://www.opengis.net/ont/geosparql#hasDefaultGeometry> ;
                    rdfs:comment "The default Geometry to be used in spatial calculations. It is usually the most detailed Geometry. Takes into account SOSA/SSN viewpoint, i.e. there can be more than one default geometry (e.g. valid at different times)."@en .


###  http://www.opengis.net/ont/geosparql#hasDefaultGeometry
<http://www.opengis.net/ont/geosparql#hasDefaultGeometry> rdf:type owl:ObjectProperty ;
                                                          rdfs:subPropertyOf <http://www.opengis.net/ont/geosparql#hasGeometry> ;
                                                          rdfs:comment "The default Geometry to be used in spatial calculations. It is usually the most detailed Geometry."@en .


###  http://www.opengis.net/ont/geosparql#hasGeometry
<http://www.opengis.net/ont/geosparql#hasGeometry> rdf:type owl:ObjectProperty .


#################################################################
#    Data properties
#################################################################

###  http://cdm.ovh/rsm/adapters/geosparql_adapter#hasNominalMetricLength
:hasNominalMetricLength rdf:type owl:DatatypeProperty ;
                        rdfs:subPropertyOf <http://www.opengis.net/ont/geosparql#hasMetricLength> ;
                        rdfs:range [ rdf:type rdfs:Datatype ;
                                     owl:onDatatype xsd:double ;
                                     owl:withRestrictions ( [ xsd:minInclusive "0.0"^^xsd:double
                                                            ]
                                                          )
                                   ] ;
                        rdfs:comment """Length (in meter) of a Linear Element. This length is assumed to be derived from the chosen Nominal Geometry.

The Nominal Metric Length is supposed to be used for conversions between linear referencing methods \"absolute\" (distance along, e.g. used in CCS/TMS data model) and \"interpolation\" (intrinsic coordinates, with values 0 to 1, used in RSM and others).

Compared to geo:hasMetricLength, from which it is derived, a restriction was applied to the range (non-negative values)."""@en .


###  http://www.opengis.net/ont/geosparql#hasMetricLength
<http://www.opengis.net/ont/geosparql#hasMetricLength> rdf:type owl:DatatypeProperty ;
                                                       rdfs:range [ rdf:type rdfs:Datatype ;
                                                                    owl:onDatatype xsd:double ;
                                                                    owl:withRestrictions ( [ xsd:minInclusive "0.0"^^xsd:double
                                                                                           ]
                                                                                         )
                                                                  ] .


#################################################################
#    Classes
#################################################################

###  http://cdm.ovh/rsm/adapters/geosparql_adapter#Feature
:Feature rdf:type owl:Class ;
         rdfs:subClassOf <http://www.opengis.net/ont/geosparql#Feature> ;
         rdfs:comment "A discrete spatial phenomenon in the CDM universe of discourse."@en .


###  http://cdm.ovh/rsm/adapters/geosparql_adapter#Geometry
:Geometry rdf:type owl:Class ;
          rdfs:subClassOf <http://www.opengis.net/ont/geosparql#Geometry> ;
          <http://purl.org/dc/elements/1.1/source> "OGC 18-010r11"@en ;
          rdfs:comment "The reference system can be geographic, geodetic, cartesian (e.g. engineering coordinate system), and its definition may be part of the WKT or GML string. See OGC documentation."@en ;
          rdfs:label "Geometry"@en ;
          <http://www.w3.org/2004/02/skos/core#definition> "A coherent set of direct positions in space. The positions are held within a Spatial Reference System (SRS)."@en ;
          <http://www.w3.org/2004/02/skos/core#prefLabel> "Geometry"@en .


###  http://www.opengis.net/ont/geosparql#Feature
<http://www.opengis.net/ont/geosparql#Feature> rdf:type owl:Class .


###  http://www.opengis.net/ont/geosparql#Geometry
<http://www.opengis.net/ont/geosparql#Geometry> rdf:type owl:Class .


###  Generated by the OWL API (version 4.5.29.2024-05-13T12:11:03Z) https://github.com/owlcs/owlapi
