@prefix : <http://cdm.ovh/rsm/adapters/geosparql_adapter#> .
@prefix owl: <http://www.w3.org/2002/07/owl#> .
@prefix rdf: <http://www.w3.org/1999/02/22-rdf-syntax-ns#> .
@prefix rsm: <http://cdm.ovh/rsm/topology#> .
@prefix xml: <http://www.w3.org/XML/1998/namespace> .
@prefix xsd: <http://www.w3.org/2001/XMLSchema#> .
@prefix rdfs: <http://www.w3.org/2000/01/rdf-schema#> .
@base <http://cdm.ovh/rsm/adapters/geosparql_adapter#> .

<http://cdm.ovh/rsm/adapters/geosparql_adapter> rdf:type owl:Ontology ;
                                                 rdfs:comment "Adapter vocabulary for connecting various parts of RSM with GeoSPARQL 1.1."@en .

#################################################################
#    Object Properties
#################################################################

###  http://cdm.ovh/rsm/adapters/geosparql_adapter#hasGeometry
:hasGeometry rdf:type owl:ObjectProperty ;
             rdfs:subPropertyOf <http://www.opengis.net/ont/geosparql#hasGeometry> ;
             rdfs:comment "A spatial representation for a given Feature. As in GeoSPARQL, a feature can be associated with more than one geometry (valid at different times, or provided by different surveys...)."@en .


###  http://cdm.ovh/rsm/adapters/geosparql_adapter#hasNominalGeometry
:hasNominalGeometry rdf:type owl:ObjectProperty ;
                    rdfs:subPropertyOf :hasGeometry ,
                                       <http://www.opengis.net/ont/geosparql#hasDefaultGeometry> ;
                    rdfs:comment "The default Geometry to be used in spatial calculations. It is usually the most detailed Geometry. Takes into account SOSA/SSN viewpoint, i.e. there can be more than one default geometry (e.g. valid at different times)."@en .


###  http://www.opengis.net/ont/geosparql#hasDefaultGeometry
<http://www.opengis.net/ont/geosparql#hasDefaultGeometry> rdf:type owl:ObjectProperty ;
                                                          rdfs:subPropertyOf <http://www.opengis.net/ont/geosparql#hasGeometry> ;
                                                          rdfs:comment "The default Geometry to be used in spatial calculations. It is usually the most detailed Geometry."@en .


###  http://www.opengis.net/ont/geosparql#hasGeometry
<http://www.opengis.net/ont/geosparql#hasGeometry> rdf:type owl:ObjectProperty .


#################################################################
#    Data properties
#################################################################

###  http://cdm.ovh/rsm/adapters/geosparql_adapter#hasNominalMetricLength
:hasNominalMetricLength rdf:type owl:DatatypeProperty ;
                        rdfs:subPropertyOf <http://www.opengis.net/ont/geosparql#hasMetricLength> ;
                        rdfs:domain rsm:LinearElement ;
                        rdfs:range [ rdf:type rdfs:Datatype ;
                                     owl:onDatatype xsd:double ;
                                     owl:withRestrictions ( [ xsd:minInclusive "0.0"^^xsd:double
                                                            ]
                                                          )
                                   ] ;
                        rdfs:comment """Length (in meter) of a Linear Element to be assumed for conversions between linear referencing methods \"absolute\" (distance along) and \"interpolation\" (intrinsic coordinates, with values 0 to 1).
Length must be consistent with the chosen Nominal Geometry.
Compared to geo:hasMetricLength, a restriction was applied to the range (non-negative values)."""@en .


###  http://www.opengis.net/ont/geosparql#hasMetricLength
<http://www.opengis.net/ont/geosparql#hasMetricLength> rdf:type owl:DatatypeProperty ;
                                                       rdfs:range [ rdf:type rdfs:Datatype ;
                                                                    owl:onDatatype xsd:double ;
                                                                    owl:withRestrictions ( [ xsd:minInclusive "0.0"^^xsd:double
                                                                                           ]
                                                                                         )
                                                                  ] .


#################################################################
#    Classes
#################################################################

###  http://cdm.ovh/rsm/adapters/geosparql_adapter#Feature
:Feature rdf:type owl:Class ;
         rdfs:subClassOf <http://www.opengis.net/ont/geosparql#Feature> ;
         rdfs:comment "A discrete spatial phenomenon in the CDM universe of discourse."@en .


###  http://cdm.ovh/rsm/adapters/geosparql_adapter#Geometry
:Geometry rdf:type owl:Class ;
          rdfs:subClassOf <http://www.opengis.net/ont/geosparql#Geometry> ;
          rdfs:comment "A coherent set of direct positions in space. The positions are held within a Spatial Reference System (SRS)."@en .


###  http://cdm.ovh/rsm/topology#LinearElement
rsm:LinearElement rdf:type owl:Class .


###  http://www.opengis.net/ont/geosparql#Feature
<http://www.opengis.net/ont/geosparql#Feature> rdf:type owl:Class .


###  http://www.opengis.net/ont/geosparql#Geometry
<http://www.opengis.net/ont/geosparql#Geometry> rdf:type owl:Class .


###  Generated by the OWL API (version 4.5.26.2023-07-17T20:34:13Z) https://github.com/owlcs/owlapi
